# baseURI: http://loop3d.org/GSO/ontology/2020/1/geologicquality/ontology
# imports: http://loop3d.org/GSO/ontology/2020/1/common/ontology

@prefix gsoc: <http://loop3d.org/GSO/ontology/2020/1/common/> .
@prefix gsog: <http://loop3d.org/GSO/ontology/2020/1/geologicfeature/> .
@prefix gsoq: <http://loop3d.org/GSO/ontology/2020/1/geologicquality/> .
@prefix owl: <http://www.w3.org/2002/07/owl#> .
@prefix rdf: <http://www.w3.org/1999/02/22-rdf-syntax-ns#> .
@prefix rdfs: <http://www.w3.org/2000/01/rdf-schema#> .
@prefix xml: <http://www.w3.org/XML/1998/namespace> .
@prefix xsd: <http://www.w3.org/2001/XMLSchema#> .

gsoq:Azimuth
  a owl:Class ;
  rdfs:comment "Bearing of a horizontal line relative to north. Use for specifying the orientation of planar or linear features."@en ;
  rdfs:label "Azimuth"@en ;
  rdfs:subClassOf gsoq:Orientation ;
  rdfs:subClassOf [
      a owl:Restriction ;
      owl:onProperty gsoc:hasQuality ;
      owl:someValuesFrom gsoc:Measured_Value ;
    ] ;
.
gsoq:Density
  a owl:Class ;
  rdfs:comment "The mass per unit volume of an Amount of Matter"@en ;
  rdfs:label "Density "@en ;
  rdfs:subClassOf gsoc:Determinable_Quality ;
  rdfs:subClassOf [
      a owl:Restriction ;
      owl:allValuesFrom gsoc:Amount_Of_Matter ;
      owl:onProperty gsoc:isQualityOf ;
    ] ;
.
gsoq:Diameter
  a owl:Class ;
  rdfs:comment "The (approximate) average length of line segments that pass through the center of an object and whose endpoints lie on the outside boundary of the object. Use to characterize the size of a broadly spheroidal object like a pluton or a rock sample."@en ;
  rdfs:label "Diameter "@en ;
  rdfs:subClassOf gsoc:Determinable_Quality ;
  rdfs:subClassOf [
      a owl:Restriction ;
      owl:onProperty gsoc:hasValue ;
      owl:someValuesFrom gsoc:Numeric_Value ;
    ] ;
.
gsoq:Dip
  a owl:Class ;
  rdfs:comment "the maximum angle between a horizontal surface and a planar feature"@en ;
  rdfs:label "Dip"@en ;
  rdfs:subClassOf gsoq:Orientation ;
  rdfs:subClassOf [
      a owl:Restriction ;
      owl:onProperty gsoc:hasQuality ;
      owl:someValuesFrom gsoc:Measured_Value ;
    ] ;
.
gsoq:Dominant_Constituent
  a owl:Class ;
  rdfs:comment "Constituent is one of the most abundant."@en ;
  rdfs:comment "Example-- in a typical granite, Quartz, plagioclase, and K-feldspar are the dominant constituents."@en ;
  rdfs:label "Dominant Constituent"@en ;
  rdfs:subClassOf gsoq:Present ;
.
gsoq:Facing
  a owl:Class ;
  rdfs:comment "property to specify if a surface is directed, i.e. has a top and bottom. Values: {upright, overturned, unknown}"@en ;
  rdfs:label "facing direction"@en ;
  rdfs:subClassOf gsoq:Orientation ;
.
gsoq:Line_Orientation
  a owl:Class ;
  rdfs:comment "specification of the orientation of a line in space, using a trend (bearing of horizontal projection of line relative to geographic north) and plunge (inclination of line measured positive downward in degrees from local horizontal).  TBD:  add 'isdirected property to indicate if the line is directed (e.g. sense of shear), values should be Boolean,"@en ;
  rdfs:label "Line orientation"@en ;
  rdfs:subClassOf gsoq:Orientation ;
  rdfs:subClassOf [
      a owl:Restriction ;
      owl:allValuesFrom [
          a owl:Class ;
          owl:unionOf [
              a rdf:List ;
              rdf:first gsoq:Azimuth ;
              rdf:rest [
                  a rdf:List ;
                  rdf:first gsoq:Plunge ;
                  rdf:rest () ;
                ] ;
            ] ;
        ] ;
      owl:onProperty gsoc:hasQuality ;
    ] ;
.
gsoq:Magnetic_Susceptibility
  a owl:Class ;
  rdfs:comment "a measure of how much a material will become magnetized in an applied magnetic field. It is the ratio of magnetization M (magnetic moment per unit volume) to the applied magnetizing field intensity H. This allows a simple classification, into two categories, of most materials' responses to an applied magnetic field: an alignment with the magnetic field, χ > 0, called paramagnetism, or an alignment against the field, χ < 0, called diamagnetism."@en ;
  rdfs:comment "dct:source -- https://en.wikipedia.org/wiki/Magnetic_susceptibility" ;
  rdfs:label "Magnetic susceptibility "@en ;
  rdfs:subClassOf gsoc:Determinable_Quality ;
  rdfs:subClassOf [
      a owl:Restriction ;
      owl:allValuesFrom gsoc:Amount_Of_Matter ;
      owl:onProperty gsoc:isQualityOf ;
    ] ;
.
gsoq:Metamorphic_Facies
  a owl:Class ;
  rdfs:comment "Categories that characterize mineral assemblages indicative of certain metamorphic P-T conditions. Examples include Barrovian metasedimentary zones (eg: biotite facies, kyanite facies) or assemblages developed in rocks of more mafic composition (eg: greenschist facies, amphibolite facies)."@en ;
  rdfs:comment "applies to Rock_Material or Geologic_Unit"@en ;
  rdfs:isDefinedBy "GeoSciML v4"@en ;
  rdfs:label "Metamorphic facies"@en ;
  rdfs:subClassOf gsoc:Determinable_Quality ;
.
gsoq:Metamorphic_Grade
  a owl:Class ;
  rdfs:comment "A term to indicate the intensity or rank of metamorphism applied to an EarthMaterial (eg: high metamorphic grade, low metamorphic grade). Indicates in a general way the P-T environment in which the metamorphism took place. Determination of metamorphic grade is based on mineral assemblages (ie, facies) present in a rock that are interpreted to have crystallized in equilibrium during a particular metamorphic event."@en ;
  rdfs:comment "applies to Earth_Material or Geologic_Unit"@en ;
  rdfs:isDefinedBy "GeoSciML v4"@en ;
  rdfs:label "Metamorphic grade"@en ;
  rdfs:subClassOf gsoc:Determinable_Quality ;
.
gsoq:Minor_Constituent
  a owl:Class ;
  rdfs:comment "Constituent is ubiquitous but not abundant"@en ;
  rdfs:comment "Example -- in some granites, hornblende is a minor constituent."@en ;
  rdfs:label "Minor Constituent"@en ;
  rdfs:subClassOf gsoq:Present ;
.
gsoq:Orientation
  a owl:Class ;
  rdfs:comment "quality used to specify the disposition of a line or plane in space"@en ;
  rdfs:label "Orientation"@en ;
  rdfs:subClassOf gsoc:Determinable_Quality ;
.
gsoq:Overturned
  a owl:Class ;
  rdfs:comment "top of surface is facing downward, toward Earth interior."@en ;
  rdfs:label "Overturned facing"@en ;
  rdfs:subClassOf gsoq:Facing ;
.
gsoq:Peak_Pressure
  a owl:Class ;
  rdfs:comment "applies to Earth_Material or Geologic_Unit"@en ;
  rdfs:comment "peak metamorphic pressure"@en ;
  rdfs:isDefinedBy "GeoSciML v3"@en ;
  rdfs:label "Peak pressure"@en ;
  rdfs:subClassOf gsoc:Determinable_Quality ;
.
gsoq:Peak_Temperature
  a owl:Class ;
  rdfs:comment "applies to Earth_Material or Geologic_Unit"@en ;
  rdfs:comment "peak metamorphic temperature"@en ;
  rdfs:isDefinedBy "GeoSciML v3"@en ;
  rdfs:label "Peak temperature"@en ;
  rdfs:subClassOf gsoc:Determinable_Quality ;
.
gsoq:Plane_Orientation
  a owl:Class ;
  rdfs:comment "Quality to specify the orientation of a surface in a geogaphic reference system"@en ;
  rdfs:label "Plane orientation "@en ;
  rdfs:subClassOf gsoq:Orientation ;
.
gsoq:Plane_Orientation_dip_dipdir
  a owl:Class ;
  rdfs:comment "specification of the orientation of a plane in space, using a dip (inclination of line of maximum inclination contained in the plane, measured positive downward in degrees from local horizontal) and the azimuth normal to the strike in the dip direction"@en ;
  rdfs:label "Plane orientation (dip and dip direction)"@en ;
  rdfs:subClassOf gsoq:Plane_Orientation ;
  rdfs:subClassOf [
      a owl:Restriction ;
      owl:allValuesFrom [
          a owl:Class ;
          owl:unionOf [
              a rdf:List ;
              rdf:first gsoq:Azimuth ;
              rdf:rest [
                  a rdf:List ;
                  rdf:first gsoq:Dip ;
                  rdf:rest [
                      a rdf:List ;
                      rdf:first gsoq:Facing ;
                      rdf:rest () ;
                    ] ;
                ] ;
            ] ;
        ] ;
      owl:onProperty gsoc:hasQuality ;
    ] ;
.
gsoq:Plane_Orientation_strike_dip
  a owl:Class ;
  rdfs:comment "A plane orientation reported with the Azimuth value in the direction of strike such that the dip is to the right when facing in the azimuth direction."@en ;
  rdfs:label "Plane orientation (strike and dip)"@en ;
  rdfs:subClassOf gsoq:Plane_Orientation ;
  rdfs:subClassOf [
      a owl:Restriction ;
      owl:allValuesFrom [
          a owl:Class ;
          owl:unionOf (
              gsoq:Azimuth
              gsoq:Dip
              gsoq:Facing
            ) ;
        ] ;
      owl:onProperty gsoc:hasQuality ;
    ] ;
.
gsoq:Plunge
  a owl:Class ;
  rdfs:comment "Numeric value should be between +90 and -90.   Negative values only valid if the linear feature is directed."@en ;
  rdfs:label "Plunge"@en ;
  rdfs:subClassOf gsoq:Orientation ;
  rdfs:subClassOf [
      a owl:Restriction ;
      owl:onProperty gsoc:hasQuality ;
      owl:someValuesFrom gsoc:Measured_Value ;
    ] ;
.
gsoq:Present
  a owl:Class ;
  rdfs:comment "A constituent is present, but in an unknown proportion."@en ;
  rdfs:comment "This quality and its sub classes are used to express proportions when quantitiative measured values are not available."@en ;
  rdfs:label "Present"@en ;
  rdfs:subClassOf gsoc:Proportion ;
.
gsoq:Rare_Constituent
  a owl:Class ;
  rdfs:comment "Constituent is present but uncommon and rarely observed."@en ;
  rdfs:comment "Example-- in a typical granite, zircon and apatite are rare constituents"@en ;
  rdfs:label "Rare constituent "@en ;
  rdfs:subClassOf gsoq:Present ;
.
gsoq:Subordinate_Constituent
  a owl:Class ;
  rdfs:comment "Constituent is less abundant than dominant constituent, but present in sufficient abundance to be an obvious constituent"@en ;
  rdfs:comment "Example--in a typical granite, biotite is a subordinate constituent."@en ;
  rdfs:label "Subordinate Constituent"@en ;
  rdfs:subClassOf gsoq:Present ;
.
gsoq:Thickness
  a owl:Class ;
  rdfs:comment "Quality of a tabular or sheet like body that is its linear dimension normal to its long dimensions. Could be quantified numerically or categorically (e.g. thin, thick, very thick)"@en ;
  rdfs:label "Thickness"@en ;
  rdfs:subClassOf gsoc:Determinable_Quality ;
.
gsoq:Unknown_Facing
  a owl:Class ;
  rdfs:comment "Facing direction is unknown {@en}	"@en ;
  rdfs:label "Unknown Facing Direction"@en ;
  rdfs:subClassOf gsoq:Facing ;
.
gsoq:Upright
  a owl:Class ;
  rdfs:comment "top of surface is away from center of earth."@en ;
  rdfs:label "Upright Facing"@en ;
  rdfs:subClassOf gsoq:Facing ;
.
gsoq:ontology
  a owl:Ontology ;
  rdfs:comment "Vocabulary of geologic physical properties used in multiple GSO modules."@en ;
  rdfs:label "Physical qualities"@en ;
  owl:imports gsoc:ontology ;
.
