# baseURI: http://loop3d.org/GSO/ontology/2020/1/geologicstructure/fold/ontology
# imports: http://loop3d.org/GSO/ontology/2020/1/common/ontology

@prefix : <http://loop3d.org/GSO/ontology/2020/1/geologicstructure/fold/> .
@prefix gsoc: <http://loop3d.org/GSO/ontology/2020/1/common/> .
@prefix gsog: <http://loop3d.org/GSO/ontology/2020/1/geologicfeature/> .
@prefix gsoq: <http://loop3d.org/GSO/ontology/2020/1/geologicquality/> .
@prefix owl: <http://www.w3.org/2002/07/owl#> .
@prefix rdf: <http://www.w3.org/1999/02/22-rdf-syntax-ns#> .
@prefix rdfs: <http://www.w3.org/2000/01/rdf-schema#> .
@prefix xml: <http://www.w3.org/XML/1998/namespace> .
@prefix xsd: <http://www.w3.org/2001/XMLSchema#> .

:Upright_Inclination
  a owl:Class ;
  rdfs:comment "Surface dips between 80 and 90 degrees, used to describe orientation of fold hinge surface or axial surface;  use equivalent term 'Vertical inclination' for other geologic surfaces."@en ;
  rdfs:comment "dct:source -- Fleuty (1964) Folds classification." ;
  rdfs:label "Upright inclination"@en ;
  rdfs:subClassOf gsoq:Plane_Orientation ;
.

:Recumbent
  a owl:Class ;
  rdfs:comment "Surface dips between 0 and 10 degrees; typically used to describe orientation of fold hing surface or axial surface, use equivalent term 'Horizontal inclination' for other geologic surfaces."@en ;
  rdfs:comment "dct:source -- Fleuty (1964) Folds classification." ;
  rdfs:label "Recumbent "@en ;
  rdfs:subClassOf gsoq:Plane_Orientation ;
.

:Anticline
  a owl:Class ;
  rdfs:comment "A fold whose core contains the stratigraphically older rocks"@en ;
  rdfs:comment "dct:source -- https://inspire.ec.europa.eu/codelist/FoldProfileTypeValue/anticline" ;
  rdfs:label "Anticline "@en ;
  rdfs:subClassOf gsog:Fold ;
.
:Antiform
  a owl:Class ;
  rdfs:comment "A convex-upward, concave downward fold."@en ;
  rdfs:comment "dct:source -- https://inspire.ec.europa.eu/codelist/FoldProfileTypeValue/antiform" ;
  rdfs:label "Antiform"@en ;
  rdfs:subClassOf gsog:Fold ;
.
:Chevron_Fold
  a owl:Class ;
  rdfs:comment "A fold with straight limbs and sharp hinges. Well developed, these folds develop repeated set of v-shaped beds.  Inter-limb angles are generally 60 degrees or less. Chevron folding preferentially occurs in well bedded units where  bedding regularly alternates between contrasting competences."@en ;
  rdfs:comment "dct:source -- http://www.geologyin.com/2015/02/types-of-folds-with-photos.html" ;
  rdfs:label "Chevron Fold "@en ;
  rdfs:subClassOf gsog:Fold ;
.
:Fold_Amplitude
  a owl:Class ;
  rdfs:comment "the length of half the distance from the crest of a fold to the adjacent troughs. "@en ;
  rdfs:label "Fold Amplitude"@en ;
  rdfs:subClassOf gsoc:Determinable_Quality ;
  rdfs:subClassOf [
      a owl:Restriction ;
      owl:allValuesFrom gsog:Fold ;
      owl:onProperty gsoc:isQualityOf ;
    ] ;
  rdfs:subClassOf [
      a owl:Restriction ;
      owl:onProperty gsoc:hasDataValue ;
      owl:someValuesFrom xsd:decimal ;
    ] ;
  rdfs:subClassOf [
      a owl:Restriction ;
      owl:onProperty gsoc:hasUOM ;
      owl:someValuesFrom gsoc:Unit_of_Measure ;
    ] ;
.
:Fold_Axial_Surface
  a owl:Class ;
  rdfs:comment "Abstract surface that bisects the limbs of a fold or is the normal to a surface defined by the poles to the folded surface (typically visualized on a stereonet).  The axial surface of a particular fold may be located based on observations of the folded geologic structure, but in general it has no direct physical manifestation. Contrast with hinge surface, which is defined as the surface containing a set of hinge lines in the stack of folded surfaces defining a fold structure.  As a geologic surface, the axial surface has geometric properties, including orientation, which may be specified by observations at one or more locations, or generalized using terminology (upright, inclined, reclined, recumbent, overturned). (revised from GeoSciML 3.2)"@en ;
  rdfs:isDefinedBy "Revised from GeoSciML v3.2"@en ;
  rdfs:label "Fold axial surface"@en ;
  rdfs:subClassOf gsoc:Low_Dimension_Feature ;
  rdfs:subClassOf [
      a owl:Restriction ;
      owl:allValuesFrom gsog:Fold ;
      owl:onProperty gsoc:hostedBy ;
    ] ;
  rdfs:subClassOf [
      a owl:Restriction ;
      owl:onProperty gsoc:hasQuality ;
      owl:someValuesFrom gsoq:Orientation ;
    ] ;
.
:Fold_Hinge
  a owl:Class ;
  rdfs:comment "the line linking points of maximum curvature on a folded surface (http://www.geosci.usyd.edu.au/users/prey/Teaching/Geos-2123/Folds/Sld22.html). A low-dimensional feature"@en ;
  rdfs:label "Fold Hinge"@en ;
  rdfs:subClassOf gsoc:Low_Dimension_Feature ;
  rdfs:subClassOf [
      a owl:Restriction ;
      owl:allValuesFrom gsog:Fold ;
      owl:onProperty gsoc:isPartOf ;
    ] ;
.
:Fold_Hinge_Surface
  a owl:Class ;
  rdfs:comment "Surface that contains the hinge lines in a stack of folded layers"@en ;
  rdfs:label "Fold - Hinge surface"@en ;
  rdfs:subClassOf gsoc:Low_Dimension_Feature ;
  rdfs:subClassOf [
      a owl:Restriction ;
      owl:allValuesFrom gsog:Fold ;
      owl:onProperty gsoc:isPartOf ;
    ] ;
  rdfs:subClassOf [
      a owl:Restriction ;
      owl:onProperty gsoc:hostedBy ;
      owl:someValuesFrom :Fold_Hinge ;
    ] ;
.
:Fold_InterLimb_Angle
  a owl:Class ;
  rdfs:comment "The angle between adjacent limbs of a fold, normally determined by drawing tangents to the fold limbs at the inflection points."@en ;
  rdfs:comment "dct:source -- Neuendorf et al., 2005" ;
  rdfs:isDefinedBy "GeoSciML v4"@en ;
  rdfs:label "Fold limb shape"@en ;
  rdfs:subClassOf gsoc:Determinable_Quality ;
  rdfs:subClassOf [
      a owl:Restriction ;
      owl:allValuesFrom gsog:Fold ;
      owl:onProperty gsoc:isQualityOf ;
    ] ;
.
:Fold_Limb
  a owl:Class ;
  rdfs:comment "The generally planar region of a fold which lies between two adjacent hinge lines and is confined between the zones of maximum curvature. A role played by some layered rock reated to the adjacent fold hinges.  Not necessarily a feature"@en ;
  rdfs:label "Fold Limb"@en ;
  rdfs:subClassOf gsog:Geologic_Structure ;
  rdfs:subClassOf [
      a owl:Restriction ;
      owl:allValuesFrom gsog:Fold ;
      owl:onProperty gsoc:isPartOf ;
    ] ;
  rdfs:subClassOf [
      a owl:Restriction ;
      owl:onProperty gsoc:hostedBy ;
      owl:someValuesFrom gsog:Geologic_Structure ;
    ] ;
.
:Fold_Limb_Shape
  a owl:Class ;
  rdfs:comment "Straight vs curved limbs, eg kink, chevron, sinusoidal, box"@en ;
  rdfs:isDefinedBy "GeoSciML v4"@en ;
  rdfs:label "Fold limb shape"@en ;
  rdfs:subClassOf gsoc:Shape ;
  rdfs:subClassOf [
      a owl:Restriction ;
      owl:allValuesFrom gsog:Fold ;
      owl:onProperty gsoc:isQualityOf ;
    ] ;
.
:Fold_Span
  a owl:Class ;
  rdfs:comment "linear distance between inflection points in a single fold (GeoSciML v3.2)"@en ;
  rdfs:isDefinedBy "GeoSciML v3.2"@en ;
  rdfs:label "Fold span"@en ;
  rdfs:subClassOf gsoc:Determinable_Quality ;
  rdfs:subClassOf [
      a owl:Restriction ;
      owl:allValuesFrom gsog:Fold ;
      owl:onProperty gsoc:isQualityOf ;
    ] ;
  rdfs:subClassOf [
      a owl:Restriction ;
      owl:onProperty gsoc:hasDataValue ;
      owl:someValuesFrom xsd:decimal ;
    ] ;
  rdfs:subClassOf [
      a owl:Restriction ;
      owl:onProperty gsoc:hasUOM ;
      owl:someValuesFrom gsoc:Unit_of_Measure ;
    ] ;
.
:Fold_Symmetry
  a owl:Class ;
  rdfs:comment "Concordance or discordance of bisecting surface and axial surface, or ratio of length of limbs. Folded surface may have asymmetry defined by limb length ratio if inflection points are defined. Definition based on bisecting surface/axial surface angle depends on having multiple surfaces defined such that the axial surface may be identified. (symmetric, assymetric)"@en ;
  rdfs:isDefinedBy "GeoSciML v4"@en ;
  rdfs:label "Fold symmetry"@en ;
  rdfs:subClassOf gsoc:Determinable_Quality ;
  rdfs:subClassOf [
      a owl:Restriction ;
      owl:allValuesFrom gsog:Fold ;
      owl:onProperty gsoc:isQualityOf ;
    ] ;
.
:Fold_System
  a owl:Class ;
  rdfs:comment "A collection of congruent folds  (axis and axial surface are parallel) produced by the same tectonic event. Sometimes referred to as a \"Fold Train\". (GeoSciML 4.0.1)"@en ;
  rdfs:label "Fold System"@en ;
  rdfs:subClassOf gsog:Geologic_Structure ;
  rdfs:subClassOf [
      a owl:Restriction ;
      owl:allValuesFrom gsog:Fold ;
      owl:onProperty gsoc:hasPart ;
    ] ;
.
:Fold_Wavelength
  a owl:Class ;
  rdfs:comment "The distance between adjacent crest or trough of  a single fold, or the average distance between adjacent crests or troughs in a fold system. "@en ;
  rdfs:label "Fold wavelength"@en ;
  rdfs:subClassOf gsoc:Determinable_Quality ;
  rdfs:subClassOf [
      a owl:Restriction ;
      owl:allValuesFrom [
          a owl:Class ;
          owl:unionOf [
              a rdf:List ;
              rdf:first gsog:Fold ;
              rdf:rest [
                  a rdf:List ;
                  rdf:first :Fold_System ;
                  rdf:rest () ;
                ] ;
            ] ;
        ] ;
      owl:onProperty gsoc:isQualityOf ;
    ] ;
  rdfs:subClassOf [
      a owl:Restriction ;
      owl:onProperty gsoc:hasDataValue ;
      owl:someValuesFrom xsd:decimal ;
    ] ;
  rdfs:subClassOf [
      a owl:Restriction ;
      owl:onProperty gsoc:hasUOM ;
      owl:someValuesFrom gsoc:Unit_of_Measure ;
    ] ;
.

:Hinge_Line_Curvature
  a owl:Class ;
  rdfs:comment "Variation in orientation of fold hinge along trend of fold, distinguish sheath from cylindrical folds. Specify with terminology eg sheath, dome, basin, cylindrical."@en ;
  rdfs:isDefinedBy "GeoSciML v4"@en ;
  rdfs:label "Fold hinge line curvature"@en ;
  rdfs:subClassOf gsoc:Determinable_Quality ;
  rdfs:subClassOf [
      a owl:Restriction ;
      owl:allValuesFrom gsog:Fold ;
      owl:onProperty gsoc:isQualityOf ;
    ] ;
.
:Hinge_Shape
  a owl:Class ;
  rdfs:comment "Rounded vs. angular hinge zones; has to do with the proportion of the wavelength that is considered part of hinge"@en ;
  rdfs:isDefinedBy "GeoSciML v4"@en ;
  rdfs:label "Fold hinge shape"@en ;
  rdfs:subClassOf gsoc:Shape ;
  rdfs:subClassOf [
      a owl:Restriction ;
      owl:allValuesFrom gsog:Fold ;
      owl:onProperty gsoc:isQualityOf ;
    ] ;
.

:Is_Periodic
  a owl:Class ;
  rdfs:comment "boolean value, true if wavelength of folds in a fold system is approximately the same"@en ;
  rdfs:label "Folds are periodic"@en ;
  rdfs:subClassOf gsoc:Determinable_Quality ;
  rdfs:subClassOf [
      a owl:Restriction ;
      owl:allValuesFrom :Fold_System ;
      owl:onProperty gsoc:isQualityOf ;
    ] ;
.

:Monocline
  a owl:Class ;
  rdfs:comment "dct:source -- https://en.wikipedia.org/wiki/Monocline" ;
  rdfs:comment "step-like fold in rock strata consisting of a zone of steeper dip within an otherwise horizontal or gently-dipping sequence."@en ;
  rdfs:label "Monocline "@en ;
  rdfs:subClassOf gsog:Fold ;
.
:Neutral_Fold
  a owl:Class ;
  rdfs:comment "A fold which closes laterally and is therefore neither antiformal nor synformal.  "@en ;
  rdfs:comment "dct:source -- https://www.encyclopedia.com/science/dictionaries-thesauruses-pictures-and-press-releases/neutral-fold" ;
  rdfs:label "Neutral Fold "@en ;
  rdfs:subClassOf gsog:Fold ;
.

:Ptygmatic_Fold
  a owl:Class ;
  rdfs:comment "Chaotic and highly sinuous fold typically in an isolated layer within a more homogeneous rock body. Typical of sedimentary slump folding and veins or dikes in medium to high-grade metamorphic rocks"@en ;
  rdfs:label "Ptygmatic Fold "@en ;
  rdfs:subClassOf gsog:Fold ;
.

:Recumbent_Fold
  a owl:Class ;
  rdfs:comment "A fold that has an essentially horizontal axial plane."@en ;
  rdfs:comment "dct:source -- Fleuty (1964) Folds classification." ;
  rdfs:label "Recumbent Fold "@en ;
  rdfs:subClassOf :Neutral_Fold ;
.

:Syncline
  a owl:Class ;
  rdfs:comment "A fold of which the core contains the stratigraphically younger rocks"@en ;
  rdfs:comment "dct:source -- https://inspire.ec.europa.eu/codelist/FoldProfileTypeValue/syncline" ;
  rdfs:label "Syncline "@en ;
  rdfs:subClassOf gsog:Fold ;
.
:Synform
  a owl:Class ;
  rdfs:comment "A convex-downward, concave upward fold."@en ;
  rdfs:comment "dct:source -- based on https://inspire.ec.europa.eu/codelist/FoldProfileTypeValue/antiform" ;
  rdfs:label "Synform"@en ;
  rdfs:subClassOf gsog:Fold ;
.

:Vertical_Fold
  a owl:Class ;
  rdfs:comment "A fold for which the fold axis is vertical and axial surface is upright."@en ;
  rdfs:comment "dct:source -- Fleuty (1964) Folds classification." ;
  rdfs:label "Vertical Fold "@en ;
  rdfs:subClassOf :Neutral_Fold ;
.

:ontology
  a owl:Ontology ;
  rdfs:comment "extension module for properties related to folds"@en ;
  owl:imports gsoc:ontology ;
.
