# baseURI: http://loop3d.org/GSO/ontology/2020/1/uom/ontology
# imports: http://loop3d.org/GSO/ontology/2020/1/common/ontology

@prefix : <http://loop3d.org/GSO/ontology/2020/1/uom/> .
@prefix gsoum: <http://loop3d.org/GSO/ontology/2020/1/uom/> .
@prefix gsoc: <http://loop3d.org/GSO/ontology/2020/1/common/> .

@prefix owl: <http://www.w3.org/2002/07/owl#> .
@prefix rdf: <http://www.w3.org/1999/02/22-rdf-syntax-ns#> .
@prefix rdfs: <http://www.w3.org/2000/01/rdf-schema#> .
@prefix skos: <http://www.w3.org/2004/02/skos/core#> .
@prefix xsd: <http://www.w3.org/2001/XMLSchema#> .

:degree
  rdf:type owl:Class ;
  rdfs:comment "a measurement of a plane angle, defined so that a full rotation is 360 degrees"@en ;
  rdfs:comment "dct:source--  https://en.wikipedia.org/wiki/Degree_(angle)"@en ;
  rdfs:comment "skos:altLabel--  °"@en ;
  rdfs:label "degree"@en ;
  rdfs:subClassOf gsoc:Unit_Of_Measure ;
.
:gramspercubiccm
  rdf:type owl:Class ;
  rdfs:comment "CGS unit of density"@en ;
  rdfs:comment "skos:altLabel--  g/cm3"@en ;
  rdfs:label "Grams per Cubic Centimeter"@en ;
  rdfs:subClassOf gsoc:Unit_Of_Measure ;
.
:ma
  rdf:type owl:Class ;
  rdfs:comment "a unit of time equal to one million, or 1 E6 yr., measured from 1950 as 'present'"@en ;
  rdfs:comment "skos:altLabel--  Ma"@en ;
  rdfs:label "Million years before present"@en ;
  rdfs:subClassOf gsoc:Unit_Of_Measure ;
.
:meter
  rdf:type owl:Class ;
  rdfs:comment "a unit of length equal to the length of the path travelled by light in vacuum during a time interval of 1/299,792,458 of a second. (https://www.nationalgeographic.org/thisday/mar30/meter-defined/)"@en ;
  rdfs:comment "skos:altLabel--  m"@en ;
  rdfs:label "meter"@en ;
  rdfs:subClassOf gsoc:Unit_Of_Measure ;
.
:millimeter
  rdf:type owl:Class ;
  rdfs:comment "a unit of length equal to one thousandth of a meter and equivalent to 0.03937 inch."@en ;
  rdfs:comment "skos:altLabel--  mm"@en ;
  rdfs:label "millimeter"@en ;
  rdfs:subClassOf gsoc:Unit_Of_Measure ;
.
:ontology
  rdf:type owl:Ontology ;
  rdfs:comment "Stephen M. Richard 2019-12-10"@en ;
  rdfs:comment "simple vocabulary for units of measure. TBD: generate mapping to QUDT or other UOM ontologies with more semantics and content as necessary"@en ;
  owl:imports gsoc:ontology ;
.
:percent
  rdf:type owl:Class ;
  rdfs:comment "fraction of a whole, expressed as a fraction of 100, a unitless ratio value"@en ;
  rdfs:comment "skos:altLabel--  %"@en ;
  rdfs:label "percent"@en ;
  rdfs:subClassOf gsoc:Unit_Of_Measure ;
.
:simagneticsusceptibility
  rdf:type owl:Class ;
  rdfs:comment "Magnetic susceptibility is a dimensionless proportionality constant that indicates the degree of magnetization of a material in response to an applied magnetic field.  Here M = chi * H. Where M is the magnetization of the material (the magnetic dipole moment per unit volume), measured in amperes per meter, and H is the magnetic field strength, also measured in amperes per meter. Chi is therefore a dimensionless quantity."@en ;
  rdfs:comment "skos:altLabel -- greek letter chi"@en ;
  rdfs:label "SI Susceptibility"@en ;
  rdfs:subClassOf gsoc:Unit_Of_Measure ;
  owl:imports gsoc:ontology ; 
.
