# baseURI: http://loop3d.org/GSO/ontology/2020/1/geologicprocess/ontology

@prefix : <http://loop3d.org/GSO/ontology/2020/1/geologicprocess/> .
@prefix gsoc: <http://loop3d.org/GSO/ontology/2020/1/common/> .
@prefix gsog: <http://loop3d.org/GSO/ontology/2020/1/geologicfeature/> .
@prefix gsoq: <http://loop3d.org/GSO/ontology/2020/1/geologicquality/> .
@prefix gspr: <http://loop3d.org/GSO/ontology/2020/1/geologicprocess/> .
@prefix owl: <http://www.w3.org/2002/07/owl#> .
@prefix rdf: <http://www.w3.org/1999/02/22-rdf-syntax-ns#> .
@prefix rdfs: <http://www.w3.org/2000/01/rdf-schema#> .
@prefix xml: <http://www.w3.org/XML/1998/namespace> .
@prefix xsd: <http://www.w3.org/2001/XMLSchema#> .

gspr:Accretion
  a owl:Class ;
  rdfs:comment "The addition of material to a continent. Typically involves convergent or transform motion."@en ;
  rdfs:comment "dct:source--  Neuendorf, K.K.E, Mehl, J.P. & Jackson, J.A. (eds), 2005. Glossary of geology, 5th Edition. American Geological Institute, Alexandria, 779 p."@en ;
  rdfs:label "accretion"@en ;
  rdfs:subClassOf gsog:Additive_Process ;
  rdfs:subClassOf gspr:Tectonic_Process ;
.
gspr:Biological_Evolution
  a owl:Class ;
  rdfs:label "Evolution"@en ;
  rdfs:subClassOf gspr:Biological_Process ;
.
gspr:Biological_Precipitation
  a owl:Class ;
  rdfs:comment "The deposition of minerals from solution by the agency of organisms"@en ;
  rdfs:comment "dct:source--  this vocabulary"@en ;
  rdfs:label "biological precipitation"@en ;
  rdfs:subClassOf gspr:Deposition ;
.
gspr:Biological_Process
  a owl:Class ;
  rdfs:label "Biological Process"@en ;
  rdfs:subClassOf gsoc:Process ;
.
gspr:Biological_Weathering
  a owl:Class ;
  rdfs:comment "breakdown of rocks by biological agents, e.g. the penetrating and expanding force of roots, the presence of moss and lichen causing humic acids to be retained in contact with rock, and the work of animals (worms, moles, rabbits) in modifying surface soil"@en ;
  rdfs:comment "dct:source--  Neuendorf, K.K.E, Mehl, J.P. & Jackson, J.A. (eds), 2005. Glossary of geology, 5th Edition. American Geological Institute, Alexandria, 779 p."@en ;
  rdfs:label "biological weathering"@en ;
  rdfs:subClassOf gspr:Weathering ;
.
gspr:Bolide_Impact
  a owl:Class ;
  rdfs:comment "Metamorphism resulting from the passage of a shock wave through a body of material, typically the result of impact of a planetary body (impactor) on a planetary surface (target)"@en ;
  rdfs:comment "dct:source--  Smulikowski et al, 2003"@en ;
  rdfs:label "impact process"@en ;
  rdfs:subClassOf gsog:Deformation ;
.
gspr:Cataclastic_Deformation
  a owl:Class ;
  rdfs:comment "Brittle deformation processes, i.e. the formation and growth of fractures and frictional sliding along fracture surfaces."@en ;
  rdfs:comment "dct:source--  based on Neuendorf et al 2005"@en ;
  rdfs:label "cataclastic deformation"@en ;
  rdfs:subClassOf gsog:Deformation ;
.
gspr:Chemical_Precipitation
  a owl:Class ;
  rdfs:comment "The deposition of mineral matter by precipitation from solution or as a result of chemical reactions. May be sedimentary or hydrothermal."@en ;
  rdfs:comment "dct:source--  Neuendorf, K.K.E, Mehl, J.P. & Jackson, J.A. (eds), 2005. Glossary of geology, 5th Edition. American Geological Institute, Alexandria, 779 p."@en ;
  rdfs:label "chemical precipitation"@en ;
  rdfs:subClassOf gspr:Deposition ;
  rdfs:subClassOf gspr:Metamorphic_Process ;
.
gspr:Chemical_Weathering
  a owl:Class ;
  rdfs:comment "The process of weathering by which chemical reactions (hydrolysishydration, oxidation, carbonation, ion exchange, and solution) transform rocks and minerals into new chemical combinations that are stable under conditions prevailing at or near the Earth's surface, e.g. the alteration of orthoclase to kaolinite."@en ;
  rdfs:comment "dct:source--  Neuendorf, K.K.E, Mehl, J.P. & Jackson, J.A. (eds), 2005. Glossary of geology, 5th Edition. American Geological Institute, Alexandria, 779 p."@en ;
  rdfs:label "chemical weathering"@en ;
  rdfs:subClassOf gspr:Weathering ;
.
gspr:Contact_Metamorphism
  a owl:Class ;
  rdfs:comment "Metamorphism taking place in rocks at or near their contact with a genetically related body of igneous rock"@en ;
  rdfs:comment "dct:source--  Neuendorf, K.K.E, Mehl, J.P. & Jackson, J.A. (eds), 2005. Glossary of geology, 5th Edition. American Geological Institute, Alexandria, 779 p."@en ;
  rdfs:label "contact metamorphism"@en ;
  rdfs:subClassOf gspr:Metamorphic_Process ;
.
gspr:Continental_Breakup
  a owl:Class ;
  rdfs:comment "Fragmentation of a continental plate into two or more smaller plates, may involve rifting or strike slip faulting."@en ;
  rdfs:comment "dct:source--  this vocabulary"@en ;
  rdfs:label "continental breakup"@en ;
  rdfs:subClassOf gsog:Deformation ;
  rdfs:subClassOf gspr:Tectonic_Process ;
.
gspr:Continental_Collision
  a owl:Class ;
  rdfs:comment "The amalgamation of two continental plates or blocks along a convergent margin."@en ;
  rdfs:comment "dct:source--  this vocabulary"@en ;
  rdfs:label "continental collision"@en ;
  rdfs:subClassOf gsog:Additive_Process ;
  rdfs:subClassOf gsog:Deformation ;
  rdfs:subClassOf gspr:Tectonic_Process ;
.
gspr:Debris_Flow_Deposition
  a owl:Class ;
  rdfs:comment "Laminar high-concentration, generally cohesionless deposition process. Flow types included liquefied flow, fluidized flow, grain flow, traction carpet or modified grain flow."@en ;
  rdfs:comment "dct:source--  Postma 1986 Geology v. 14 p291-294"@en ;
  rdfs:label "debris flow deposition"@en ;
  rdfs:subClassOf gspr:Mechanical_Deposition ;
.
gspr:Deep_Water_Oxygen_Depletion
  a owl:Class ;
  rdfs:comment "" ;
  rdfs:label "Deep Water Oxygen Depletion"@en ;
  rdfs:subClassOf gsog:Subtractive_Process ;
.
gspr:Deformation_Twinning
  a owl:Class ;
  rdfs:comment "Deformation of a crystal by gliding to produce crystallographic twinning."@en ;
  rdfs:comment "dct:source--  Neuendorf, K.K.E, Mehl, J.P. & Jackson, J.A. (eds), 2005. Glossary of geology, 5th Edition. American Geological Institute, Alexandria, 779 p."@en ;
  rdfs:label "deformation twinning"@en ;
  rdfs:subClassOf gsog:Transformation ;
.
gspr:Deposition
  a owl:Class ;
  rdfs:comment "Accumulation of material, the constructive process of accumulation of sedimentary particles, chemical precipitation of mineral matter from solution, or the accumulation of organic material on the death of plants and animals."@en ;
  rdfs:comment "dct:source--  Neuendorf, K.K.E, Mehl, J.P. & Jackson, J.A. (eds), 2005. Glossary of geology, 5th Edition. American Geological Institute, Alexandria, 779 p."@en ;
  rdfs:label "deposition"@en ;
  rdfs:subClassOf gsog:Additive_Process ;
  rdfs:subClassOf gspr:Rock_Forming_Process ;
  rdfs:subClassOf gspr:Sedimentary_Process ;
.
gspr:Deposition_Hiatus
  a owl:Class ;
  rdfs:comment "process in which a depositional surface does not accumulate sediment. Use to indicate paraconformable boundaries."@en ;
  rdfs:label "Deposition Hiatus "@en ;
  rdfs:subClassOf gspr:Sedimentary_Process ;
.
gspr:Diagenetic_Process
  a owl:Class ;
  rdfs:comment "Any chemical, physical, or biological process that affects a sedimentary EarthMaterial after initial deposition, and during or after lithification, exclusive of weathering and metamorphism. [adapt. Jackson, 1997] Example processes include compaction, cementation, authigenesis, replacement, leachinghydration, and bacterial action. Includes processes that are normal in the surficial or outer part of the earth’s crust [Jackson, 1997]. Changes in a deeply buried sedimentary rock may be continuous from diagenesis into recrystallization to form a metamorphic rock. Robertson [1999] defines the boundary between diagenesis and metamorphism in sedimentary rocks as follows: \\the boundary between diagenesis and metamorphism is somewhat arbitrary and strongly dependent on the rock types involved. For example changes take place in organic materials at lower temperatures than in rocks dominated by silicate minerals. In mudrocks, a white mica (illite) crystallinity value of less than 0.42D.2U obtained by X-ray diffraction analysis, is used to define the onset of metamorphism (Kisch, 1991). In this scheme, the first appearance of glaucophane, lawsonite, paragonite, prehnite, pumpellyite or stilpnomelane is taken to indicate the lower limit of metamorphism (Frey and Kisch, 1987, Bucher and Frey, 1994, Frey and Robinson, 1998). Most workers agree that such mineral growth starts at 150 ± 50° C in silicate rocks. Many rock types may show no change in mineralogy under these conditions and hence the recognition of the onset of metamorphism will vary with bulk composition.\\"@en ;
  rdfs:comment "dct:source--  Neuendorf, K.K.E, Mehl, J.P. & Jackson, J.A. (eds), 2005. Glossary of geology, 5th Edition. American Geological Institute, Alexandria, 779 p."@en ;
  rdfs:label "diagenetic process"@en ;
  rdfs:subClassOf gsog:Transformation ;
  rdfs:subClassOf gspr:Rock_Forming_Process ;
  rdfs:subClassOf gspr:Sedimentary_Process ;
.
gspr:Diffusion_Creep
  a owl:Class ;
  rdfs:comment "Grain-scale, ductile deformation accomplished by the motion of atoms through crystals, along grain boundaries, and through pore fluids."@en ;
  rdfs:comment "dct:source--  Neuendorf, K.K.E, Mehl, J.P. & Jackson, J.A. (eds), 2005. Glossary of geology, 5th Edition. American Geological Institute, Alexandria, 779 p."@en ;
  rdfs:label "diffusion creep"@en ;
  rdfs:subClassOf gsog:Transformation ;
.
gspr:Dislocation_Metamorphism
  a owl:Class ;
  rdfs:comment "Metamorphism concentrated along narrow belts of shearing or crushing without an appreciable rise in temperature"@en ;
  rdfs:comment "dct:source--  Neuendorf, K.K.E, Mehl, J.P. & Jackson, J.A. (eds), 2005. Glossary of geology, 5th Edition. American Geological Institute, Alexandria, 779 p."@en ;
  rdfs:label "dislocation metamorphism"@en ;
  rdfs:subClassOf gspr:Metamorphic_Process ;
.
gspr:Dissolution
  a owl:Class ;
  rdfs:comment "The process of dissolving into a homogenous solution, as when an acidic solution dissolves limestone. In karst, refers to the process of dissolving rock to produce landforms, in contrast to solution, the chemical product of dissolution."@en ;
  rdfs:comment "dct:source--  Neuendorf, K.K.E, Mehl, J.P. & Jackson, J.A. (eds), 2005. Glossary of geology, 5th Edition. American Geological Institute, Alexandria, 779 p."@en ;
  rdfs:label "dissolution"@en ;
  rdfs:subClassOf gsog:Subtractive_Process ;
  rdfs:subClassOf gspr:Chemical_Weathering ;
.
gspr:Dissolution_Creep
  a owl:Class ;
  rdfs:comment "Deformation by dissolution under the effects of differential stress and its transport to a new location by movement of fluid in the rock body."@en ;
  rdfs:comment "dct:source--  Neuendorf, K.K.E, Mehl, J.P. & Jackson, J.A. (eds), 2005. Glossary of geology, 5th Edition. American Geological Institute, Alexandria, 779 p."@en ;
  rdfs:label "dissolution creep"@en ;
  rdfs:subClassOf gsog:Transformation ;
.
gspr:Ductile_Flattening
  a owl:Class ;
  rdfs:comment "Also known as pure shear; a three-dimensional homogeneous flattening of a body (http://www.geology.sdsu.edu/visualstructure/vss/htm_hlp/pure_s.htm) accomodated by ductile deformation. It is an example of irrotational strain in which body is elongated in one direction while being shortened perpendicularly (https://en.wikipedia.org/wiki/Pure_shear)."@en ;
  rdfs:label "Ductile Flattening"@en ;
  rdfs:subClassOf gspr:Ductile_Flow ;
.
gspr:Ductile_Flow
  a owl:Class ;
  rdfs:comment "Deformation without apparent loss of continuity at the scale of observation."@en ;
  rdfs:comment "dct:source--  Neuendorf, K.K.E, Mehl, J.P. & Jackson, J.A. (eds), 2005. Glossary of geology, 5th Edition. American Geological Institute, Alexandria, 779 p."@en ;
  rdfs:label "ductile flow"@en ;
  rdfs:subClassOf gsog:Deformation ;
.
gspr:Ductile_Simple_Shear
  a owl:Class ;
  rdfs:comment "Simple shear accomodated by ductile deformation. Simple sheare is a deformation in which parallel planes in a material remain parallel and maintain a constant distance, while translating relative to each other (https://en.wikipedia.org/wiki/Simple_shear)."@en ;
  rdfs:label "Ductile Simple Shear"@en ;
  rdfs:subClassOf gspr:Ductile_Flow ;
  rdfs:subClassOf gspr:Shearing ;
.
gspr:Effusive_Eruption
  a owl:Class ;
  rdfs:comment "Eruptions characterized by low volatile content of the erupting magma relative to ambient pressure"@en ;
  rdfs:comment "dct:source--  Orton, G.J., 1996. Volcanic environments. 485-567 in Readingh.G. (ed.), Sedimentary Environments: Processes, Facies and Stratigraphy, Third Edition. Blackwell Science, Oxford"@en ;
  rdfs:label "effusive eruption"@en ;
  rdfs:subClassOf gspr:Eruption ;
.
gspr:Erosion
  a owl:Class ;
  rdfs:comment "The process of disaggregation of rock and displacement of the resultant particles (sediment) usually by the agents of currents such as, wind, water, or ice by downward or down-slope movement in response to gravity or by living organisms (in the case of bioerosion)."@en ;
  rdfs:comment "dct:source--  this vocabulary"@en ;
  rdfs:label "erosion"@en ;
  rdfs:subClassOf gsog:Subtractive_Process ;
  rdfs:subClassOf gspr:Sedimentary_Process ;
.
gspr:Eruption
  a owl:Class ;
  rdfs:comment "The ejection of volcanic materials (lava, pyroclasts, and volcanic gases) onto the Earth's surface, either from a central vent or from a fissure or group of fissures"@en ;
  rdfs:comment "dct:source--  Neuendorf, K.K.E, Mehl, J.P. & Jackson, J.A. (eds), 2005. Glossary of geology, 5th Edition. American Geological Institute, Alexandria, 779 p."@en ;
  rdfs:label "eruption"@en ;
  rdfs:subClassOf gsog:Additive_Process ;
  rdfs:subClassOf gspr:Magmatic_Process ;
  rdfs:subClassOf gspr:Rock_Forming_Process ;
.
gspr:Excavation
  a owl:Class ;
  rdfs:comment "The removal of material by human activity, as in a mining operation"@en ;
  rdfs:comment "dct:source--  this vocabulary"@en ;
  rdfs:label "excavation"@en ;
  rdfs:subClassOf gsog:Subtractive_Process ;
  rdfs:subClassOf gspr:Human_Activity ;
.
gspr:Extinction
  a owl:Class ;
  rdfs:comment "Process of disappearance of a species or higher taxon, so that it no longer exists anywhere or in the subsequent fossil record."@en ;
  rdfs:comment "dct:source--  this vocabulary"@en ;
  rdfs:label "extinction"@en ;
  rdfs:subClassOf gspr:Biological_Process ;
.
gspr:Faulting
  a owl:Class ;
  rdfs:comment "The process of fracturing, frictional slip, and displacement accumulation that produces a fault"@en ;
  rdfs:comment "dct:source--  Neuendorf, K.K.E, Mehl, J.P. & Jackson, J.A. (eds), 2005. Glossary of geology, 5th Edition. American Geological Institute, Alexandria, 779 p."@en ;
  rdfs:label "faulting"@en ;
  rdfs:subClassOf gsog:Deformation ;
.
gspr:Flexural_Slip
  a owl:Class ;
  rdfs:comment "A folding process in which shearing is concentrated as layer boundaries and the folded layers maintain a relatively constant thickness"@en ;
  rdfs:isDefinedBy "this vocabulary"@en ;
  rdfs:label "Flexural slip folding @en}" ;
  rdfs:subClassOf gspr:Folding ;
.
gspr:Folding
  a owl:Class ;
  rdfs:comment "Deformation in which planar surfaces become regularly curviplanar surfaces with definable limbs (zones of lower curvature) and hinges (zones of higher curvature)."@en ;
  rdfs:comment "dct:source--  this vocabulary"@en ;
  rdfs:label "folding"@en ;
  rdfs:subClassOf gsog:Deformation ;
.
gspr:Fracturing
  a owl:Class ;
  rdfs:comment "The formation of a surface of failure resulting from stress"@en ;
  rdfs:comment "dct:source--  this vocabulary"@en ;
  rdfs:label "fracturing"@en ;
  rdfs:subClassOf gsog:Deformation ;
.
gspr:Frost_Shattering
  a owl:Class ;
  rdfs:comment "Propagation of fractures due to expansion of freezing water in intergranular spaces and fractures in a rock body. Result is mechanical disintegration spliitting, or breakup of rock."@en ;
  rdfs:comment "dct:source--  Neuendorf, K.K.E, Mehl, J.P. & Jackson, J.A. (eds), 2005. Glossary of geology, 5th Edition. American Geological Institute, Alexandria, 779 p."@en ;
  rdfs:label "frost shattering"@en ;
  rdfs:subClassOf gspr:Physical_Weathering ;
.
gspr:Geodynamo_Process
  a owl:Class ;
  rdfs:comment "Process that generates electric currents due to the motion of convection currents of molten iron in the Earth's outer core, caused by heat escaping from the core. Process responsible for Earth’s magnetic field."@en ;
  rdfs:label "Geodynamo process"@en ;
  rdfs:subClassOf gspr:Geomagnetic_Process ;
.
gspr:Geomagnetic_Process
  a owl:Class ;
  rdfs:comment "dct:source--  this vocabulary"@en ;
  rdfs:comment "process that results in change in Earth's magnetic field"@en ;
  rdfs:label "Geomagnetic Process"@en ;
  rdfs:subClassOf gsog:Geologic_Process ;
  rdfs:subClassOf gsog:Transformation ;
.
gspr:Grading
  a owl:Class ;
  rdfs:comment "Leveling of earth surface by rearrangement of prexisting material"@en ;
  rdfs:comment "dct:source--  this vocabulary"@en ;
  rdfs:label "grading"@en ;
  rdfs:subClassOf gsog:Transformation ;
  rdfs:subClassOf gspr:Human_Activity ;
.
gspr:Haloclasty
  a owl:Class ;
  rdfs:comment "Propagation of fractures in rock due to crytallization of mineral salts (typically sodium chloride) from interstitial water, or volumetrick expansion of salts in capillaries, or hydration pressure of interstitial, trapped salts. Generally results in mechanical disintegration of the rock surface."@en ;
  rdfs:comment "dct:source--  Neuendorf, K.K.E, Mehl, J.P. & Jackson, J.A. (eds), 2005. Glossary of geology, 5th Edition. American Geological Institute, Alexandria, 779 p."@en ;
  rdfs:label "haloclasty"@en ;
  rdfs:subClassOf gspr:Physical_Weathering ;
.
gspr:Hawaiian_Eruption
  a owl:Class ;
  rdfs:comment "Eruption in which great quantities of extremely fluid basaltic lava are poured out, mainly issuing in lava fountains from fissures on the flanks of a volcano. Explosive phenomena are rare, but much spatter and scoria are piled into cones and mounds along the vents. Characteristic of shield volcanoes"@en ;
  rdfs:comment "dct:source--  Neuendorf, K.K.E, Mehl, J.P. & Jackson, J.A. (eds), 2005. Glossary of geology, 5th Edition. American Geological Institute, Alexandria, 779 p."@en ;
  rdfs:label "hawaiian eruption"@en ;
  rdfs:subClassOf gspr:Eruption ;
.
gspr:Human_Activity
  a owl:Class ;
  rdfs:comment "Processes of human modification of the earth to produce geologic features"@en ;
  rdfs:comment "dct:source--  this vocabulary"@en ;
  rdfs:label "Human Activity"@en ;
  rdfs:subClassOf gsoc:Process ;
.
gspr:Human_Deposition
  a owl:Class ;
  rdfs:comment "Human processes of material deposition, e.g. landfill, mining waste heaps, tailings, road-grade fill."@en ;
  rdfs:label "Human material deposition "@en ;
  rdfs:subClassOf gspr:Human_Activity ;
  rdfs:subClassOf gspr:Mechanical_Deposition ;
  rdfs:subClassOf gspr:Rock_Forming_Process ;
.
gspr:Hydration
  a owl:Class ;
  rdfs:comment "The process of absorption of water into the crystal structure of a mineral, thereby changing its volume and fracturing and loosening grains"@en ;
  rdfs:comment "dct:source--  this vocabulary"@en ;
  rdfs:label "hydration"@en ;
  rdfs:subClassOf gspr:Chemical_Weathering ;
.
gspr:Hydrolysis
  a owl:Class ;
  rdfs:comment "A decomposition reaction involving water. In geology, it commonly indicates reaction between silicate minerals and either pure water or aqueous solution. In such reactionsh"@en ;
  rdfs:comment "dct:source--  Neuendorf, K.K.E, Mehl, J.P. & Jackson, J.A. (eds), 2005. Glossary of geology, 5th Edition. American Geological Institute, Alexandria, 779 p."@en ;
  rdfs:label "hydrolysis"@en ;
  rdfs:subClassOf gspr:Chemical_Weathering ;
.
gspr:Ice_Erosion
  a owl:Class ;
  rdfs:comment "Erosion by corrasion or plucking by moving ice."@en ;
  rdfs:comment "dct:source--  this vocabulary"@en ;
  rdfs:label "ice erosion"@en ;
  rdfs:subClassOf gspr:Erosion ;
.
gspr:Intrusion_Process
  a owl:Class ;
  rdfs:comment "The process of emplacement of magma in pre-existing rock"@en ;
  rdfs:comment "dct:source--  Neuendorf, K.K.E, Mehl, J.P. & Jackson, J.A. (eds), 2005. Glossary of geology, 5th Edition. American Geological Institute, Alexandria, 779 p."@en ;
  rdfs:label "intrusion"@en ;
  rdfs:subClassOf gsog:Additive_Process ;
  rdfs:subClassOf gspr:Magmatic_Process ;
.
gspr:Lava_Flow
  a owl:Class ;
  rdfs:comment "process of melted rock flowing over the Earth's surface and solidifying to form new rock."@en ;
  rdfs:label "Lava Flow "@en ;
  rdfs:subClassOf gspr:Eruption ;
.
gspr:Magmatic_Cystallisation
  a owl:Class ;
  rdfs:comment "The process by which matter becomes crystalline, from a gaseous, fluid, or dispersed state"@en ;
  rdfs:comment "dct:source--  Neuendorf, K.K.E, Mehl, J.P. & Jackson, J.A. (eds), 2005. Glossary of geology, 5th Edition. American Geological Institute, Alexandria, 779 p."@en ;
  rdfs:label "magmatic crystallisation"@en ;
  rdfs:subClassOf gsog:Transformation ;
  rdfs:subClassOf gspr:Magmatic_Process ;
  rdfs:subClassOf gspr:Rock_Forming_Process ;
.
gspr:Magmatic_Process
  a owl:Class ;
  rdfs:comment "A process involving melted rock (magma)."@en ;
  rdfs:comment "dct:source--  this vocabulary"@en ;
  rdfs:label "Magmatic Process"@en ;
  rdfs:subClassOf gsog:Geologic_Process ;
.
gspr:Mass_Wasting
  a owl:Class ;
  rdfs:comment "dct:source--  Neuendorf, K.K.E, Mehl, J.P. & Jackson, J.A. (eds), 2005. Glossary of geology, 5th Edition. American Geological Institute, Alexandria, 779 p."@en ;
  rdfs:comment "the dislodgement and downslope transport of soil and rock material under the direct application of gravitational body stresses. In contrast to other erosion processes, the debris removed by mass wasting is not carried within, on, or under another medium. The mass properties of the material being transported depend on the interaction of the soil and rock particles and on the moisture content."@en ;
  rdfs:label "mass wasting"@en ;
  rdfs:subClassOf gspr:Erosion ;
.
gspr:Mass_Wasting_Deposition
  a owl:Class ;
  rdfs:comment "A general term for the dislodgement and downslope transport of soil and rock material under the direct application of gravitational body stresses. In contrast to other erosion processes, the debris removed by mass wasting is not carried within, on, or under another medium. The mass properties of the material being transported depend on the interaction of the soil and rock particles and on the moisture content. Mass wasting includes slow displacements, such as creep and solifluction, and rapid movements such as rockfalls, rockslides, and cohesive debris flows (Jackson, 1997, p. 392). Includes both subaerial mass-wasting processes and subaqueous mass-wasting processes."@en ;
  rdfs:comment "dct:source--  Neuendorf, K.K.E, Mehl, J.P. & Jackson, J.A. (eds), 2005. Glossary of geology, 5th Edition. American Geological Institute, Alexandria, 779 p."@en ;
  rdfs:label "mass wasting deposition"@en ;
  rdfs:subClassOf gspr:Mechanical_Deposition ;
.
gspr:Material_Transport
  a owl:Class ;
  rdfs:comment "Transport and heaping of material, as in a land fill, mine dump, dredging operations. Can be anthropogenic, or geologic transport process"@en ;
  rdfs:comment "dct:source--  this vocabulary"@en ;
  rdfs:label "Material Transport And Deposition"@en ;
  rdfs:subClassOf gsoc:Process ;
.
gspr:Mechanical_Deposition
  a owl:Class ;
  rdfs:comment "Process by which material that is being transported as particles by moving air, water, ice, or other fluid comes to rest and accumulates."@en ;
  rdfs:comment "dct:source--  NADM SLTTs 2004"@en ;
  rdfs:label "mechanical deposition"@en ;
  rdfs:subClassOf gspr:Deposition ;
.
gspr:Melting
  a owl:Class ;
  rdfs:comment "change of state from a solid to a liquid"@en ;
  rdfs:comment "dct:source--  this vocabulary"@en ;
  rdfs:label "melting"@en ;
  rdfs:subClassOf gsog:Transformation ;
  rdfs:subClassOf gspr:Magmatic_Process ;
.
gspr:Metamorphic_Process
  a owl:Class ;
  rdfs:comment "Mineralogical, chemical, and structural adjustment of solid rocks to physical and chemical conditions that differ from the conditions under which the rocks in question originated, and are generally been imposed at depth, below the surface zones of weathering and cementation."@en ;
  rdfs:comment "dct:source--  this vocabulary"@en ;
  rdfs:label "Metamorphic Process"@en ;
  rdfs:subClassOf gsog:Geologic_Process ;
  rdfs:subClassOf gsog:Transformation ;
.
gspr:Metasomatism
  a owl:Class ;
  rdfs:comment "Processes causing open-system changes in chemical composition by reaction with an external source, typically involving chemical transport by a fluid medium flowing through the rock. Metasomatism typically involves introduction of chemical constituents into a rock volume. General term for any change in the mineralogical or chemical composition of a rock. Typically related to interaction with hydrous fluids."@en ;
  rdfs:comment "dct:source--  Fettes and Desmons, 2007"@en ;
  rdfs:label "Metasomatism or hydrothermal process"@en ;
  rdfs:subClassOf gspr:Metamorphic_Process ;
.
gspr:Microfracturing
  a owl:Class ;
  rdfs:comment "Development of fractures within a single grain or cutting several grains."@en ;
  rdfs:comment "dct:source--  Neuendorf, K.K.E, Mehl, J.P. & Jackson, J.A. (eds), 2005. Glossary of geology, 5th Edition. American Geological Institute, Alexandria, 779 p."@en ;
  rdfs:label "microfracturing"@en ;
  rdfs:subClassOf gspr:Fracturing ;
.
gspr:Mountain_Building
  a owl:Class ;
  rdfs:comment "dct:source--  Neuendorf et al., 2005"@en ;
  rdfs:comment "orogenic process or mountain building process."@en ;
  rdfs:comment "skos:altLabel--  orogenesis"@en ;
  rdfs:label "Mountain building"@en ;
  rdfs:subClassOf gsog:Deformation ;
  rdfs:subClassOf gspr:Tectonic_Process ;
.
gspr:Obduction
  a owl:Class ;
  rdfs:comment "The overthrusting of continental crust by oceanic crust or mantle rocks at a convergent plate boundary."@en ;
  rdfs:comment "dct:source--  Neuendorf et al., 2005, http://en.wikipedia.org/wiki/Obduction, Coleman, R. G., 1971, Plate tectonic emplacement of upper mantle peridotites along continental edge: J.Geophys. Res., v75, p1212-1222."@en ;
  rdfs:label "obduction"@en ;
  rdfs:subClassOf gsog:Deformation ;
  rdfs:subClassOf gspr:Tectonic_Process ;
.
gspr:Organic_Accumulation
  a owl:Class ;
  rdfs:comment "Sediment accumulation of biologically produced organic material, as in bog, coal swamps."@en ;
  rdfs:label "organic accumulation"@en ;
  rdfs:subClassOf gspr:Deposition ;
.
gspr:Oxidation
  a owl:Class ;
  rdfs:comment "Chemical reaction that involve stripping of electrons from cations. Typicall reactions include converting sulfide minerals to oxide minerals, or increasing the oxidation state of cations in existing oxide minerals. The most commonly observed is the oxidation of Fe"@en ;
  rdfs:comment "dct:source--  this vocabulary"@en ;
  rdfs:label "oxidation"@en ;
  rdfs:subClassOf gspr:Chemical_Weathering ;
.
gspr:Partial_Melting
  a owl:Class ;
  rdfs:comment "Process of melting involving only some of the mineral phases in a rock, to produce a mixture of melt and residual particles."@en ;
  rdfs:comment "dct:source--  Neuendorf, K.K.E, Mehl, J.P. & Jackson, J.A. (eds), 2005. Glossary of geology, 5th Edition. American Geological Institute, Alexandria, 779 p."@en ;
  rdfs:label "partial melting"@en ;
  rdfs:subClassOf gspr:Melting ;
.
gspr:Physical_Weathering
  a owl:Class ;
  rdfs:comment "The process of weathering by which frost action, salt-crystal growth, absorption of water, and other physical processes break down a rock to fragments, involving no chemical change"@en ;
  rdfs:comment "dct:source--  Neuendorf, K.K.E, Mehl, J.P. & Jackson, J.A. (eds), 2005. Glossary of geology, 5th Edition. American Geological Institute, Alexandria, 779 p."@en ;
  rdfs:label "physical weathering"@en ;
  rdfs:subClassOf gspr:Weathering ;
.
gspr:Plinian_Eruption
  a owl:Class ;
  rdfs:comment "An explosive eruption in which a steady, turbulent stream of fragmented magma and magmatic gas is released at a high velocity from a vent. Large volumes of tephra and tall eruption columns are characteristic"@en ;
  rdfs:comment "dct:source--  Neuendorf, K.K.E, Mehl, J.P. & Jackson, J.A. (eds), 2005. Glossary of geology, 5th Edition. American Geological Institute, Alexandria, 779 p."@en ;
  rdfs:label "plinian eruption"@en ;
  rdfs:subClassOf gspr:Pyroclastic_Eruption ;
.
gspr:Polar_Wander
  a owl:Class ;
  rdfs:comment "Process of migration of the axis of the earth's dipole field relative to the rotation axis of the Earth."@en ;
  rdfs:comment "dct:source--  this vocabulary"@en ;
  rdfs:label "polar wander"@en ;
  rdfs:subClassOf gsog:Transformation ;
  rdfs:subClassOf gspr:Geomagnetic_Process ;
.
gspr:Pressure_Release_Weathering
  a owl:Class ;
  rdfs:comment "Propagation of fractures near the surface of solid rock due to expansion related to release of confining pressure when deeply buried rock is unroofed. Fractures typically propagate along surfaces close to and subparallel to the surface of the outcrop."@en ;
  rdfs:comment "dct:source--  Neuendorf, K.K.E, Mehl, J.P. & Jackson, J.A. (eds), 2005. Glossary of geology, 5th Edition. American Geological Institute, Alexandria, 779 p."@en ;
  rdfs:label "pressure release weathering"@en ;
  rdfs:subClassOf gspr:Physical_Weathering ;
.
gspr:Pyroclastic_Eruption
  a owl:Class ;
  rdfs:comment "Eruption produced by the generation and rapid expansion of a gas phase that disrupts magma, surrounding wall rock or sediment"@en ;
  rdfs:comment "dct:source--  Orton, G.J., 1996. Volcanic environments. 485-567 in Readingh.G. (ed.), Sedimentary Environments: Processes, Facies and Stratigraphy, Third Edition. Blackwell Science, Oxford"@en ;
  rdfs:label "pyroclastic eruption"@en ;
  rdfs:subClassOf gspr:Eruption ;
.
gspr:Pyrometamorphism
  a owl:Class ;
  rdfs:comment "metamorphism caused by high-temperature near surface events like lightning strikes,  underground coal fires or nuclear reactions."@en ;
  rdfs:label "Pyrometamorphism "@en ;
  rdfs:subClassOf gspr:Metamorphic_Process ;
.
gspr:Regional_Metamorphism
  a owl:Class ;
  rdfs:comment "Metamorphic processes driven by temperature and pressure changes affecting a large rock volume, associated with large-scale tectonic processes."@en ;
  rdfs:comment "dct:source--  based on Smulikowski et al, 2003"@en ;
  rdfs:label "regional metamorphic genesis"@en ;
  rdfs:subClassOf gspr:Metamorphic_Process ;
.
gspr:Rifting
  a owl:Class ;
  rdfs:comment "Extension of the crust to form one or more long, narrow graben of regional extent."@en ;
  rdfs:comment "dct:source--  Neuendorf, K.K.E, Mehl, J.P. & Jackson, J.A. (eds), 2005. Glossary of geology, 5th Edition. American Geological Institute, Alexandria, 779 p."@en ;
  rdfs:label "rifting"@en ;
  rdfs:subClassOf gspr:Continental_Breakup ;
.
gspr:Rock_Forming_Process
  a owl:Class ;
  rdfs:comment "A process that produces a new igneous or sedimentary rock material. " ;
  rdfs:label "Rock forming process "@en ;
  rdfs:subClassOf gsog:Geologic_Process ;
.
gspr:Sea_Level_Fluctuation
  a owl:Class ;
  rdfs:comment "process of alteration of global sea levels due to changes in either the volume of water in the world's oceans or net changes in the volume of the oceanic basins."@en ;
  rdfs:label "Sea Level Fluctuation"@en ;
  rdfs:subClassOf gsog:Geologic_Process ;
.
gspr:Sedimentary_Process
  a owl:Class ;
  rdfs:comment "A process that changes the distribution or physical properties of sediment at or near the earth's surface"@en ;
  rdfs:comment "dct:source--  this vocabulary"@en ;
  rdfs:label "Sedimentary Process"@en ;
  rdfs:subClassOf gsog:Geologic_Process ;
.
gspr:Shearing
  a owl:Class ;
  rdfs:comment "A deformation in which contiguous parts of a body are displaced relatively to each other in a direction parallel to a surface. The surface may be a discrete fault, or the deformation may be a penetrative strain and the shear surface is a geometric abstraction."@en ;
  rdfs:comment "dct:source--  Neuendorf, K.K.E, Mehl, J.P. & Jackson, J.A. (eds), 2005. Glossary of geology, 5th Edition. American Geological Institute, Alexandria, 779 p."@en ;
  rdfs:label "shearing"@en ;
  rdfs:subClassOf gsog:Deformation ;
.
gspr:Speciation
  a owl:Class ;
  rdfs:comment "dct:source--  this vocabulary"@en ;
  rdfs:comment "process that results inappearance of new species"@en ;
  rdfs:label "speciation"@en ;
  rdfs:subClassOf gspr:Biological_Process ;
.
gspr:Spreading
  a owl:Class ;
  rdfs:comment "A process whereby new oceanic crust is formed by upwelling of magma at the center of mid-ocean ridges and by a moving-away of the new material from the site of upwelling at rates of one to ten centimeters per year."@en ;
  rdfs:comment "dct:source--  Neuendorf, K.K.E, Mehl, J.P. & Jackson, J.A. (eds), 2005. Glossary of geology, 5th Edition. American Geological Institute, Alexandria, 779 p."@en ;
  rdfs:label "spreading"@en ;
  rdfs:subClassOf gsog:Additive_Process ;
  rdfs:subClassOf gsog:Deformation ;
  rdfs:subClassOf gspr:Tectonic_Process ;
.
gspr:Strombolian_Eruption
  a owl:Class ;
  rdfs:comment "Eruption characterized by jetting of clots or \\fountains\\ of fluid, basaltic lava from a central crater"@en ;
  rdfs:comment "dct:source--  Neuendorf, K.K.E, Mehl, J.P. & Jackson, J.A. (eds), 2005. Glossary of geology, 5th Edition. American Geological Institute, Alexandria, 779 p."@en ;
  rdfs:label "strombolian eruption"@en ;
  rdfs:subClassOf gspr:Eruption ;
.
gspr:Subaerial_Extrusion
  a owl:Class ;
  rdfs:comment "Process of magma crystallisation either in the open air or immediately adjacent to the land surface."@en ;
  rdfs:comment "dct:source--  This vocabulary"@en ;
  rdfs:label "subaerial extrusion"@en ;
  rdfs:subClassOf gspr:Eruption ;
.
gspr:Subaqueous_Extrusion
  a owl:Class ;
  rdfs:comment "Process of magma crystallisation under water or ice."@en ;
  rdfs:comment "dct:source--  This vocabulary"@en ;
  rdfs:label "subaqueous extrusion"@en ;
  rdfs:subClassOf gspr:Eruption ;
.
gspr:Subduction
  a owl:Class ;
  rdfs:comment "The process of one lithospheric plate descending beneath another"@en ;
  rdfs:comment "dct:source--  Neuendorf, K.K.E, Mehl, J.P. & Jackson, J.A. (eds), 2005. Glossary of geology, 5th Edition. American Geological Institute, Alexandria, 779 p."@en ;
  rdfs:label "subduction"@en ;
  rdfs:subClassOf gsog:Deformation ;
  rdfs:subClassOf gsog:Subtractive_Process ;
  rdfs:subClassOf gspr:Tectonic_Process ;
.
gspr:Tectonic_Process
  a owl:Class ;
  rdfs:comment "Processes related to the interaction between or deformation of rigid plates forming the crust of the Earth."@en ;
  rdfs:comment "dct:source--  this vocabulary"@en ;
  rdfs:label "Tectonic Process"@en ;
  rdfs:subClassOf gsog:Geologic_Process ;
.
gspr:Thermal_Shock_Weathering
  a owl:Class ;
  rdfs:comment "Propagation of fractures near the surface of solid rock due to expansion and contraction caused by temperature changes. Fractures typically propagate along surfaces close to and subparallel to the surface of the outcrop."@en ;
  rdfs:comment "dct:source--  this vocabulary"@en ;
  rdfs:label "thermal shock weathering"@en ;
  rdfs:subClassOf gspr:Physical_Weathering ;
.
gspr:Traction_Saltation_or_Suspension_Deposition
  a owl:Class ;
  rdfs:comment "Deposition of sediment from moving water or air, in which the sediment is transported by entrainment in the moving fluid. Constrast with debris flow or turbidity current deposition in which movement of fluid/sediment mixture is due to incorporation of sediment in fluid."@en ;
  rdfs:comment "dct:source--  this vocabulary"@en ;
  rdfs:label "deposition from moving fluid"@en ;
  rdfs:subClassOf gspr:Mechanical_Deposition ;
.
gspr:Transform_Faulting
  a owl:Class ;
  rdfs:comment "A strike-slip fault that links two other faults or two other plate boundaries (e.g. two segments of a mid-ocean ridge). Transform faults often exhibit characteristics that distinguish them from transcurrent faults: (1) For transform faults formed at the same time as the faults they link, slip on the transform fault has equal magnitude at all points along the transform, slip magnitude on the transform fault can exceed the length of the transform fault, and slip does not decrease to zero at the fault termini. (2) For transform faults linking two similar features, e.g. if two mid-ocean ridge segments linked by a transform have equal spreading rates, then the length of the transform does not change as slip accrues on it."@en ;
  rdfs:comment "dct:source--  Neuendorf, K.K.E, Mehl, J.P. & Jackson, J.A. (eds), 2005. Glossary of geology, 5th Edition. American Geological Institute, Alexandria, 779 p."@en ;
  rdfs:label "transform faulting"@en ;
  rdfs:subClassOf gspr:Faulting ;
  rdfs:subClassOf gspr:Tectonic_Process ;
.
gspr:Turbidity_Current_Deposition
  a owl:Class ;
  rdfs:comment "Deposition from a turbulent, low concentration sediment-water mixture."@en ;
  rdfs:comment "dct:source--  Postma 1986 Geology v. 14 p291-294"@en ;
  rdfs:label "turbidity current deposition"@en ;
  rdfs:subClassOf gspr:Mechanical_Deposition ;
.
gspr:Vulcanian_Eruption
  a owl:Class ;
  rdfs:comment "Eruption characterized by the explosive ejection of fragments of new lava, commonly incandescent when they leave the vent but either solid or too viscous to assume any appreciable degree of rounding during their flight through the air. With these there are often breadcrust bombs or blocks, and generally large proportions of ash"@en ;
  rdfs:comment "dct:source--  Neuendorf, K.K.E, Mehl, J.P. & Jackson, J.A. (eds), 2005. Glossary of geology, 5th Edition. American Geological Institute, Alexandria, 779 p."@en ;
  rdfs:label "vulcanian eruption"@en ;
  rdfs:subClassOf gspr:Pyroclastic_Eruption ;
.
gspr:Water_Erosion
  a owl:Class ;
  rdfs:comment "Erosion by clast impact or plucking by moving liquid water"@en ;
  rdfs:comment "dct:source--  this vocabulary"@en ;
  rdfs:label "water erosion"@en ;
  rdfs:subClassOf gspr:Erosion ;
.
gspr:Weathering
  a owl:Class ;
  rdfs:comment "The process or group of processes by which earth materials exposed to atmospheric agents at or near the Earth's surface are changed in color, texture, composition, firmness, or form, with little or no transport of the loosened or altered material. Processes typically include oxidationhydration, and leaching of soluble constituents."@en ;
  rdfs:comment "dct:source--  this vocabulary"@en ;
  rdfs:label "weathering"@en ;
  rdfs:subClassOf gsog:Transformation ;
.
gspr:Wind_Erosion
  a owl:Class ;
  rdfs:comment "Erosion by clast impact or plucking by moving air (wind)"@en ;
  rdfs:comment "dct:source--  this vocabulary"@en ;
  rdfs:label "wind erosion"@en ;
  rdfs:subClassOf gspr:Erosion ;
.
gspr:ontology
  a owl:Ontology ;
  rdfs:comment "This file contains terms and definitions from the 2016 SKOS-RDF version of the CGI Event Process vocabulary."@en ;
  rdfs:comment "This scheme specifies concepts used to describe the geological processes that are associated with geological events, as defined by the IUGS Commission for Geoscience Information (CGI) Geoscience Terminology Working Group."@en ;
  rdfs:comment "dct:creator--  CGI Geoscience Terminology Working Group, OWL adaptation by Stephen Richard for Loop3D project"@en ;
  rdfs:comment "dct:date--  2016-06-15"@en ;
  rdfs:comment "dct:modified-- 2019-12-04"@en ;
  rdfs:label "Geologic processes"@en ;
.
