# baseURI: http://loop3d.org/GSO/ontology/2020/1/geologicstructure/fault/ontology

@prefix gsfa: <http://loop3d.org/GSO/ontology/2020/1/geologicstructure/fault/> .
@prefix gsfms: <http://loop3d.org/GSO/ontology/2020/1/geologicstructure/fault/movementsense/> .
@prefix gsfmt: <http://loop3d.org/GSO/ontology/2020/1/geologicstructure/fault/movementtype/> .
@prefix gsgu: <http://loop3d.org/GSO/ontology/2020/1/geologicunit/> .
@prefix gsoc: <http://loop3d.org/GSO/ontology/2020/1/common/> .
@prefix gsog: <http://loop3d.org/GSO/ontology/2020/1/geologicfeature/> .
@prefix gsoq: <http://loop3d.org/GSO/ontology/2020/1/geologicquality/>  .
@prefix owl: <http://www.w3.org/2002/07/owl#> .
@prefix rdf: <http://www.w3.org/1999/02/22-rdf-syntax-ns#> .
@prefix rdfs: <http://www.w3.org/2000/01/rdf-schema#> .
@prefix xml: <http://www.w3.org/XML/1998/namespace> .
@prefix xsd: <http://www.w3.org/2001/XMLSchema#> .

gsog:Fault_Zone
  a owl:Class ;
  rdfs:subClassOf [
      a owl:Restriction ;
      owl:onProperty gsoc:hasPart ;
      owl:someValuesFrom gsog:Fault ;
    ] ;
  rdfs:subClassOf [
      a owl:Restriction ;
      owl:onProperty gsoc:hasQuality ;
      owl:someValuesFrom gsoq:Thickness ;
    ] ;
  rdfs:subClassOf [
      a owl:Restriction ;
      owl:onProperty gsoc:isColocatedWith ;
      owl:someValuesFrom gsgu:deformation_unit ;
    ] ;
  rdfs:subClassOf [
      a owl:Restriction ;
      owl:onProperty gsoc:isParticipantIn ;
      owl:someValuesFrom gsog:Deformation ;
    ] ;
.
gsfa:Fault_Movement_Magnitude
  a owl:Class ;
  rdfs:comment "magnitude of slip or separation"@en ;
  rdfs:label "Displacement magnitude"@en ;
  rdfs:subClassOf gsoc:Quality ;
  rdfs:subClassOf [
      a owl:Restriction ;
      owl:allValuesFrom gsog:Displacement ;
      owl:onProperty gsoc:isQualityOf ;
    ] ;
  rdfs:subClassOf [
      a owl:Restriction ;
      owl:onProperty gsoc:hasDataValue ;
      owl:someValuesFrom xsd:decimal ;
    ] ;
  rdfs:subClassOf [
      a owl:Restriction ;
      owl:onProperty gsoc:hasUOM ;
      owl:someValuesFrom gsoc:Unit_of_Measure ;
    ] ;
.
gsfa:Fault_Movement_Sense
  a owl:Class ;
  rdfs:comment "eg, dextral, sinistral"@en ;
  rdfs:label "Movement sense"@en ;
  rdfs:subClassOf gsoc:Quality ;
  rdfs:subClassOf [
      a owl:Restriction ;
      owl:allValuesFrom [
          a owl:Class ;
          owl:unionOf (
              gsog:Displacement
              gsog:Fault
            ) ;
        ] ;
      owl:onProperty gsoc:isQualityOf ;
    ] ;
.
gsfa:Fault_Movement_Type
  a owl:Class ;
  rdfs:comment "Defines the type of movement  (eg dip-slip, strike-slip)"@en ;
  rdfs:label "Movement Type"@en ;
  rdfs:subClassOf gsoc:Quality ;
  rdfs:subClassOf [
      a owl:Restriction ;
      owl:allValuesFrom [
          a owl:Class ;
          owl:unionOf (
              gsog:Displacement
              gsog:Fault
            ) ;
        ] ;
      owl:onProperty gsoc:isQualityOf ;
    ] ;
.
gsfa:Fault_Movement_Vector
  a owl:Class ;
  rdfs:comment "Slip vector linking piercing point on opposite sides of fault, or separation vector linking offset surface along fault trace."@en ;
  rdfs:label "Movement Vector"@en ;
  rdfs:subClassOf gsoc:Quality ;
  rdfs:subClassOf [
      a owl:Restriction ;
      owl:allValuesFrom gsog:Displacement ;
      owl:onProperty gsoc:isQualityOf ;
    ] ;
  rdfs:subClassOf [
      a owl:Restriction ;
      owl:onProperty gsoc:hasQuality ;
      owl:someValuesFrom gsoq:Azimuth ;
    ] ;
  rdfs:subClassOf [
      a owl:Restriction ;
      owl:onProperty gsoc:hasQuality ;
      owl:someValuesFrom gsoq:Plunge ;
    ] ;
.
gsfa:detachment_fault
  a owl:Class ;
  rdfs:comment "A regional-scale, large displacement, low-angle normal fault."@en ;
  rdfs:comment "dct:source--  CGI faulttype SKOS vocabulary 2016-10-19"@en ;
  rdfs:label "detachment fault"@en ;
  rdfs:subClassOf gsfa:low_angle_normal_fault ;
.
gsfa:dextral_strike_slip_fault
  a owl:Class ;
  rdfs:comment "Fault with right-lateral strike-parallel displacement component of slip vector more than 10 times the dip-parallel component of the slip vector at at least one location along the fault, and right-lateral displacement over more than half the mapped trace of the fault."@en ;
  rdfs:comment "dct:source--  CGI faulttype SKOS vocabulary 2016-10-19"@en ;
  rdfs:label "dextral strike slip fault"@en ;
  rdfs:subClassOf gsfa:strike_slip_fault ;
.
gsfa:extraction_fault
  a owl:Class ;
  rdfs:comment "A fault whose two sides have approached each other substantially in the direction perpendicular to the fault."@en ;
  rdfs:comment "dct:source--  Froitzheim, N., Pleuger, J. & Nagel, T.J., 2006. Extraction faults. Journal of Structural Geology v28, pp. 1388-1395."@en ;
  rdfs:label "extraction fault"@en ;
  rdfs:subClassOf gsog:Fault ;
.
gsfa:high_angle_fault
  a owl:Class ;
  rdfs:comment "Fault that dips at least 45 degrees over more than half of its recognized extent, for which slip or separation is not explicitly specified."@en ;
  rdfs:comment "dct:source--  CGI faulttype SKOS vocabulary 2016-10-19"@en ;
  rdfs:label "high angle fault"@en ;
  rdfs:subClassOf gsog:Fault ;
.
gsfa:high_angle_normal_fault
  a owl:Class ;
  rdfs:comment "Fault that dips at least 45 degrees over more than half of the recognized extent of the fault with the hanging wall displaced from a structurally higher position relative to footwall rocks."@en ;
  rdfs:comment "dct:source--  CGI faulttype SKOS vocabulary 2016-10-19"@en ;
  rdfs:label "high angle normal fault"@en ;
  rdfs:subClassOf gsfa:high_angle_fault ;
  rdfs:subClassOf gsfa:normal_fault ;
.
gsfa:high_angle_reverse
  a owl:Class ;
  rdfs:comment "Reverse fault that dips at least 45 degrees over more than half of its recognized extent, for which slip or separation is not explicitly specified."@en ;
  rdfs:comment "dct:source--  CGI faulttype SKOS vocabulary 2016-10-19"@en ;
  rdfs:label "high angle reverse"@en ;
  rdfs:subClassOf gsfa:high_angle_fault ;
  rdfs:subClassOf gsfa:reverse_fault ;
.
gsfa:horizontal_fault
  a owl:Class ;
  rdfs:comment "Fault that dips less than 10 degrees over more than half the recognized extent of the fault."@en ;
  rdfs:comment "dct:source--  GGIC vocabularies working group (Australia)"@en ;
  rdfs:label "horizontal fault"@en ;
  rdfs:subClassOf gsfa:low_angle_fault ;
.
gsfa:left_normal_fault
  a owl:Class ;
  rdfs:comment "High angle fault with slip vector that has ratio of strike-parallel to dip-parallel displacement between 10 to 1 and 1 to 10 at at least one location along the mapped trace, with left-lateral strike-parallel component and normal dip-parallel component over at least half the mapped trace of the fault."@en ;
  rdfs:comment "dct:source--  CGI faulttype SKOS vocabulary 2016-10-19"@en ;
  rdfs:label "left normal fault"@en ;
  rdfs:subClassOf gsfa:oblique_slip_fault ;
.
gsfa:left_reverse_fault
  a owl:Class ;
  rdfs:comment "High angle fault with slip vector that has ratio of strike-parallel to dip-parallel displacement between 10 to 1 and 1 to 10 at at least one location along the mapped trace, with left-lateral strike-parallel component and reverse dip-parallel component over at least half the mapped trace of the fault."@en ;
  rdfs:comment "dct:source--  CGI faulttype SKOS vocabulary 2016-10-19"@en ;
  rdfs:label "left reverse fault"@en ;
  rdfs:subClassOf gsfa:oblique_slip_fault ;
.
gsfa:low_angle_fault
  a owl:Class ;
  rdfs:comment "Fault that dips less than 45 degrees over more than half of the recognized extent of the fault."@en ;
  rdfs:comment "dct:source--  CGI faulttype SKOS vocabulary 2016-10-19"@en ;
  rdfs:label "low angle fault"@en ;
  rdfs:subClassOf gsog:Fault ;
.
gsfa:low_angle_normal_fault
  a owl:Class ;
  rdfs:comment "Fault that dips less than 45 degrees over more than half of the recognized extent of the fault with the hanging wall displaced from a structurally higher position relative to footwall rocks."@en ;
  rdfs:comment "dct:source--  CGI faulttype SKOS vocabulary 2016-10-19"@en ;
  rdfs:label "low angle normal fault"@en ;
  rdfs:subClassOf gsfa:low_angle_fault ;
  rdfs:subClassOf gsfa:normal_fault ;
.
gsfa:mixed_extraction_fault
  a owl:Class ;
  rdfs:comment "An extraction fault with some displacement within the fault plane."@en ;
  rdfs:comment "dct:source--  Froitzheim, N., Pleuger, J. & Nagel, T.J., 2006. Extraction faults. Journal of Structural Geology v28, pp. 1388-1395."@en ;
  rdfs:label "mixed extraction fault"@en ;
  rdfs:subClassOf gsfa:extraction_fault ;
.
gsfms:detachment
  a owl:Class ;
  rdfs:comment "A regional-scale low-angle normal fault."@en ;
  rdfs:comment "dct:source--  GGIC vocabularies working group (Australia)"@en ;
  rdfs:label "detachment"@en ;
  rdfs:label "d√©tachement"@fr ;
  rdfs:subClassOf gsfms:normal ;
.
gsfms:dextral
  a owl:Class ;
  rdfs:comment "Right-lateral separation sense, in plan view, the side opposite the observer appears displaced to the right.,"@en ;
  rdfs:comment "dct:source--  GGIC vocabularies working group (Australia)"@en ;
  rdfs:label "dextral"@en ;
  rdfs:label "dextre"@fr ;
  rdfs:subClassOf gsfa:Fault_Movement_Sense ;
.
gsfms:generic_decollement
  a owl:Class ;
  rdfs:comment "A large-displacement (kilometers or tens of kilometers) shallowly dipping to subhorizontal fault or shear zone."@en ;
  rdfs:comment "dct:source--  Neuendorf et al. 2005"@en ;
  rdfs:label "decollement"@fr ;
  rdfs:label "generic decollement"@en ;
  rdfs:subClassOf gsfa:Fault_Movement_Sense ;
.
gsfms:no_movement_sense
  a owl:Class ;
  rdfs:comment "The fault-parallel displacement is effectively zero, as in an extraction fault."@en ;
  rdfs:comment "dct:source--  Froitzheim, N., Pleuger, J. & Nagel, T.J., 2006. Extraction faults. Journal of Structural Geology v28, pp. 1388-1395."@en ;
  rdfs:label "no movement sense"@en ;
  rdfs:subClassOf gsfa:Fault_Movement_Sense ;
.
gsfms:normal
  a owl:Class ;
  rdfs:comment "The hanging wall appears to have moved down relative to the footwall, dip of fault usually 45-90 degrees."@en ;
  rdfs:comment "dct:source--  GGIC vocabularies working group (Australia)"@en ;
  rdfs:label "normal"@en ;
  rdfs:subClassOf gsfa:Fault_Movement_Sense ;
.
gsfms:normal_dextral
  a owl:Class ;
  rdfs:comment "The movement sense includes both normal and dextral components."@en ;
  rdfs:comment "dct:source--  GGIC vocabularies working group (Australia)"@en ;
  rdfs:label "normal dextral"@en ;
  rdfs:subClassOf gsfms:dextral ;
  rdfs:subClassOf gsfms:normal ;
.
gsfms:normal_sinistral
  a owl:Class ;
  rdfs:comment "The movement sense includes both normal and sinistral components."@en ;
  rdfs:comment "dct:source--  GGIC vocabularies working group (Australia)"@en ;
  rdfs:label "normal sinistral"@en ;
  rdfs:subClassOf gsfms:normal ;
  rdfs:subClassOf gsfms:sinistral ;
.
gsfms:reverse
  a owl:Class ;
  rdfs:comment "The hanging wall appears to have moved down relative to the footwall, dip of fault usually greater than 45 degrees."@en ;
  rdfs:comment "dct:source--  GGIC vocabularies working group (Australia)"@en ;
  rdfs:label "inverse"@fr ;
  rdfs:label "reverse"@en ;
  rdfs:subClassOf gsfa:Fault_Movement_Sense ;
.
gsfms:reverse_dextral
  a owl:Class ;
  rdfs:comment "The movement sense includes both reverse and dextral components."@en ;
  rdfs:comment "dct:source--  GGIC vocabularies working group (Australia)"@en ;
  rdfs:label "reverse dextral"@en ;
  rdfs:subClassOf gsfms:dextral ;
  rdfs:subClassOf gsfms:reverse ;
.
gsfms:reverse_sinistral
  a owl:Class ;
  rdfs:comment "The movement sense includes both reverse and sinistral components."@en ;
  rdfs:comment "dct:source--  GGIC vocabularies working group (Australia)"@en ;
  rdfs:label "reverse sinistral"@en ;
  rdfs:subClassOf gsfms:reverse ;
  rdfs:subClassOf gsfms:sinistral ;
.
gsfms:sinistral
  a owl:Class ;
  rdfs:comment "Left-lateral separation sense, in plan view, the side opposite the observer appears displaced to the left."@en ;
  rdfs:comment "dct:source--  GGIC vocabularies working group (Australia)"@en ;
  rdfs:label "sinistral"@en ;
  rdfs:subClassOf gsfa:Fault_Movement_Sense ;
.
gsfms:thrust
  a owl:Class ;
  rdfs:comment "Reverse fault with dip typically less than 45 degrees, horizontal compression, rather than vertical displacement is characteristic."@en ;
  rdfs:comment "dct:source--  GGIC vocabularies working group (Australia)"@en ;
  rdfs:label "d√©crochement"@fr ;
  rdfs:label "thrust"@en ;
  rdfs:subClassOf gsfms:reverse ;
.
gsfms:thrust_decollement
  a owl:Class ;
  rdfs:comment "A regional-scale low-angle thrust fault."@en ;
  rdfs:comment "dct:source--  GeoScience Victoria and others"@en ;
  rdfs:label "thrust decollement"@en ;
  rdfs:subClassOf gsfms:thrust ;
.
gsfmt:dip_separation_sense
  a owl:Class ;
  rdfs:comment "A fault along which there is some separation parallel to the dip of the fault."@en ;
  rdfs:comment "dct:source--  GGIC vocabularies working group (Australia)"@en ;
  rdfs:label "dip separation sense"@en ;
  rdfs:subClassOf gsfa:Fault_Movement_Type ;
.
gsfmt:dip_slip
  a owl:Class ;
  rdfs:comment "The net slip of the fault lies in the dip direction of the fault."@en ;
  rdfs:comment "dct:source--  GGIC vocabularies working group (Australia)"@en ;
  rdfs:label "dip slip"@en ;
  rdfs:subClassOf gsfmt:dip_separation_sense ;
.
gsfmt:extraction
  a owl:Class ;
  rdfs:comment "A fault whose two sides have approached each other substantially in the direction perpendicular to the fault."@en ;
  rdfs:comment "dct:source--  Froitzheim, N., Pleuger, J. & Nagel, T.J., 2006. Extraction faults. Journal of Structural Geology v28, pp. 1388-1395."@en ;
  rdfs:label "extraction"@en ;
  rdfs:subClassOf gsfa:Fault_Movement_Type ;
.
gsfmt:horizontal
  a owl:Class ;
  rdfs:comment "The fault is horizontal."@en ;
  rdfs:comment "dct:source--  GGIC vocabularies working group (Australia)"@en ;
  rdfs:label "horizontal"@en ;
  rdfs:subClassOf gsfa:Fault_Movement_Type ;
.
gsfmt:mixed_extraction
  a owl:Class ;
  rdfs:comment "An extraction fault with some displacement within the fault plane."@en ;
  rdfs:comment "dct:source--  Froitzheim, N., Pleuger, J. & Nagel, T.J., 2006. Extraction faults. Journal of Structural Geology v28, pp. 1388-1395."@en ;
  rdfs:label "mixed extraction"@en ;
  rdfs:subClassOf gsfmt:extraction ;
.
gsfmt:oblique_slip
  a owl:Class ;
  rdfs:comment "The net slip of the fault lies between the strike and dip directions of the fault, the slip vector rakes between 10 and 80 degrees in the plane of the fault."@en ;
  rdfs:comment "dct:source--  GGIC vocabularies working group (Australia), SMR"@en ;
  rdfs:label "oblique slip"@en ;
  rdfs:subClassOf gsfa:Fault_Movement_Type ;
.
gsfmt:pure_extraction
  a owl:Class ;
  rdfs:comment "An extraction fault with no discernible displacement within the fault plane."@en ;
  rdfs:comment "dct:source--  Froitzheim, N., Pleuger, J. & Nagel, T.J., 2006. Extraction faults. Journal of Structural Geology v28, pp. 1388-1395."@en ;
  rdfs:label "pure extraction"@en ;
  rdfs:subClassOf gsfmt:extraction ;
.
gsfmt:scissor
  a owl:Class ;
  rdfs:comment "A fault on which there is increasing offset or separation along the strike from an initial point of no offset, with reverse offset in the opposite direction."@en ;
  rdfs:comment "dct:source--  Neuendorf et al 2005"@en ;
  rdfs:label "scissor"@en ;
  rdfs:subClassOf gsfa:Fault_Movement_Type ;
.
gsfmt:strike_separation_sense
  a owl:Class ;
  rdfs:comment "A fault along which there is some separation parallel to the strike of the fault."@en ;
  rdfs:comment "dct:source--  GGIC vocabularies working group (Australia)"@en ;
  rdfs:label "strike separation sense"@en ;
  rdfs:subClassOf gsfa:Fault_Movement_Type ;
.
gsfmt:strike_slip
  a owl:Class ;
  rdfs:comment "The net slip of the fault (slip vector) is parallel to the strike of the fault."@en ;
  rdfs:comment "dct:source--  GGIC vocabularies working group (Australia), this vocabulary"@en ;
  rdfs:label "strike slip"@en ;
  rdfs:subClassOf gsfmt:strike_separation_sense ;
.
gsfmt:transcurrent
  a owl:Class ;
  rdfs:comment "A large scale strike-slip fault in which the fault surface is steeply inclined."@en ;
  rdfs:comment "dct:source--  GGIC vocabularies working group (Australia)"@en ;
  rdfs:label "transcurrent"@en ;
  rdfs:subClassOf gsfmt:strike_slip ;
.
gsfmt:transform
  a owl:Class ;
  rdfs:comment "A variety of strike-slip fault along which the displacement suddenly stops or changes form, typically associated with mid-ocean ridges."@en ;
  rdfs:comment "dct:source--  GGIC vocabularies working group (Australia)"@en ;
  rdfs:label "transform"@en ;
  rdfs:subClassOf gsfmt:strike_slip ;
.
gsfmt:transpressional
  a owl:Class ;
  rdfs:comment "A fault along which strike-slip deformation is accompanied by a component of shortening transverse to the fault."@en ;
  rdfs:comment "dct:source--  GGIC vocabularies working group (Australia)"@en ;
  rdfs:label "transpressional"@en ;
  rdfs:subClassOf gsfmt:oblique_slip ;
.
gsfmt:transtensional
  a owl:Class ;
  rdfs:comment "A fault along which strike-slip deformation is accompanied by a component of extension transverse to the fault."@en ;
  rdfs:comment "dct:source--  GGIC vocabularies working group (Australia)"@en ;
  rdfs:label "transtensional"@en ;
  rdfs:subClassOf gsfmt:oblique_slip ;
.
gsfmt:wrench
  a owl:Class ;
  rdfs:comment "A strike slip fault in which the faut plane is more or less vertical."@en ;
  rdfs:comment "dct:source--  GGIC vocabularies working group (Australia)"@en ;
  rdfs:label "wrench"@en ;
  rdfs:subClassOf gsfmt:strike_slip ;
.
gsfa:normal_fault
  a owl:Class ;
  rdfs:comment "Fault with dip-parallel displacement component of slip vector more than 10 times the strike-parallel component of the slip vector over more than half recognized extent of the fault, and for which the fault dips consistently in the same direction, and for which the hanging wall has been displaced down relative to the footwall."@en ;
  rdfs:comment "dct:source--  CGI faulttype SKOS vocabulary 2016-10-19"@en ;
  rdfs:label "normal fault"@en ;
  rdfs:subClassOf gsog:Fault ;
.
gsfa:oblique_slip_fault
  a owl:Class ;
  rdfs:comment "Fault with slip vector that has ratio of strike-parallel to dip-parallel displacement between 10 to 1 and 1 to 10 at at least one location along the mapped trace of the fault."@en ;
  rdfs:comment "dct:source--  CGI faulttype SKOS vocabulary 2016-10-19"@en ;
  rdfs:label "oblique slip fault"@en ;
  rdfs:subClassOf gsog:Fault ;
.
gsfa:ontology
  a owl:Ontology ;
  rdfs:comment "This file contains the 2016 SKOS-RDF version of the CGI Fault Type, Fault Movement Sense and Fault Movement Type vocabulary. Compilation and review in MS Excel spreadsheet, converted to MS Excel for SKOS generation using SKOS_for_GA_from_XLS_2016.03.xslt"@en ;
  rdfs:comment "This ontology includes extensions for describing faults in more detail. (ie, a summary of movement type and orientation) as defined by the IUGS Commission for Geoscience Information (CGI) Geoscience Terminology Working Group. Although the terms in this vocabulary are in common usage with definitions in standard texts or glossaries like Neuendorf et al. (2005), the definitions here attempt to establish unambiguous criteria to distinguish the categories, and are thus listed with this vocabulary as the source."@en ;
  rdfs:comment "dct:creator--  CGI Geoscience Terminology Working Group; OWL conversion by Stephen Richard for Loop3D project"@en ;
  rdfs:comment "dct:date--  2016-10-19"@en ;
  rdfs:comment "dct:modified-- 2020-01-29"@en ;
  rdfs:label "Fault Type"@en ;
.
gsfa:pure_extraction_fault
  a owl:Class ;
  rdfs:comment "An extraction fault with no discernible displacement within the fault plane."@en ;
  rdfs:comment "dct:source--  Froitzheim, N., Pleuger, J. & Nagel, T.J., 2006. Extraction faults. Journal of Structural Geology v28, pp. 1388-1395."@en ;
  rdfs:label "pure extraction fault"@en ;
  rdfs:subClassOf gsfa:extraction_fault ;
.
gsfa:reverse_fault
  a owl:Class ;
  rdfs:comment "Fault with dip-parallel displacement component of slip vector more than 10 times the strike-parallel component of the slip vector at at least one location along the mapped trace of the fault, and the fault dips consistently in the same direction with the hanging wall displaced up relative to the footwall over at least half the mapped trace of the fault."@en ;
  rdfs:comment "dct:source--  CGI faulttype SKOS vocabulary 2016-10-19"@en ;
  rdfs:label "reverse fault"@en ;
  rdfs:subClassOf gsog:Fault ;
.
gsfa:right_normal_fault
  a owl:Class ;
  rdfs:comment "High angle fault with slip vector that has ratio of strike-parallel to dip-parallel displacement between 10 to 1 and 1 to 10 at at least one location along the mapped trace, with right-lateral strike-parallel component and normal dip-parallel component of slip over at least half the mapped trace of the fault"@en ;
  rdfs:comment "dct:source--  CGI faulttype SKOS vocabulary 2016-10-19"@en ;
  rdfs:label "right normal fault"@en ;
  rdfs:subClassOf gsfa:oblique_slip_fault ;
.
gsfa:right_reverse_fault
  a owl:Class ;
  rdfs:comment "High angle fault with slip vector that has ratio of strike-parallel to dip-parallel displacement between 10 to 1 and 1 to 10 at at least one location along the mapped trace, with a right-lateral strike-parallel component and reverse dip-parallel component of slip over at least half the mapped trace of the fault."@en ;
  rdfs:comment "dct:source--  CGI faulttype SKOS vocabulary 2016-10-19"@en ;
  rdfs:label "right reverse fault"@en ;
  rdfs:subClassOf gsfa:oblique_slip_fault ;
.
gsfa:scissor_fault
  a owl:Class ;
  rdfs:comment "A fault on which there is increasing offset or separation along the strike from an initial point of no offset, with the opposite sense of offset in the opposite direction."@en ;
  rdfs:comment "dct:source--  Neuendorf et al 2005"@en ;
  rdfs:label "scissor fault"@en ;
  rdfs:subClassOf gsog:Fault ;
.
gsfa:sinistral_strike_slip_fault
  a owl:Class ;
  rdfs:comment "Fault with left-lateral strike-parallel displacement component of slip vector more than 10 times the dip-parallel component of the slip vector at at least one location along the fault, and left-lateral displacement over more than half the mapped trace of the fault."@en ;
  rdfs:comment "dct:source--  CGI faulttype SKOS vocabulary 2016-10-19"@en ;
  rdfs:label "sinistral strike slip fault"@en ;
  rdfs:subClassOf gsfa:strike_slip_fault ;
.
gsfa:strike_slip_fault
  a owl:Class ;
  rdfs:comment "Fault with strike-parallel displacement component of slip vector more than 10 times the dip-parallel component of the slip vector at at least one location along the mapped trace of the fault."@en ;
  rdfs:comment "dct:source--  CGI faulttype SKOS vocabulary 2016-10-19"@en ;
  rdfs:label "strike slip fault"@en ;
  rdfs:subClassOf gsog:Fault ;
.
gsfa:thrust_fault
  a owl:Class ;
  rdfs:comment "Fault that dips less than 45 degrees over more than half of the recognized extent of the fault, with a hanging wall displaced from a structurally deeper position relative to footwall rocks."@en ;
  rdfs:comment "dct:source--  CGI faulttype SKOS vocabulary 2016-10-19"@en ;
  rdfs:label "thrust fault"@en ;
  rdfs:subClassOf gsfa:low_angle_fault ;
  rdfs:subClassOf gsfa:reverse_fault ;
.
gsfa:wrench_fault
  a owl:Class ;
  rdfs:comment "A strike slip fault in which the fault plane dips at least 45 degrees over more than half of the recognized extent of the fault."@en ;
  rdfs:comment "dct:source--  GGIC vocabularies working group (Australia)"@en ;
  rdfs:label "wrench fault"@en ;
  rdfs:subClassOf gsfa:high_angle_fault ;
  rdfs:subClassOf gsfa:strike_slip_fault ;
.
