# baseURI: http://loop3d.org/GSO/ontology/2020/1/lithology/ontology
# imports: http://loop3d.org/GSO/ontology/2020/1/geologicfeature/ontology
# imports: http://loop3d.org/GSO/ontology/2020/1/geologicquality/ontology
# imports: http://loop3d.org/GSO/ontology/2020/1/lithology/compositioncategory/ontology
# imports: http://loop3d.org/GSO/ontology/2020/1/lithology/consolidationdegree/ontology
# imports: http://loop3d.org/GSO/ontology/2020/1/lithology/geneticcategory/ontology
# imports: http://loop3d.org/GSO/ontology/2020/1/lithology/particleaspectratio/ontology
# imports: http://loop3d.org/GSO/ontology/2020/1/lithology/particleroundness/ontology/
# imports: http://loop3d.org/GSO/ontology/2020/1/lithology/particletype/ontology
# imports: http://loop3d.org/GSO/ontology/2020/1/metamorphicfacies/ontology
# imports: http://loop3d.org/GSO/ontology/2020/1/metamorphicgrade/ontology

@prefix : <http://loop3d.org/GSO/ontology/2020/1/lithology/> .
@prefix dcam: <http://purl.org/dc/dcam/> .
@prefix gsar: <http://loop3d.org/GSO/ontology/2020/1/lithology/particleaspectratio/> .
@prefix gscc: <http://loop3d.org/GSO/ontology/2020/1/lithology/compositioncategory/> .
@prefix gsgc: <http://loop3d.org/GSO/ontology/2020/1/lithology/geneticcategory/> .
@prefix gslth: <http://loop3d.org/GSO/ontology/2020/1/lithology/> .
@prefix gsmf: <http://loop3d.org/GSO/ontology/2020/1/metamorphicfacies/> .
@prefix gsmg: <http://loop3d.org/GSO/ontology/2020/1/metamorphicgrade/> .
@prefix gsoc: <http://loop3d.org/GSO/ontology/2020/1/common/> .
@prefix gsog: <http://loop3d.org/GSO/ontology/2020/1/geologicfeature/> .
@prefix gsop: <http://loop3d.org/GSO/ontology/2020/1/geologicquality/> .
@prefix gsps: <http://loop3d.org/GSO/ontology/2020/1/lithology/particleroundness/> .
@prefix gspt: <http://loop3d.org/GSO/ontology/2020/1/lithology/particletype/> .
@prefix owl: <http://www.w3.org/2002/07/owl#> .
@prefix rdf: <http://www.w3.org/1999/02/22-rdf-syntax-ns#> .
@prefix rdfs: <http://www.w3.org/2000/01/rdf-schema#> .
@prefix xml: <http://www.w3.org/XML/1998/namespace> .
@prefix xsd: <http://www.w3.org/2001/XMLSchema#> .

gsoc:Unit_of_Measure
  a owl:Class ;
.
gsog:Granular_Material
  a owl:Class ;
  rdfs:comment "Granular material properties are bound in the Rock_Material module"@en ;
  rdfs:subClassOf [
      a owl:Restriction ;
      owl:onProperty gsoc:hasQuality ;
      owl:someValuesFrom gslth:Grain_Size ;
    ] ;
  rdfs:subClassOf [
      a owl:Restriction ;
      owl:onProperty gsoc:hasQuality ;
      owl:someValuesFrom gslth:Particle_Sorting_Category ;
    ] ;
.
gsog:Rock_Material
  a owl:Class ;
  rdfs:comment "Rock_material properties a bound in the Rock_Material module"@en ;
.
gsop:Alteration_Degree
  a owl:Class ;
.
gsop:Alteration_Distribution
  a owl:Class ;
.
gsop:Alteration_Type
  a owl:Class ;
.
gsop:Metamorphic_Facies
  a owl:Class ;
.
gsop:Metamorphic_Grade
  a owl:Class ;
.
gslth:Consolidation_Degree
  a owl:Class ;
  rdfs:comment "A property that specifies the degree to which an aggregation of EarthMaterial particles is a distinct solid material. Consolidation and induration are related concepts specified by this property. They define a continuum from unconsolidated material to very hard rock. Induration is the degree to which a consolidated material is made hard, operationally determined by how difficult it is to break a piece of the material. Consolidated materials may have varying degrees of induration (NADMSC, 2004)"@en ;
  rdfs:isDefinedBy "GeoSciML v4"@en ;
  rdfs:label "Consolidation degree"@en ;
  rdfs:subClassOf gsoc:Quality ;
  rdfs:subClassOf [
      a owl:Restriction ;
      owl:onProperty gsoc:isQualityOf ;
      owl:someValuesFrom gsog:Rock_Material ;
    ] ;
.
gslth:Grain_Roundness
  a owl:Class ;
  rdfs:label "Grain Shape"@en ;
  rdfs:subClassOf gsoc:Quality ;
  rdfs:subClassOf [
      a owl:Restriction ;
      owl:allValuesFrom gsoc:Shape ;
      owl:onProperty gsoc:isQualityOf ;
    ] ;
.
gslth:Grain_Size
  a owl:Class ;
  rdfs:comment "generaly property for specification of grain size; sub-properties have value spaces for different size specification types."@en ;
  rdfs:label "Grain Size property "@en ;
  rdfs:subClassOf gsoc:Quality ;
  rdfs:subClassOf [
      a owl:Restriction ;
      owl:allValuesFrom [
          a owl:Class ;
          owl:unionOf (
              gsog:Granular_Material
              gsog:Rock_Material
            ) ;
        ] ;
      owl:onProperty gsoc:isQualityOf ;
    ] ;
.
gslth:Grain_Size_Average
  a owl:Class ;
  rdfs:comment "mean diameter for grain size distribution "@en ;
  rdfs:label "Grain Size Average "@en ;
  rdfs:subClassOf gslth:Grain_Size ;
  rdfs:subClassOf [
      a owl:Restriction ;
      owl:allValuesFrom xsd:decimal ;
      owl:onProperty gsoc:hasDataValue ;
    ] ;
  rdfs:subClassOf [
      a owl:Restriction ;
      owl:onProperty gsoc:hasUOM ;
      owl:someValuesFrom gsoc:Unit_of_Measure ;
    ] ;
.
gslth:Grain_Size_Category
  a owl:Class ;
  rdfs:comment "grain size range expressed using a named size category vocabulary"@en ;
  rdfs:isDefinedBy "GeoSciML v3"@en ;
  rdfs:label "Grain size term"@en ;
  rdfs:subClassOf gslth:Grain_Size ;
  rdfs:subClassOf [
      a owl:Restriction ;
      owl:allValuesFrom xsd:string ;
      owl:onProperty gsoc:hasDataValue ;
    ] ;
.
gslth:Grain_Size_Max
  a owl:Class ;
  rdfs:comment "upper bound of 95% interval for grain size distribution "@en ;
  rdfs:label "Grain Size Maximum "@en ;
  rdfs:subClassOf gslth:Grain_Size ;
  rdfs:subClassOf [
      a owl:Restriction ;
      owl:allValuesFrom xsd:decimal ;
      owl:onProperty gsoc:hasDataValue ;
    ] ;
  rdfs:subClassOf [
      a owl:Restriction ;
      owl:onProperty gsoc:hasUOM ;
      owl:someValuesFrom gsoc:Unit_of_Measure ;
    ] ;
.
gslth:Grain_Size_Min
  a owl:Class ;
  rdfs:comment "lower bound of 95% interval for grain size distribution "@en ;
  rdfs:label "Grain Size Minimum "@en ;
  rdfs:subClassOf gslth:Grain_Size ;
  rdfs:subClassOf [
      a owl:Restriction ;
      owl:allValuesFrom xsd:decimal ;
      owl:onProperty gsoc:hasDataValue ;
    ] ;
  rdfs:subClassOf [
      a owl:Restriction ;
      owl:onProperty gsoc:hasUOM ;
      owl:someValuesFrom gsoc:Unit_of_Measure ;
    ] ;
.
gslth:Particle_Aspect_Ratio_Category
  a owl:Class ;
  rdfs:comment "AspectRatio describes the geometry of particles based on the ratios of lengths of long, intermediate and short axes of grains. Equates to sphericity in sedimentary rocks (ie: the degree to which the shape of a particle approximates a sphere).  A quantitative specification based on the ratio of lengths of long, intermediate and short axes of grain shape (Sneed and Folk, 1958; Zingg, 1935). (eg: prolate, slightly flattened, very bladed, equant, acicular, tabular) "@en ;
  rdfs:isDefinedBy "GeoSciML v4"@en ;
  rdfs:label "Particle aspect ratio "@en ;
  rdfs:subClassOf gsoc:Quality ;
  rdfs:subClassOf [
      a owl:Restriction ;
      owl:allValuesFrom gsoc:Shape ;
      owl:onProperty gsoc:isQualityOf ;
    ] ;
.
gslth:Particle_Sorting_Category
  a owl:Class ;
  rdfs:comment "The Sorting attribute holds text terms to specify size distribution of particles in a CompoundMaterial. Terminology for sorting in sedimentary rocks is based on the quantitative Graphic Standard Deviation (IGSD) scheme proposed by Folk (1968, 1974).  Example terms for this attribute may include sedimentary terms such as well sorted and poorly sorted, or igneous terms such as porphyritic, equigranuilar, seriate."@en ;
  rdfs:isDefinedBy "GeoSciML v4"@en ;
  rdfs:label "Particle sorting"@en ;
  rdfs:subClassOf gsoc:Quality ;
  rdfs:subClassOf [
      a owl:Restriction ;
      owl:allValuesFrom xsd:string ;
      owl:onProperty gsoc:hasDataValue ;
    ] ;
  rdfs:subClassOf [
      a owl:Restriction ;
      owl:allValuesFrom [
          a owl:Class ;
          owl:unionOf (
              gsog:Granular_Material
              gsog:Rock_Material
            ) ;
        ] ;
      owl:onProperty gsoc:isQualityOf ;
    ] ;
.
gslth:Rock_Material_Color
  a owl:Class ;
  rdfs:comment "Property for specification of color of rocks, minerals, other Earth Material "@en ;
  rdfs:label "Earth Material Color"@en ;
  rdfs:subClassOf gsoc:Quality ;
  rdfs:subClassOf [
      a owl:Restriction ;
      owl:allValuesFrom gsoc:Amount_Of_Matter ;
      owl:onProperty gsoc:isQualityOf ;
    ] ;
  rdfs:subClassOf [
      a owl:Restriction ;
      owl:onProperty gsoc:hasValue ;
      owl:someValuesFrom gsoc:Colour ;
    ] ;
.
gslth:Rock_Material_Composition_Category
  a owl:Class ;
  rdfs:comment "Term to specify the gross compositional character of a rock material. Composition as used here is loosely construed to include both chemical composition and petrograpic composition, thus multiple values may be applied to a single rock, e.g. metaluminous and alkalic, undersaturated and basic, etc. Terms would typically include broad chemical classifications such as silicate, carbonate, ferromagnesian, oxide.  However, this attribute may have different terminology for different kinds of rocks - for example sandstone petrographic classification terms (e.g. feldspathic) might be placed here."@en ;
  rdfs:isDefinedBy "GeoSciML v4"@en ;
  rdfs:label "Rock material composition category"@en ;
  rdfs:subClassOf gsoc:Quality ;
  rdfs:subClassOf [
      a owl:Restriction ;
      owl:allValuesFrom gsog:Rock_Material ;
      owl:onProperty gsoc:isQualityOf ;
    ] ;
.
gslth:Rock_Material_Genetic_Category
  a owl:Class ;
  rdfs:comment "A term that represents a summary geologic history of the material. (ie, a genetic process classifier term) Examples include igneous, sedimentary, metamorphic, shock metamorphic, volcanic, pyroclastic."@en ;
  rdfs:isDefinedBy "GeoSciML v4"@en ;
  rdfs:label "Rock material genetic category"@en ;
  rdfs:subClassOf gsoc:Quality ;
  rdfs:subClassOf [
      a owl:Restriction ;
      owl:allValuesFrom gsog:Rock_Material ;
      owl:onProperty gsoc:isQualityOf ;
    ] ;
.
gslth:acidic_igneous_material
  a owl:Class ;
  rdfs:comment "Igneous material with more than 63 percent SiO2."@en ;
  rdfs:comment "dct:source--  after LeMaitre et al. 2002"@en ;
  rdfs:label "acidic igneous material"@en ;
  rdfs:subClassOf gslth:igneous_material ;
.
gslth:acidic_igneous_rock
  a owl:Class ;
  rdfs:comment "Igneous rock with more than 63 percent SiO2."@en ;
  rdfs:comment "dct:source--  after LeMaitre et al. 2002"@en ;
  rdfs:label "acidic igneous rock"@en ;
  rdfs:subClassOf gslth:acidic_igneous_material ;
  rdfs:subClassOf gslth:igneous_rock ;
.
gslth:alkali-olivine_basalt
  a owl:Class ;
  rdfs:comment "Alkali olivine basalt is silica-undersaturated, characterized by the absence of orthopyroxene, absence of quartz, presence of olivine, and typically contains some feldspathoid mineral, alkali feldspar or phlogopite in the groundmass. Feldspar phenocrysts typically are labradorite to andesine in composition. Augite is rich in titanium compared to augite in tholeiitic basalt. Alkali olivine basalt is relatively rich in sodium."@en ;
  rdfs:comment "The definition of tholeiite and alkali basalt here are more prescriptive than those found in most reference authorities. This is to actually provide some descriptive criteria to allow assignment of rocks on a hand sample basis to the tholeiite or alkali basalt categories if detailed petrographic or chemical data are available."@en ;
  rdfs:comment "dct:source--  http://en.wikipedia.org/wiki/Basalt; Carmichael, I.S. Turner, F.J., Verhoogen, John, 1974, Igneous petrology: New York, McGraw HIll Book Co., p.42-43."@en ;
  rdfs:label "alkali olivine basalt"@en ;
  rdfs:subClassOf gslth:basalt ;
.
gslth:alkali_feldspar_granite
  a owl:Class ;
  rdfs:comment "Granitic rock that has a plagioclase to total feldspar ratio less than 0.1. QAPF field 2."@en ;
  rdfs:comment "dct:source--  LeMaitre et al. 2002"@en ;
  rdfs:label "alkali feldspar granite"@en ;
  rdfs:subClassOf gslth:granitoid ;
.
gslth:alkali_feldspar_rhyolite
  a owl:Class ;
  rdfs:comment "Rhyolitoid in which the ratio of plagioclase to total feldspar is less than 0.1. QAPF field 2."@en ;
  rdfs:comment "dct:source--  LeMaitre et al. 2002"@en ;
  rdfs:label "alkali feldspar rhyolite"@en ;
  rdfs:subClassOf gslth:rhyolitoid ;
.
gslth:alkali_feldspar_syenite
  a owl:Class ;
  rdfs:comment "Alkali feldspar syenitic rock that contains 0-5 percent quartz and no feldspathoid in the QAPF fraction. QAPF field 6."@en ;
  rdfs:comment "dct:source--  LeMaitre et al. 2002"@en ;
  rdfs:label "alkali feldspar syenite"@en ;
  rdfs:subClassOf gslth:alkali_feldspar_syenitic_rock ;
.
gslth:alkali_feldspar_syenitic_rock
  a owl:Class ;
  rdfs:comment "Syenitoid with a plagioclase to total feldspar ratio of less than 0.1. QAPF fields 6, 6*, and 6'."@en ;
  rdfs:comment "dct:source--  LeMaitre et al. 2002"@en ;
  rdfs:label "alkali feldspar syenitic rock"@en ;
  rdfs:subClassOf gslth:syenitoid ;
.
gslth:alkali_feldspar_trachyte
  a owl:Class ;
  rdfs:comment "Trachytoid that has a plagioclase to total feldspar ratio less than 0.1, between 0 and 5 percent quartz in the QAPF fraction, and no feldspathoid minerals. QAPF field 6."@en ;
  rdfs:comment "dct:source--  LeMaitre et al. 2002"@en ;
  rdfs:label "alkali feldspar trachyte"@en ;
  rdfs:subClassOf gslth:alkali_feldspar_trachytic_rock ;
.
gslth:alkali_feldspar_trachytic_rock
  a owl:Class ;
  rdfs:comment "Trachytoid that has a plagioclase to total feldspar ratio less than 0.1. QAPF fields 6, 6', and 6*."@en ;
  rdfs:comment "dct:source--  LeMaitre et al. 2002"@en ;
  rdfs:label "alkali feldspar trachytic rock"@en ;
  rdfs:subClassOf gslth:trachytoid ;
.
gslth:amphibolite
  a owl:Class ;
  rdfs:comment "Metamorphic rock mainly consisting of green, brown or black amphibole and plagioclase (including albite), which combined form 75 percent or more of the rock, and both of which are present as major constituents. The amphibole constitutes 50 percent or more of the total mafic constituents and is present in an amount of 30 percent or more; other common minerals include quartz, clinopyroxene, garnet, epidote-group minerals, biotite, titanite and scapolite."@en ;
  rdfs:comment "dct:source--  Coutinho et al. 2007, IUGS SCMR chapter 8 (http://www.bgs.ac.uk/SCMR/)"@en ;
  rdfs:label "amphibolite"@en ;
  rdfs:subClassOf gslth:metamorphic_rock ;
.
gslth:andesite
  a owl:Class ;
  rdfs:comment "Fine-grained igneous rock with less than 20 percent quartz and less than 10 percent feldspathoid minerals in the QAPF fraction, in which the ratio of plagioclase to total feldspar is greater 0.65. Includes rocks defined modally in QAPF fields 9 and 10 or chemically in TAS field O2 as andesite. Basalt and andesite, which share the same QAPF fields, are distinguished chemically based on silica content, with basalt defined to contain less than 52 weight percent silica. If chemical data are not available, the color index is used to distinguish the categories, with basalt defined to contain greater than 35 percent mafic minerals by volume or greater than 40 percent mafic minerals by weight. Typically consists of plagioclase (frequently zoned from labradorite to oligoclase), pyroxene, hornblende and/or biotite. Fine grained equivalent of dioritic rock."@en ;
  rdfs:comment "Note the mela-andesite and leuco-basalt categories are not recommended in this system. If chemical analytical data are available to constrain the silica content, the basalt or andesite category should be used."@en ;
  rdfs:comment "dct:source--  after LeMaitre et al. 2002"@en ;
  rdfs:label "andesite"@en ;
  rdfs:subClassOf gslth:fine_grained_igneous_rock ;
  rdfs:subClassOf gslth:intermediate_composition_igneous_rock ;
.
gslth:anorthosite
  a owl:Class ;
  rdfs:comment "Anorthositic rock that contains between 0 and 5 percent quartz and no feldspathoid mineral in the QAPF fraction. QAPF field 10."@en ;
  rdfs:comment "dct:source--  LeMaitre et al. 2002"@en ;
  rdfs:label "anorthosite"@en ;
  rdfs:subClassOf gslth:anorthositic_rock ;
.
gslth:anorthositic_rock
  a owl:Class ;
  rdfs:comment "Anorthositic rock term invented to label the combined QAPF fields 10, 10*, and 10', in order to construct hierarchy in this vocabulary."@en ;
  rdfs:comment "Leucocratic phaneritic crystalline igneous rock consisting essentially of plagioclase, often with small amounts of pyroxene. By definition, colour index M is less than 10, and plagiclase to total feldspar ratio is greater than 0.9. Less than 20 percent quartz and less than 10 percent feldspathoid in the QAPF fraction. QAPF field 10, 10*, and 10'."@en ;
  rdfs:comment "dct:source--  LeMaitre et al. 2002; This vocabulary"@en ;
  rdfs:label "anorthositic rock"@en ;
  rdfs:subClassOf gslth:phaneritic_igneous_rock ;
.
gslth:anthracite_coal
  a owl:Class ;
  a owl:NamedIndividual ;
  rdfs:comment "Coal that has vitrinite mean random reflectance greater than 2.0% (determined in conformance with ISO 7404-5). Less than 12-14 percent volatiles (dry, ash free), greater than 91 percent fixed carbon (dry, ash free basis). The highest rank coal; very hard, glossy, black, with semimetallic luster, semi conchoidal fracture."@en ;
  rdfs:comment "dct:source--  Economic commission for Europe, committee on Sustainable Energy- United Nations (ECE-UN), 1998, International Classification of in-Seam Coals: Energy 19, 41 pp; see also Neuendorf et al. 2005; http://en.wikipedia.org/wiki/Coal#Types_of_coal; Eberhard Lindner; Chemie für Ingenieure; Lindner Verlag Karlsruhe, S. 258"@en ;
  rdfs:comment "skos:altLabel--  High rank coal"@en ;
  rdfs:label "anthracite"@en ;
  rdfs:label "anthrazit"@de ;
  rdfs:subClassOf gslth:coal ;
.
gslth:anthropogenic_material
  a owl:Class ;
  rdfs:comment "Material known to have artificial (human-related) origin; insufficient information to classify in more detail."@en ;
  rdfs:comment "dct:source--  This vocabulary"@en ;
  rdfs:label "anthropogenic material"@en ;
  rdfs:subClassOf gslth:compound_material ;
.
gslth:anthropogenic_unconsolidated_material
  a owl:Class ;
  rdfs:comment "Unconsolidated material known to have artificial (human-related) origin."@en ;
  rdfs:comment "dct:source--  This vocabulary"@en ;
  rdfs:label "anthropogenic unconsolidated material"@en ;
  rdfs:subClassOf gslth:anthropogenic_material ;
  rdfs:subClassOf gslth:unconsolidated_material ;
.
gslth:aphanite
  a owl:Class ;
  rdfs:comment "Rock that is too fine grained to categorize in more detail."@en ;
  rdfs:comment "dct:source--  This vocabulary"@en ;
  rdfs:label "aphanite"@en ;
  rdfs:subClassOf gslth:rock ;
.
gslth:aplite
  a owl:Class ;
  rdfs:comment "Light coloured crystalline rock, characterized by a fine grained allotriomorphic-granular (aplitic, saccharoidal or xenomorphic) texture; typically granitic composition, consisting of quartz, alkali feldspar and sodic plagioclase."@en ;
  rdfs:comment "dct:source--  Neuendorf et al. 2005"@en ;
  rdfs:label "aplite"@en ;
  rdfs:subClassOf gslth:phaneritic_igneous_rock ;
.
gslth:arenite
  a owl:Class ;
  rdfs:comment "Clastic sandstone that contains less than 10 percent matrix. Matrix is mud-size silicate minerals (clay, feldspar, quartz, rock fragments, and alteration products) of detrital or diagenetic nature."@en ;
  rdfs:comment "dct:source--  Pettijohn, Potter, Siever, 1972, Sand and Sandstone: New York, Springer Verlag, 681 p."@en ;
  rdfs:label "arenit"@de ;
  rdfs:label "arenite"@en ;
  rdfs:subClassOf gslth:clastic_sandstone ;
.
gslth:ash_and_lapilli
  a owl:Class ;
  rdfs:comment "Tephra in which less than 25 percent of fragments are greater than 64 mm in longest dimension"@en ;
  rdfs:comment "dct:source--  Schmid 1981; LeMaitre et al. 2002"@en ;
  rdfs:label "ash and lapilli"@en ;
  rdfs:subClassOf gslth:tephra ;
.
gslth:ash_breccia_bomb_or_block_tephra
  a owl:Class ;
  rdfs:comment "Tephra in which more than 25 percent of particles are greater than 64 mm in largest dimension. Includes ash breccia, bomb tephra and block tephra of Gillespie and Styles (1999)"@en ;
  rdfs:comment "dct:source--  Schmid 1981; LeMaitre et al. 2002"@en ;
  rdfs:label "ash breccia bomb or block tephra"@en ;
  rdfs:subClassOf gslth:tephra ;
.
gslth:ash_tuff_lapillistone_and_lapilli_tuff
  a owl:Class ;
  rdfs:comment "Pyroclastic rock in which less than 25 percent of rock by volume are more than 64 mm in longest diameter. Includes tuff, lapilli tuff, and lapillistone."@en ;
  rdfs:comment "dct:source--  Schmid 1981; LeMaitre et al. 2002"@en ;
  rdfs:label "ash tuff lapillistone and lapilli tuff"@en ;
  rdfs:subClassOf gslth:pyroclastic_rock ;
.
gslth:basalt
  a owl:Class ;
  rdfs:comment "Fine-grained or porphyritic igneous rock with less than 20 percent quartz, and less than 10 percent feldspathoid minerals, in which the ratio of plagioclase to total feldspar is greater 0.65. Typically composed of calcic plagioclase and clinopyroxene; phenocrysts typically include one or more of calcic plagioclase, clinopyroxene, orthopyroxene, and olivine. Includes rocks defined modally in QAPF fields 9 and 10 or chemically in TAS field B as basalt. Basalt and andesite are distinguished chemically based on silica content, with basalt defined to contain less than 52 weight percent silica. If chemical data are not available, the color index is used to distinguish the categories, with basalt defined to contain greater than 35 percent mafic minerals by volume or greater than 40 percent mafic minerals by weight."@en ;
  rdfs:comment "dct:source--  after LeMaitre et al. 2002"@en ;
  rdfs:label "basalt"@en ;
  rdfs:subClassOf gslth:basic_igneous_rock ;
  rdfs:subClassOf gslth:fine_grained_igneous_rock ;
.
gslth:basanite
  a owl:Class ;
  rdfs:comment "Tephritoid that has a plagioclase to total feldspar ratio greater than 0.9, and contains more than 10 percent normative (CIPW) olivine."@en ;
  rdfs:comment "dct:source--  LeMaitre et al. 2002"@en ;
  rdfs:label "basanite"@en ;
  rdfs:subClassOf gslth:tephritoid ;
.
gslth:basanitic_foidite
  a owl:Class ;
  rdfs:comment "Foiditoid that contains less than 90 percent feldspathoid minerals in the QAPF fraction, and has a plagioclase to total feldspar ratio that is greater than 0.5, with greater than 10 percent normative olivine."@en ;
  rdfs:comment "dct:source--  LeMaitre et al. 2002"@en ;
  rdfs:label "basanitic foidite"@en ;
  rdfs:subClassOf gslth:foiditoid ;
.
gslth:basic_igneous_material
  a owl:Class ;
  rdfs:comment "Igneous material with between 45 and 52 percent SiO2."@en ;
  rdfs:comment "dct:source--  after LeMaitre et al. 2002"@en ;
  rdfs:label "basic igneous material"@en ;
  rdfs:subClassOf gslth:igneous_material ;
.
gslth:basic_igneous_rock
  a owl:Class ;
  rdfs:comment "Igneous rock with between 45 and 52 percent SiO2."@en ;
  rdfs:comment "dct:source--  after LeMaitre et al. 2002"@en ;
  rdfs:label "basic igneous rock"@en ;
  rdfs:subClassOf gslth:basic_igneous_material ;
  rdfs:subClassOf gslth:igneous_rock ;
.
gslth:bauxite
  a owl:Class ;
  rdfs:comment "Highly aluminous material containing abundant aluminium hydroxides (gibbsite, less commonly boehmite, diaspore) and aluminium-substituted iron oxides or hydroxides and generally minor or negligible kaolin minerals; may contain up to 20 percent quartz. commonly has a pisolitic or nodular texture, and may be cemented."@en ;
  rdfs:comment "dct:source--  Eggleton 2001"@en ;
  rdfs:label "bauxite"@en ;
  rdfs:subClassOf gslth:material_formed_in_surficial_environment ;
.
gslth:biogenic_sediment
  a owl:Class ;
  rdfs:comment "Corresponding biogenic sedimentary material and biogenic sedimentary rock categories are not included based on the interpretation that biogenic sedimentary rock will be in a different category, e.g. carbonate sedimentary rock or organic rich sedimentary rock."@en ;
  rdfs:comment "Sediment composed of greater than 50 percent material of biogenic origin. Because the biogenic material may be skeletal remains that are not organic, all biogenic sediment is not necessarily organic-rich."@en ;
  rdfs:comment "dct:source--  SLTTs 2004"@en ;
  rdfs:label "biogenic sediment"@en ;
  rdfs:subClassOf gslth:sediment ;
.
gslth:biogenic_silica_sedimentary_rock
  a owl:Class ;
  rdfs:comment "Sedimentary rock that consists of at least 50 percent silicate mineral material, deposited directly by biological processes at the depositional surface, or in particles formed by biological processes within the basin of deposition."@en ;
  rdfs:comment "dct:source--  based on NADM SLTT sedimentary; Hallsworth and Knox 1999"@en ;
  rdfs:label "biogenic silica sedimentary rock"@en ;
  rdfs:subClassOf gslth:non_clastic_siliceous_sedimentary_rock ;
.
gslth:bituminous_coal
  a owl:Class ;
  a owl:NamedIndividual ;
  rdfs:comment "Coal that has vitrinite mean random reflectance greater than 0.6% and less than 2.0% (determined in conformance with ISO 7404-5), or has a gross calorific value greater than 24 MJ/kg (determined in conformance with ISO 1928). Hard, black, organic rich sedimentary rock; contains less than 91 percent fixed carbon on a dry, mineral-matter-free basis, and greater than 13-14 percent volatiles (dry, ash free). Formed from the compaction or induration of variously altered plant remains similar to those of peaty deposits."@en ;
  rdfs:comment "dct:source--  Economic commission for Europe, committee on Sustainable Energy- United Nations (ECE-UN), 1998, International Classification of in-Seam Coals: Energy 19, 41 pp; see also http://en.wikipedia.org/wiki/Coal#Types_of_coal; Eberhard Lindner; Chemie für Ingenieure; Lindner Verlag Karlsruhe, S. 258"@en ;
  rdfs:comment "skos:altLabel--  medium rank coal"@en ;
  rdfs:label "bituminous coal"@en ;
  rdfs:subClassOf gslth:coal ;
.
gslth:boninite
  a owl:Class ;
  rdfs:comment "andesitic rock that contains more than 8 percent MgO. Typically consists of phenocrysts of protoenstatite, orthopyroxene, clinopyroxene, and olivine in a glassy base full of crystallites, and exhibits textures characterisitc of rapid crystal growth."@en ;
  rdfs:comment "dct:source--  LeMaitre et al. 2002"@en ;
  rdfs:label "boninite"@en ;
  rdfs:subClassOf gslth:andesite ;
  rdfs:subClassOf gslth:high_magnesium_fine_grained_igneous_rocks ;
.
gslth:boulder_gravel_size_sediment
  a owl:Class ;
  rdfs:comment "Sediment containing greater than 30 percent boulder-size particles (greater than 256 mm in diameter)"@en ;
  rdfs:comment "dct:source--  Wentworth size scale"@en ;
  rdfs:label "boulder gravel size sediment"@en ;
  rdfs:subClassOf gslth:gravel_size_sediment ;
.
gslth:boundstone
  a owl:Class ;
  rdfs:comment "Sedimentary carbonate rock with preserved biogenic texture, whose original components were bound and encrusted together during deposition by the action of plants and animals during deposition, and remained substantially in the position of growth."@en ;
  rdfs:comment "dct:source--  Hallsworth and Knox 1999; SLTTs 2004"@en ;
  rdfs:label "boundstone"@en ;
  rdfs:subClassOf gslth:carbonate_sedimentary_rock ;
.
gslth:breccia
  a owl:Class ;
  rdfs:comment "Coarse-grained material composed of angular broken rock fragments; the fragments typically have sharp edges and unworn corners. The fragments may be held together by a mineral cement or in a fine-grained matrix, and consolidated or nonconsolidated. Clasts may be of any composition or origin. In sedimentary environments, breccia is used for material that consists entirely of angular fragments, mostly derived from a single source rock body, as in a rock avalanche deposit, and matrix is interpreted to be the product of comminution of clasts during transport. Diamictite or diamicton is used when the material reflects mixing of rock from a variety of sources, some sub angular or subrounded clasts may be present, and matrix is pre-existing fine grained material that is not a direct product of the brecciation/deposition process."@en ;
  rdfs:comment "dct:source--  Neuendorf et al. 2005"@en ;
  rdfs:label "breccia"@en ;
  rdfs:subClassOf gslth:compound_material ;
.
gslth:breccia_gouge_series
  a owl:Class ;
  rdfs:comment "Fault material with features such as void spaces (filled or unfilled), or unconsolidated matrix material between fragments, indicating loss of cohesion during deformation. Includes fault-related breccia and gouge."@en ;
  rdfs:comment "dct:source--  SLTTm 2004"@en ;
  rdfs:label "breccia gouge series"@en ;
  rdfs:subClassOf gslth:fault_related_material ;
.
gslth:calcareous_carbonate_sediment
  a owl:Class ;
  rdfs:comment "Carbonate sediment with a calcite (plus aragonite) to dolomite ratio greater than 1 to 1. Includes lime-sediments."@en ;
  rdfs:comment "dct:source--  after Hallsworth and Knox 1999"@en ;
  rdfs:label "calcareous carbonate sediment"@en ;
  rdfs:subClassOf gslth:calcareous_carbonate_sedimentary_material ;
  rdfs:subClassOf gslth:carbonate_sediment ;
.
gslth:calcareous_carbonate_sedimentary_material
  a owl:Class ;
  rdfs:comment "Carbonate sedimentary material of unspecified consolidation state with a calcite (plus aragonite) to dolomite ratio greater than 1 to 1. Includes lime-sediments, limestone and dolomitic limestone."@en ;
  rdfs:comment "dct:source--  after Hallsworth and Knox 1999"@en ;
  rdfs:label "calcareous carbonate sedimentary material"@en ;
  rdfs:subClassOf gslth:carbonate_sedimentary_material ;
.
gslth:calcareous_carbonate_sedimentary_rock
  a owl:Class ;
  rdfs:comment "Carbonate sedimentary rock with a calcite (plus aragonite) to dolomite ratio greater than 1 to 1. Includes limestone and dolomitic limestone."@en ;
  rdfs:comment "dct:source--  SLTTs 2004; Hallsworth and Knox 1999"@en ;
  rdfs:label "calcareous carbonate sedimentary rock"@en ;
  rdfs:subClassOf gslth:calcareous_carbonate_sedimentary_material ;
  rdfs:subClassOf gslth:carbonate_sedimentary_rock ;
.
gslth:carbonate_mud
  a owl:Class ;
  a owl:NamedIndividual ;
  rdfs:comment "Carbonate sediment composed of less than 25 percent clasts that have a maximum diameter more than 2 mm, and the ratio of sand size to mud size clasts is less than one."@en ;
  rdfs:comment "dct:source--  follow pattern used for clastic sand and mud categories, based on SLTTs 2004"@en ;
  rdfs:comment "skos:altLabel--  marl"@en ;
  rdfs:label "carbonate mud"@en ;
  rdfs:subClassOf gslth:carbonate_sediment ;
  rdfs:subClassOf gslth:mud_size_sediment ;
.
gslth:carbonate_mudstone
  a owl:Class ;
  a owl:NamedIndividual ;
  rdfs:comment "Mudstone that consists of greater than 50 percent carbonate minerals of any origin in the mud size fraction."@en ;
  rdfs:comment "Not a subcategory of carbonate sedimentary rock because definition does not specify 'carbonate minerals of intrabasinal origin', but is agnostic on origin of carbonate. Schnurrenberger et al. 2003 point out that it is very difficult (at least in lacustrine rocks) to distinguish chemically precipitated or diagenetic carbonate from primary biogenic carbonate. This distinction between biogenic, detrital, and pedogenic or authigenic carbonate material is thus not a good one to use in a general purpose classification system. Schnurrenberger, D., Russell, J. and Kelts, K., 2003, Classification of lacustrine sediments based on sedimentary components: Journal of Paleolimnology, v.29, p141-154."@en ;
  rdfs:comment "dct:source--  This vocabulary"@en ;
  rdfs:comment "skos:altLabel--  marlstone"@en ;
  rdfs:label "carbonate mudstone"@en ;
  rdfs:subClassOf gslth:carbonate_sedimentary_rock ;
  rdfs:subClassOf gslth:generic_mudstone ;
.
gslth:carbonate_ooze
  a owl:Class ;
  rdfs:comment "dct:source--  This vocabulary"@en ;
  rdfs:comment "ooze that consists of more than 50 percent carbonate skeletal remains"@en ;
  rdfs:label "carbonate ooze"@en ;
  rdfs:subClassOf gslth:carbonate_mud ;
  rdfs:subClassOf gslth:ooze ;
.
gslth:carbonate_rich_mud
  a owl:Class ;
  a owl:NamedIndividual ;
  rdfs:comment "Mud size sediment that contains between 10 and 50 percent carbonate minerals in any size fraction. Carbonate origin is not specified."@en ;
  rdfs:comment "dct:source--  This vocabulary"@en ;
  rdfs:comment "skos:altLabel--  carbonate rich loess"@en ;
  rdfs:comment "skos:altLabel--  marl"@en ;
  rdfs:label "carbonate rich mud"@en ;
  rdfs:subClassOf gslth:mud_size_sediment ;
.
gslth:carbonate_rich_mudstone
  a owl:Class ;
  a owl:NamedIndividual ;
  rdfs:comment "Carbonate-rich mudstone' definition limits carbonate to mud-size fraction to avoid overlap with 'impure carbonate sedimentary rock'. If carbonate minerals are in sand or gravel size fractions, use 'impure carbonate sedimentary rock'. The operational test typically used to identify this category is if the rock fizzes when hydrochloric acid is applied. The '10 percent carbonate' criteria is a fuzzy boundary."@en ;
  rdfs:comment "Mudstone that contains between 10 and 50 percent carbonate minerals in the mud size fraction. Carbonate origin is not specified."@en ;
  rdfs:comment "dct:source--  This vocabulary"@en ;
  rdfs:comment "skos:altLabel--  marlstone"@en ;
  rdfs:label "carbonate rich mudstone"@en ;
  rdfs:subClassOf gslth:generic_mudstone ;
.
gslth:carbonate_sediment
  a owl:Class ;
  rdfs:comment "Sediment in which at least 50 percent of the primary and/or recrystallized constituents are composed of one (or more) of the carbonate minerals calcite, aragonite and dolomite, in particles of intrabasinal origin."@en ;
  rdfs:comment "dct:source--  SLTTs 2004"@en ;
  rdfs:label "carbonate sediment"@en ;
  rdfs:subClassOf gslth:carbonate_sedimentary_material ;
  rdfs:subClassOf gslth:sediment ;
.
gslth:carbonate_sedimentary_material
  a owl:Class ;
  rdfs:comment "Sedimentary material in which at least 50 percent of the primary and/or recrystallized constituents are composed of one (or more) of the carbonate minerals calcite, aragonite and dolomite, in particles of intrabasinal origin."@en ;
  rdfs:comment "Should carbonate sedimentary material be considered a kind of chemical sedimentary material? Is biogenic precipitation a chemical sedimentary process?"@en ;
  rdfs:comment "dct:source--  SLTTs 2004"@en ;
  rdfs:label "carbonate sedimentary material"@en ;
  rdfs:subClassOf gslth:sedimentary_material ;
.
gslth:carbonate_sedimentary_rock
  a owl:Class ;
  rdfs:comment "Particularly for fine-grained sedimentary rocks, distinction of 'intrabasinal' versus 'clastic' genesis can be very interpretive. In practice the use of clastic mudstone terminology as opposed to carbonate mudstone terminology may be dermined by a priori knowledge about the rock being categorized. If it is associated with other clastic rocks, the clastic categories will be favored, if with cabonate rocks, the carbonate categories will be favored. Carbonate rock subcatgories are defined on two orthogonal dimensions--mineralogy (calcitic vs. dolomitic vs non-carbonate impurities), and texture. The texture categories used here are those of Dunham (1962), and involve grain size (matrix vs. grains/allochems), fabric (matrix vs. grain supported), and genesis (bound, frame, or fragmental). The textural approach used for carbonate rocks is conceptually incompatible with that used for clastic sedimentary rocks, which is solely grain size or mineralogy based. This leads to problems in the vocabulary for rocks of mixed siliclastic/carbonate mineralogy (grainstone vs. sandstone, carbonate mudstone vs. carbonate rich mudstone, how to accomodate marlstone...)."@en ;
  rdfs:comment "Sedimentary rock in which at least 50 percent of the primary and/or recrystallized constituents are composed of one (or more) of the carbonate minerals calcite, aragonite, magnesite or dolomite."@en ;
  rdfs:comment "dct:source--  SLTTs 2004"@en ;
  rdfs:label "carbonate sedimentary rock"@en ;
  rdfs:subClassOf gslth:carbonate_sedimentary_material ;
  rdfs:subClassOf gslth:sedimentary_rock ;
.
gslth:carbonate_wackestone
  a owl:Class ;
  rdfs:comment "Carbonate sedimentary rock with discernible mud supported depositional texture and containing greater than 10 percent allochems, and constituent particles are of intrabasinal origin. If particles are not intrabasinal, categorization as a mudstone or wackestone should be considered."@en ;
  rdfs:comment "dct:source--  Dunham 1962"@en ;
  rdfs:label "carbonate wackestone"@en ;
  rdfs:subClassOf gslth:carbonate_sedimentary_rock ;
.
gslth:carbonatite
  a owl:Class ;
  rdfs:comment "Igneous rock composed of more than 50 percent modal carbonate minerals."@en ;
  rdfs:comment "dct:source--  LeMaitre et al. 2002"@en ;
  rdfs:label "carbonatite"@en ;
  rdfs:subClassOf gslth:exotic_composition_igneous_rock ;
.
gslth:cataclasite_series
  a owl:Class ;
  rdfs:comment "Fault-related rock that maintained primary cohesion during deformation, with matrix comprising greater than 10 percent of rock mass; matrix is fine-grained material formed through grain size reduction by fracture as opposed to crystal plastic process that operate in mylonitic rock. Includes cataclasite, protocataclasite and ultracataclasite."@en ;
  rdfs:comment "dct:source--  Sibson, 1977; Scholz, 1990; Snoke and Tullis, 1998; Barker, 1998 Appendix II; NADM SLTTm, 2004"@en ;
  rdfs:label "cataclasite series"@en ;
  rdfs:subClassOf gslth:composite_genesis_rock ;
  rdfs:subClassOf gslth:fault_related_material ;
.
gslth:chalk
  a owl:Class ;
  rdfs:comment "A generally soft, white, very fine-grained, extremely pure, porous limestone. It forms under marine conditions from the gradual accumulation of skeletal elements from minute planktonic green algae (cocoliths), associated with varying proportions of larger microscopic fragments of bivalves, foraminifera and ostracods. It is common to find flint and chert nodules embedded in chalk."@en ;
  rdfs:comment "dct:source--  http://en.wikipedia.org/wiki/Chalk; C.S. Harris, 2009, unpublished web page, http://www.geologyshop.co.uk/chalk.htm"@en ;
  rdfs:label "chalk"@en ;
  rdfs:subClassOf gslth:limestone ;
.
gslth:chemical_sedimentary_material
  a owl:Class ;
  rdfs:comment "Sedimentary material that consists of at least 50 percent material produced by inorganic chemical processes within the basin of deposition. Includes inorganic siliceous, carbonate, evaporite, iron-rich, and phosphatic sediment classes."@en ;
  rdfs:comment "dct:source--  SLTTs 2004"@en ;
  rdfs:label "chemical sedimentary material"@en ;
  rdfs:subClassOf gslth:sedimentary_material ;
.
gslth:chlorite_actinolite_epidote_metamorphic_rock
  a owl:Class ;
  rdfs:comment "Metamorphic rock characterized by 50 percent or more of combined chlorite, actinolite and epidote. Category for rocks generally named greenschist or greenstone."@en ;
  rdfs:comment "Rock classified as Greenschist is difficult to categorize in the CGI SimpleLithology scheme. This stems in part from the variation in usage and the general fuzzy definition of the term. The definition of greenschist is generally something along the lines of 'metamorphosed rock with a greenish colour, characterized by the presence of actinolite, chlorite and epidote, and containing a planar or linear fabric. The presence or absence of schistose fabric in rocks called 'greenschist' is problematic. The fabric present in many rocks called greenschist is too weak or variably developed to meet the definition of 'schist' per CGI SimpleLithology. Generally if the rock has achieved metamorphic grade such that the term 'gneiss' is applicable, it would not be called greenschist. Thus, 'greenschist' would correspond most closely to a chlorite + actinolite rich 'Foliated metamorphic rock', but if it actually meets the definition of 'Schist' it would be a chlorite + actinolite 'Schist'."@en ;
  rdfs:comment "dct:source--  This vocabulary"@en ;
  rdfs:label "chlorite actinolite epidote metamorphic rock"@en ;
  rdfs:subClassOf gslth:metamorphic_rock ;
.
gslth:clastic_conglomerate
  a owl:Class ;
  a owl:NamedIndividual ;
  rdfs:comment "Clastic sedimentary rock composed of at least 30 percent rounded to subangular fragments larger than 2 mm in diameter; typically contains finer grained material in interstices between larger fragments. If more than 15 percent of the fine grained matrix is of indeterminant clastic or diagenetic origin and the fabric is matrix supported, may also be categorized as wackestone. If rock has unsorted or poorly sorted texture with a wide range of particle sizes, may also be categorized as diamictite."@en ;
  rdfs:comment "Note this category is equivlanet to category labeled 'Conglomeratic rock in SLTTs (2004), not to the category labeled 'Conglomerate' in that system."@en ;
  rdfs:comment "dct:source--  Neuendorf et al. 2005; SLTTs 2004"@en ;
  rdfs:comment "skos:altLabel--  conglomeratic rock"@en ;
  rdfs:label "conglomerate"@en ;
  rdfs:subClassOf gslth:clastic_sedimentary_rock ;
  rdfs:subClassOf gslth:generic_conglomerate ;
.
gslth:clastic_mudstone
  a owl:Class ;
  a owl:NamedIndividual ;
  rdfs:comment "Clastic sedimentary rock consisting of less than 30 percent gravel-size (2 mm) particles and with a mud to sand ratio greater than 1."@en ;
  rdfs:comment "Distinction of intrabasinal, diagenetic, or clastic genesis for very fine-grained carbonate minerals is interpretive in many cases. If there is uncertainty on the mudstone category based on intrabasinal vs epiclastic distinction required for clastic sedimentary rock-carbonate sedimentary rock categorization in this system, it is recommended to use the generic_mudstone category. This category is the union of the various fields labeled 'mudstone' with various qualifiers in Folk, 1954, Figure 1a, although Folk's (1954) category labeled 'mudstone' is a much more restricted category. The CGI category is equivalent to category labeled 'Mudrock' in SLTTs (2004), not to the category labeled 'Mudstone' adopted by that system from Folk (1954). Schnurrenberger, D., Russell, J. and Kelts, K., 2003, Classification of lacustrine sediments based on sedimentary components: Journal of Paleolimnology, v.29, p141-154."@en ;
  rdfs:comment "dct:source--  Pettijohn et al. 1987 referenced in Hallsworth and Knox 1999."@en ;
  rdfs:comment "skos:altLabel--  clastic mudstone"@en ;
  rdfs:comment "skos:altLabel--  mudrock"@en ;
  rdfs:label "mudstone"@en ;
  rdfs:subClassOf gslth:clastic_sedimentary_rock ;
  rdfs:subClassOf gslth:generic_mudstone ;
.
gslth:clastic_sandstone
  a owl:Class ;
  a owl:NamedIndividual ;
  rdfs:comment "Clastic sedimentary rock in which less than 30 percent of particles are greater than 2 mm in diameter (gravel) and the sand to mud ratio is at least 1."@en ;
  rdfs:comment "Note this category is equivalent to cagetory labeled 'sandy rock' in SLTTs (2004), not to the much more restricted category labeled 'Sandstone' in that system."@en ;
  rdfs:comment "dct:source--  SLTTs 2004; Neuendorf et al. 2005; particle size from Wentworth grade scale"@en ;
  rdfs:comment "skos:altLabel--  clastic sandstone"@en ;
  rdfs:comment "skos:altLabel--  sandy rock"@en ;
  rdfs:label "sandstone"@en ;
  rdfs:subClassOf gslth:clastic_sedimentary_rock ;
  rdfs:subClassOf gslth:generic_sandstone ;
.
gslth:clastic_sediment
  a owl:Class ;
  rdfs:comment "Choice of 'clastic' is purposful. Other suggested labels for this category include siliciclastic and terrigineous clastic. Siliciclastic is considered too limiting because the category includes rocks that consists clasts of carbonate minerals, e.g. epiclastic detritus eroded from carbonate rock. Terrigineous clastic was considered and rejected first because it is considered redundant, anything that is terrigineous is clastic. Second, it is questionable if clastic sediment derived by submarine processes (fragementation by gravity sliding, faulting, or volcanic activity, with transport by sediment gravity flow or submarine currents) is terrigineous, but it is clastic and is meant to be included in this category."@en ;
  rdfs:comment "Sediment in which at least 50 percent of the constituent particles were derived from erosion, weathering, or mass-wasting of pre-existing earth materials, and transported to the place of deposition by mechanical agents such as water, wind, ice and gravity."@en ;
  rdfs:comment "dct:source--  SLTTs 2004; Neuendorf et al. 2005"@en ;
  rdfs:label "clastic sediment"@en ;
  rdfs:subClassOf gslth:clastic_sedimentary_material ;
  rdfs:subClassOf gslth:sediment ;
.
gslth:clastic_sedimentary_material
  a owl:Class ;
  rdfs:comment "Sedimentary material of unspecified consolidation state in which at least 50 percent of the constituent particles were derived from erosion, weathering, or mass-wasting of pre-existing earth materials, and transported to the place of deposition by mechanical agents such as water, wind, ice and gravity."@en ;
  rdfs:comment "dct:source--  SLTTs 2004; Neuendorf et al. 2005"@en ;
  rdfs:label "clastic sedimentary material"@en ;
  rdfs:subClassOf gslth:sedimentary_material ;
.
gslth:clastic_sedimentary_rock
  a owl:Class ;
  rdfs:comment "Sedimentary rock in which at least 50 percent of the constituent particles were derived from erosion, weathering, or mass-wasting of pre-existing earth materials, and transported to the place of deposition by mechanical agents such as water, wind, ice and gravity."@en ;
  rdfs:comment "The conglomerate, sandstone, mudstone, and wackestone categories are not defined as kinds of clastic sedimentary rocks because rocks meeting their purely grainsize based definitions might also be iron-rich, phosphatic, or carbonate. This is based on GeoSciML allowance to assign rocks to more than one lithology category. For example to categorize a rock as a clastic conglomerate requires assignment ot the 'clastic sedimentary rock' category and to the 'conglomerate' category. Particularly for fine-grained sedimentary rocks, distinction of 'intrabasinal' versus 'clastic' genesis can be very interpretive. In practice the use of clastic mudstone terminology as opposed to carbonate mudstone terminology may be dermined by a priori knowledge about the rock being categorized. If it is associated with other clastic rocks, the clastic categories will be favored, if with cabonate rocks, the carbonate categories will be favored."@en ;
  rdfs:comment "dct:source--  SLTTs 2004; Neuendorf et al. 2005"@en ;
  rdfs:label "clastic sedimentary rock"@en ;
  rdfs:subClassOf gslth:clastic_sedimentary_material ;
  rdfs:subClassOf gslth:sedimentary_rock ;
.
gslth:clay
  a owl:Class ;
  rdfs:comment "Mud that consists of greater than 50 percent particles with grain size less than 0.004 mm"@en ;
  rdfs:comment "dct:source--  based on SLTTs 2004; Neuendorf et al. 2005; particle size from Wentworth grade scale"@en ;
  rdfs:label "clay"@en ;
  rdfs:subClassOf gslth:mud ;
.
gslth:claystone
  a owl:Class ;
  rdfs:comment "Mudstone that contains no detectable silt, inferred to consist virtually entirely of clay-size particles."@en ;
  rdfs:comment "dct:source--  This vocabulary"@en ;
  rdfs:label "claystone"@en ;
  rdfs:subClassOf gslth:clastic_mudstone ;
.
gslth:coal
  a owl:Class ;
  rdfs:comment "A consolidated organic sedimentary material having less than 75% moisture. This category includes low, medium, and high rank coals according to International Classification of In-Seam Coal (United Nations, 1998), thus including lignite. Sapropelic coal is not distinguished in this category from humic coals. Formed from the compaction or induration of variously altered plant remains similar to those of peaty deposits."@en ;
  rdfs:comment "dct:source--  Economic commission for Europe, committee on Sustainable Energy- United Nations (ECE-UN), 1998, International Classification of in-Seam Coals: Energy 19, 41 pp."@en ;
  rdfs:label "coal"@en ;
  rdfs:label "kohle"@de ;
  rdfs:subClassOf gslth:organic_rich_sedimentary_rock ;
.
gslth:cobble_gravel_size_sediment
  a owl:Class ;
  rdfs:comment "Sediment containing greater than 30 percent cobble-size particles (64-256 mm in diameter)"@en ;
  rdfs:comment "dct:source--  Wentworth size scale"@en ;
  rdfs:label "cobble gravel size sediment"@en ;
  rdfs:subClassOf gslth:gravel_size_sediment ;
.
gslth:composite_genesis_material
  a owl:Class ;
  rdfs:comment "Material of unspecified consolidation state formed by geological modification of pre-existing materials outside the realm of igneous and sedimentary processes. Includes rocks formed by impact metamorphism, standard dynamothermal metamorphism, brittle deformation, weathering, metasomatism and hydrothermal alteration (diagenesis is a sedimentary process in this context)."@en ;
  rdfs:comment "dct:source--  SLTTm 2004"@en ;
  rdfs:label "composite genesis material"@en ;
  rdfs:subClassOf gslth:compound_material ;
.
gslth:composite_genesis_rock
  a owl:Class ;
  rdfs:comment "Rock formed by geological modification of pre-existing rocks outside the realm of igneous and sedimentary processes. Includes rocks formed by impact metamorphism, standard dynamothermal metamorphism, brittle deformation, weathering, metasomatism and hydrothermal alteration (diagenesis is a sedimentary process in this context)."@en ;
  rdfs:comment "dct:source--  SLTTm 2004"@en ;
  rdfs:label "composite genesis rock"@en ;
  rdfs:subClassOf gslth:composite_genesis_material ;
  rdfs:subClassOf gslth:rock ;
.
gslth:compound_material
  a owl:Class ;
  rdfs:comment "An Earth Material composed of an aggregation of particles of Earth Material, possibly including other compound Materials. This is 'top' of lithology category hierarchy, and should be used to indicate 'any rock or unconsolidated material'."@en ;
  rdfs:comment "dct:source--  NADM C1 2004"@en ;
  rdfs:label "compound material"@en ;
  rdfs:subClassOf gsog:Rock_Material ;
.
gslth:crystalline_carbonate
  a owl:Class ;
  rdfs:comment "Carbonate rock of indeterminate mineralogy in which diagenetic processes have obliterated any original depositional texture."@en ;
  rdfs:comment "dct:source--  SLTTs 2004"@en ;
  rdfs:label "crystalline carbonate"@en ;
  rdfs:subClassOf gslth:carbonate_sedimentary_rock ;
.
gslth:dacite
  a owl:Class ;
  rdfs:comment "Fine grained or porphyritic crystalline rock that contains less than 90 percent mafic minerals, between 20 and 60 percent quartz in the QAPF fraction, and has a plagioclase to total feldspar ratio greater than 0.65. Includes rocks defined modally in QAPF fields 4 and 5 or chemically in TAS Field O3. Typcially composed of quartz and sodic plagioclase with minor amounts of biotite and/or hornblende and/or pyroxene; fine-grained equivalent of granodiorite and tonalite."@en ;
  rdfs:comment "dct:source--  LeMaitre et al. 2002"@en ;
  rdfs:label "dacite"@en ;
  rdfs:subClassOf gslth:acidic_igneous_rock ;
  rdfs:subClassOf gslth:fine_grained_igneous_rock ;
.
gslth:diamictite
  a owl:Class ;
  rdfs:comment "Unsorted or poorly sorted, clastic sedimentary rock with a wide range of particle sizes including a muddy matrix. Biogenic materials that have such texture are excluded. Distinguished from conglomerate, sandstone, mudstone based on polymodality and lack of structures related to transport and deposition of sediment by moving air or water. If more than 10 percent of the fine grained matrix is of indeterminant clastic or diagenetic origin and the fabric is matrix supported, may also be categorized as wacke."@en ;
  rdfs:comment "dct:source--  Fairbridge and Bourgeois 1978"@en ;
  rdfs:label "diamictite"@en ;
  rdfs:subClassOf gslth:clastic_sedimentary_rock ;
.
gslth:diamicton
  a owl:Class ;
  rdfs:comment "Unsorted or poorly sorted, clastic sediment with a wide range of particle sizes, including a muddy matrix. Biogenic materials that have such texture are excluded. Distinguished from conglomerate, sandstone, mudstone based on polymodality and lack of structures related to transport and deposition of sediment by moving air or water. Assignment to an other size class can be used in conjunction to indicate the dominant grain size."@en ;
  rdfs:comment "dct:source--  Fairbridge and Bourgeois 1978"@en ;
  rdfs:comment "definition amplified to help distinguish diamicton, conglomerate and wackestone in this version"@en ;
  rdfs:label "diamicton"@en ;
  rdfs:subClassOf gslth:clastic_sediment ;
.
gslth:diorite
  a owl:Class ;
  rdfs:comment "Phaneritic crystalline rock consisting of intermediate plagioclase, commonly with hornblende and often with biotite or augite; colour index M less than 90, sodic plagioclase (An0-An50), no feldspathoid, and between 0 and 5 percent quartz. Includes rocks defined modally in QAPF field 10 as diorite."@en ;
  rdfs:comment "dct:source--  LeMaitre et al. 2002"@en ;
  rdfs:label "diorite"@en ;
  rdfs:subClassOf gslth:dioritic_rock ;
.
gslth:dioritic_rock
  a owl:Class ;
  rdfs:comment "Phaneritic crystalline rock with M less than 90, consisting of intermediate plagioclase, commonly with hornblende and often with biotite or augite. A dioritoid with a plagioclase to total feldspar ratio (in the QAPF fraction) greater than 0.9. Includes rocks defined modally in QAPF fields 10, 10' and 10*."@en ;
  rdfs:comment "dct:source--  LeMaitre et al. 2002"@en ;
  rdfs:label "dioritic rock"@en ;
  rdfs:subClassOf gslth:dioritoid ;
.
gslth:dioritoid
  a owl:Class ;
  rdfs:comment "Phaneritic crystalline igneous rock with M less than 90, consisting of intermediate plagioclase, commonly with hornblende and often with biotite or augite. Plagioclase to total feldspar ratio is greater that 0.65, and anorthite content of plagioclase is less than 50 percent. Less than 10 percent feldspathoid mineral and less than 20 percent quartz in the QAPF fraction. Includes rocks defined modally in QAPF fields 9 and 10 (and their subdivisions)."@en ;
  rdfs:comment "dct:source--  LeMaitre et al. 2002"@en ;
  rdfs:label "dioritoid"@en ;
  rdfs:subClassOf gslth:intermediate_composition_igneous_rock ;
  rdfs:subClassOf gslth:phaneritic_igneous_rock ;
.
gslth:doleritic_rock
  a owl:Class ;
  rdfs:comment "Dark colored gabbroic (basaltic) or dioritic (andesitic) rock intermediate in grain size between basalt and gabbro and composed of plagioclase, pyroxene and opaque minerals; often with ophitic texture. Typically occurs as hypabyssal intrusions. Includes dolerite, microdiorite, diabase and microgabbro."@en ;
  rdfs:comment "dct:source--  Neuendorf et al 2005; LeMaitre et al. 2002; Gillespie and Styles 1999"@en ;
  rdfs:label "doleritic rock"@en ;
  rdfs:subClassOf gslth:igneous_rock ;
.
gslth:dolomitic_or_magnesian_sedimentary_material
  a owl:Class ;
  rdfs:comment "Carbonate sedimentary material of unspecified consolidation degree with a ratio of magnesium carbonate to calcite (plus aragonite) greater than 1 to 1. Includes dolomite sediment, dolostone, lime dolostone and magnesite-stone."@en ;
  rdfs:comment "dct:source--  after SLTTs 2004, Hallsworth and Knox 1999"@en ;
  rdfs:label "dolomitic or magnesian sedimentary material"@en ;
  rdfs:subClassOf gslth:carbonate_sedimentary_material ;
.
gslth:dolomitic_or_magnesian_sedimentary_rock
  a owl:Class ;
  rdfs:comment "Carbonate sedimentary rock with a ratio of magnesium carbonate to calcite (plus aragonite) greater than 1 to 1. Includes dolostone, lime dolostone and magnesite-stone."@en ;
  rdfs:comment "dct:source--  after SLTTs 2004, Hallsworth and Knox 1999"@en ;
  rdfs:label "dolomitic or magnesian sedimentary rock"@en ;
  rdfs:subClassOf gslth:carbonate_sedimentary_rock ;
  rdfs:subClassOf gslth:dolomitic_or_magnesian_sedimentary_material ;
.
gslth:dolomitic_sediment
  a owl:Class ;
  rdfs:comment "Carbonate sediment with a ratio of magnesium carbonate to calcite (plus aragonite) greater than 1 to 1."@en ;
  rdfs:comment "dct:source--  after SLTTs 2004, Hallsworth and Knox 1999"@en ;
  rdfs:label "dolomitic sediment"@en ;
  rdfs:subClassOf gslth:carbonate_sediment ;
  rdfs:subClassOf gslth:dolomitic_or_magnesian_sedimentary_material ;
.
gslth:dolostone
  a owl:Class ;
  a owl:NamedIndividual ;
  rdfs:comment "Pure carbonate sedimentary rock with a ratio of magnesium carbonate to calcite (plus aragonite) greater than 1 to 1."@en ;
  rdfs:comment "dct:source--  This vocabulary"@en ;
  rdfs:comment "skos:altLabel--  dolostone"@en ;
  rdfs:comment "skos:altLabel--  pure dolomitic or magnesian carbonate sedimentary rock"@en ;
  rdfs:label "dolomite"@en ;
  rdfs:subClassOf gslth:dolomitic_or_magnesian_sedimentary_rock ;
  rdfs:subClassOf gslth:pure_carbonate_sedimentary_rock ;
.
gslth:duricrust
  a owl:Class ;
  rdfs:comment "Rock forming a hard crust or layer at or near the Earth's surface at the time of formation, e.g. in the upper horizons of a soil, characterized by structures indicative of pedogenic origin."@en ;
  rdfs:comment "dct:source--  This vocabulary"@en ;
  rdfs:label "duricrust"@en ;
  rdfs:subClassOf gslth:composite_genesis_rock ;
  rdfs:subClassOf gslth:material_formed_in_surficial_environment ;
.
gslth:eclogite
  a owl:Class ;
  rdfs:comment "Metamorphic rock composed of 75 percent or more (by volume) omphacite and garnet, both of which are present as major constituents, the amount of neither of them being higher than 75 percent (by volume); the presence of plagioclase precludes classification as an eclogite."@en ;
  rdfs:comment "dct:source--  IUGS SCMR 2007 (http://www.bgs.ac.uk/SCMR/)"@en ;
  rdfs:label "eclogite"@en ;
  rdfs:subClassOf gslth:metamorphic_rock ;
.
gslth:evaporite
  a owl:Class ;
  rdfs:comment "Nonclastic sedimentary rock composed of at least 50 percent non-carbonate salts, including chloride, sulfate or borate minerals; formed through precipitation of mineral salts from a saline solution (non-carbonate salt rock)."@en ;
  rdfs:comment "dct:source--  Jackson 1997; SLTTs 2004"@en ;
  rdfs:label "evaporite"@en ;
  rdfs:subClassOf gslth:chemical_sedimentary_material ;
.
gslth:exotic_alkaline_rock
  a owl:Class ;
  rdfs:comment "Kimberlite, lamproite, or lamprophyre. Generally are potassic, mafic or ultramafic rocks. Olivine (commonly serpentinized in kimberlite), and phlogopite are significant constituents."@en ;
  rdfs:comment "dct:source--  based on LeMaitre et al. 2002"@en ;
  rdfs:label "exotic alkaline rock"@en ;
  rdfs:subClassOf gslth:exotic_composition_igneous_rock ;
.
gslth:exotic_composition_igneous_rock
  a owl:Class ;
  rdfs:comment "Rock with 'exotic' mineralogical, textural or field setting characteristics; typically dark colored, with abundant phenocrysts. Criteria include: presence of greater than 10 percent melilite or leucite, or presence of kalsilite, or greater than 50 percent carbonate minerals. Includes Carbonatite, Melilitic rock, Kalsilitic rocks, Kimberlite, Lamproite, Leucitic rock and Lamprophyres."@en ;
  rdfs:comment "dct:source--  Gillespie and Styles 1999; LeMaitre et al. 2002"@en ;
  rdfs:label "exotic composition igneous rock"@en ;
  rdfs:subClassOf gslth:igneous_rock ;
.
gslth:exotic_evaporite
  a owl:Class ;
  rdfs:comment "Category represents evaporite material that is not mostly gypsum/anhydrite or halite. These are generally not very common, thus the 'exotic' name"@en ;
  rdfs:comment "Evaporite that is not 50 percent halite or 50 percent gypsum or anhydrite."@en ;
  rdfs:comment "dct:source--  This vocabulary"@en ;
  rdfs:label "exotic evaporite"@en ;
  rdfs:subClassOf gslth:evaporite ;
.
gslth:fault_related_material
  a owl:Class ;
  rdfs:comment "Material formed as a result brittle faulting, composed of greater than 10 percent matrix; matrix is fine-grained material caused by tectonic grainsize reduction. Includes cohesive (cataclasite series) and non-cohesive (breccia-gouge series) material."@en ;
  rdfs:comment "dct:source--  This vocabulary; SLTTm 2004"@en ;
  rdfs:label "fault related material"@en ;
  rdfs:subClassOf gslth:composite_genesis_material ;
.
gslth:fine_grained_igneous_rock
  a owl:Class ;
  a owl:NamedIndividual ;
  rdfs:comment "Igneous rock in which the framework of the rock consists of crystals that are too small to determine mineralogy with the unaided eye; framework may include up to 50 percent glass. A significant percentage of the rock by volume may be phenocrysts. Includes rocks that are generally called volcanic rocks."@en ;
  rdfs:comment "Need to make decision as to whether devitrified glass should be considered glass or microcrystalline framework for purposes of categorization"@en ;
  rdfs:comment "dct:source--  Gillespie and Styles 1999; LeMaitre et al. 2002"@en ;
  rdfs:comment "skos:altLabel--  volcanic rock"@en ;
  rdfs:label "fine grained igneous rock"@en ;
  rdfs:subClassOf gslth:igneous_rock ;
.
gslth:foid_bearing_alkali_feldspar_syenite
  a owl:Class ;
  rdfs:comment "Alkali feldspar syenitic rock that contains 0-10 percent feldspathoid mineral and no quartz in the QAPF fraction. QAPF field 6'."@en ;
  rdfs:comment "dct:source--  LeMaitre et al. 2002"@en ;
  rdfs:label "foid bearing alkali feldspar syenite"@en ;
  rdfs:subClassOf gslth:alkali_feldspar_syenitic_rock ;
.
gslth:foid_bearing_alkali_feldspar_trachyte
  a owl:Class ;
  rdfs:comment "Alkali feldspar trachytic rock that contains no quartz and between 0 and 10 percent feldspathoid mineral in the QAPF fraction. QAPF field 6'."@en ;
  rdfs:comment "dct:source--  LeMaitre et al. 2002"@en ;
  rdfs:label "foid bearing alkali feldspar trachyte"@en ;
  rdfs:subClassOf gslth:alkali_feldspar_trachytic_rock ;
.
gslth:foid_bearing_anorthosite
  a owl:Class ;
  rdfs:comment "Anorthositic rock that contains between 0 and 10 percent feldspathoid mineral and no quartz in the QAPF fraction. QAPF field 10'."@en ;
  rdfs:comment "dct:source--  LeMaitre et al. 2002"@en ;
  rdfs:label "foid bearing anorthosite"@en ;
  rdfs:subClassOf gslth:anorthositic_rock ;
.
gslth:foid_bearing_diorite
  a owl:Class ;
  rdfs:comment "Dioritic rock that contains between 0 and 10 percent feldspathoid minerals in the QAPF fraction. QAPF field 10'."@en ;
  rdfs:comment "dct:source--  LeMaitre et al. 2002"@en ;
  rdfs:label "foid bearing diorite"@en ;
  rdfs:subClassOf gslth:dioritic_rock ;
.
gslth:foid_bearing_gabbro
  a owl:Class ;
  rdfs:comment "Gabbroic rock that contains 0-10 percent feldspathoid minerals and no quartz in the QAPF fraction. QAPF field 10'."@en ;
  rdfs:comment "dct:source--  LeMaitre et al. 2002"@en ;
  rdfs:label "foid bearing gabbro"@en ;
  rdfs:subClassOf gslth:gabbroic_rock ;
.
gslth:foid_bearing_latite
  a owl:Class ;
  rdfs:comment "Latitic rock that contains no quartz and between 0 and 10 percent feldspathoid minerals in the QAPF fraction. QAPF field 8'."@en ;
  rdfs:comment "dct:source--  LeMaitre et al. 2002"@en ;
  rdfs:label "foid bearing latite"@en ;
  rdfs:subClassOf gslth:latitic_rock ;
.
gslth:foid_bearing_monzodiorite
  a owl:Class ;
  rdfs:comment "Monzodioritic rock that contains between 0 and 10 percent feldspathoid mineral."@en ;
  rdfs:comment "dct:source--  LeMaitre et al. 2002"@en ;
  rdfs:label "foid bearing monzodiorite"@en ;
  rdfs:subClassOf gslth:monzodioritic_rock ;
.
gslth:foid_bearing_monzogabbro
  a owl:Class ;
  rdfs:comment "Monzogabbroic rock that contains 0 to 10 percent feldspathoid mineral in the QAPF fraction. QAPF field 9'."@en ;
  rdfs:comment "dct:source--  LeMaitre et al. 2002"@en ;
  rdfs:label "foid bearing monzogabbro"@en ;
  rdfs:subClassOf gslth:monzogabbroic_rock ;
.
gslth:foid_bearing_monzonite
  a owl:Class ;
  rdfs:comment "Monzonitic rock that contains 0-10 percent feldspathoid mineral and no quartz in the QAPF fraction. Includes rocks defined modally in QAPF Field 8'."@en ;
  rdfs:comment "dct:source--  LeMaitre et al. 2002"@en ;
  rdfs:label "foid bearing monzonite"@en ;
  rdfs:subClassOf gslth:monzonitic_rock ;
.
gslth:foid_bearing_syenite
  a owl:Class ;
  rdfs:comment "Syenitic rock that contains between 0 and 10 percent feldspathoid mineral and no quartz in the QAPF fraction. Defined modally in QAPF Field 7'."@en ;
  rdfs:comment "dct:source--  LeMaitre et al. 2002"@en ;
  rdfs:label "foid bearing syenite"@en ;
  rdfs:subClassOf gslth:syenitic_rock ;
.
gslth:foid_bearing_trachyte
  a owl:Class ;
  rdfs:comment "Trachytic rock that contains between 0 and 10 percent feldspathoid in the QAPF fraction, and no quartz. QAPF field 7'."@en ;
  rdfs:comment "dct:source--  LeMaitre et al. 2002"@en ;
  rdfs:label "foid bearing trachyte"@en ;
  rdfs:subClassOf gslth:trachytic_rock ;
.
gslth:foid_diorite
  a owl:Class ;
  rdfs:comment "Foid dioritoid in which the plagioclase to total feldspar ratio is greater than 0.9. Includes rocks defined modally in QAPF field 14."@en ;
  rdfs:comment "dct:source--  LeMaitre et al. 2002"@en ;
  rdfs:label "foid diorite"@en ;
  rdfs:subClassOf gslth:foid_dioritoid ;
.
gslth:foid_dioritoid
  a owl:Class ;
  rdfs:comment "Phaneritic crystalline igneous rock in which M is less than 90, the plagioclase to total feldspar ratio is greater than 0.5, feldspathoid minerals form 10-60 percent of the QAPF fraction, plagioclase has anorthite content less than 50 percent. These rocks typically contain large amounts of mafic minerals. Includes rocks defined modally in QAPF fields 13 and 14."@en ;
  rdfs:comment "dct:source--  LeMaitre et al. 2002"@en ;
  rdfs:label "foid dioritoid"@en ;
  rdfs:subClassOf gslth:phaneritic_igneous_rock ;
.
gslth:foid_gabbro
  a owl:Class ;
  rdfs:comment "Foid gabbroid that has a plagioclase to total feldspar ratio greater than 0.9. Includes rocks defined modally in QAPF field 14."@en ;
  rdfs:comment "dct:source--  LeMaitre et al. 2002"@en ;
  rdfs:label "foid gabbro"@en ;
  rdfs:subClassOf gslth:foid_gabbroid ;
.
gslth:foid_gabbroid
  a owl:Class ;
  rdfs:comment "Phaneritic crystalline igneous rock in which M is less than 90, the plagioclase to total feldspar ratio is greater than 0.5, feldspathoids form 10-60 percent of the QAPF fraction, and plagioclase has anorthite content greater than 50 percent. These rocks typically contain large amounts of mafic minerals. Includes rocks defined modally in QAPF fields 13 and 14."@en ;
  rdfs:comment "dct:source--  LeMaitre et al. 2002"@en ;
  rdfs:label "foid gabbroid"@en ;
  rdfs:subClassOf gslth:phaneritic_igneous_rock ;
.
gslth:foid_monzodiorite
  a owl:Class ;
  rdfs:comment "Foid dioritoid in which the plagioclase to total feldspar ratio is between 0.1 and 0.9. Includes rocks defined modally in QAPF field 13."@en ;
  rdfs:comment "dct:source--  LeMaitre et al. 2002"@en ;
  rdfs:label "foid monzodiorite"@en ;
  rdfs:subClassOf gslth:foid_dioritoid ;
.
gslth:foid_monzogabbro
  a owl:Class ;
  rdfs:comment "Foid gabbroid that has a plagioclase to total feldspar ratio between 0.5 and 0.9. Includes rocks defined modally in QAPF field 13."@en ;
  rdfs:comment "dct:source--  LeMaitre et al. 2002"@en ;
  rdfs:label "foid monzogabbro"@en ;
  rdfs:subClassOf gslth:foid_gabbroid ;
.
gslth:foid_monzosyenite
  a owl:Class ;
  rdfs:comment "Foid syenitoid rock that has a plagioclase to total feldspar ratio of between 0.1 and 0.5. Includes rocks defined modally in QAPF Field 12."@en ;
  rdfs:comment "dct:source--  LeMaitre et al. 2002"@en ;
  rdfs:label "foid monzosyenite"@en ;
  rdfs:subClassOf gslth:foid_syenitoid ;
.
gslth:foid_syenite
  a owl:Class ;
  rdfs:comment "Foid syenitoid that has a plagioclase to total feldspar ratio of less than 0.1. Includes rocks defined modally in QAPF field 11."@en ;
  rdfs:comment "dct:source--  LeMaitre et al. 2002"@en ;
  rdfs:label "foid syenite"@en ;
  rdfs:subClassOf gslth:foid_syenitoid ;
.
gslth:foid_syenitoid
  a owl:Class ;
  rdfs:comment "Phaneritic crystalline igneous rock with M less than 90, contains between 10 and 60 percent feldspathoid mineral in the QAPF fraction, and has a plagioclase to total feldspar ratio less than 0.5. Includes QAPF fields 11 and 12."@en ;
  rdfs:comment "dct:source--  LeMaitre et al. 2002"@en ;
  rdfs:label "foid syenitoid"@en ;
  rdfs:subClassOf gslth:phaneritic_igneous_rock ;
.
gslth:foidite
  a owl:Class ;
  rdfs:comment "Foiditoid that contains greater than 90 percent feldspathoid minerals in the QAPF fraction."@en ;
  rdfs:comment "dct:source--  LeMaitre et al. 2002"@en ;
  rdfs:label "foidite"@en ;
  rdfs:subClassOf gslth:foiditoid ;
.
gslth:foiditoid
  a owl:Class ;
  a owl:NamedIndividual ;
  rdfs:comment "Fine grained crystalline rock containing less than 90 percent mafic minerals and more than 60 percent feldspathoid minerals in the QAPF fraction. Includes rocks defined modally in QAPF field 15 or chemically in TAS field F."@en ;
  rdfs:comment "dct:source--  LeMaitre et al. 2002"@en ;
  rdfs:comment "skos:altLabel--  foidite (sensu lato)"@en ;
  rdfs:comment "skos:altLabel--  foiditic rock"@en ;
  rdfs:label "foiditoid"@en ;
  rdfs:subClassOf gslth:fine_grained_igneous_rock ;
.
gslth:foidolite
  a owl:Class ;
  rdfs:comment "Phaneritic crystalline rock containing more than 60 percent feldspathoid minerals in the QAPF fraction. Includes rocks defined modally in QAPF field 15"@en ;
  rdfs:comment "dct:source--  LeMaitre et al. 2002"@en ;
  rdfs:label "foidolite"@en ;
  rdfs:subClassOf gslth:phaneritic_igneous_rock ;
.
gslth:foliated_metamorphic_rock
  a owl:Class ;
  rdfs:comment "Metamorphic rock in which 10 percent or more of the contained mineral grains are elements in a planar or linear fabric. Cataclastic or glassy character precludes classification with this concept."@en ;
  rdfs:comment "dct:source--  based on NADM SLTT metamorphic"@en ;
  rdfs:label "foliated metamorphic rock"@en ;
  rdfs:subClassOf gslth:metamorphic_rock ;
.
gslth:fragmental_igneous_material
  a owl:Class ;
  rdfs:comment "dct:source--  CGI concept definition task group"@en ;
  rdfs:comment "igneous_material of unspecified consolidation state in which greater than 75 percent of the rock consists of fragments produced as a result of igneous rock-forming process."@en ;
  rdfs:label "fragmental igneous material"@en ;
  rdfs:subClassOf gslth:igneous_material ;
.
gslth:fragmental_igneous_rock
  a owl:Class ;
  rdfs:comment "Igneous rock in which greater than 75 percent of the rock consists of fragments produced as a result of igneous rock-forming process. Includes pyroclastic rocks, autobreccia associated with lava flows and intrusive breccias. Excludes deposits reworked by epiclastic processes (see Tuffite)"@en ;
  rdfs:comment "dct:source--  This vocabulary"@en ;
  rdfs:label "fragmental igneous rock"@en ;
  rdfs:subClassOf gslth:fragmental_igneous_material ;
  rdfs:subClassOf gslth:igneous_rock ;
.
gslth:framestone
  a owl:Class ;
  rdfs:comment "Carbonate reef rock consisting of a rigid framework of colonies, shells or skeletons, with internal cavities filled with fine sediment; usually created through the activities of colonial organisms."@en ;
  rdfs:comment "dct:source--  Hallsworth and Knox 1999; SLTTs 2004, Table 15-3-1"@en ;
  rdfs:label "framestone"@en ;
  rdfs:subClassOf gslth:carbonate_sedimentary_rock ;
.
gslth:gabbro
  a owl:Class ;
  rdfs:comment "Gabbroic rock that contains between 0 and 5 percent quartz and no feldspathoid mineral in the QAPF fraction. Includes rocks defined modally in QAPF Field 10 as gabbro."@en ;
  rdfs:comment "Note that this category includes gabbro (sensu stricto) of LeMaitre et al. 2002, but is broader, including the other rock types defined by orthopyroxene-clinopyroxene-olivine-hornblende mineral ratios."@en ;
  rdfs:comment "dct:source--  LeMaitre et al. 2002"@en ;
  rdfs:label "gabbro"@en ;
  rdfs:subClassOf gslth:gabbroic_rock ;
.
gslth:gabbroic_rock
  a owl:Class ;
  rdfs:comment "Gabbroid that has a plagioclase to total feldspar ratio greater than 0.9 in the QAPF fraction. Includes QAPF fields 10*, 10, and 10'. This category includes the various categories defined in LeMaitre et al. (2002) based on the mafic mineralogy, but apparently not subdivided based on the quartz/feldspathoid content."@en ;
  rdfs:comment "dct:source--  LeMaitre et al. 2002"@en ;
  rdfs:label "gabbroic rock"@en ;
  rdfs:subClassOf gslth:basic_igneous_rock ;
  rdfs:subClassOf gslth:gabbroid ;
.
gslth:gabbroid
  a owl:Class ;
  rdfs:comment "Phaneritic crystalline igneous rock that contains less than 90 percent mafic minerals, and up to 20 percent quartz or up to 10 percent feldspathoid in the QAPF fraction. The ratio of plagioclase to total feldspar is greater than 0.65, and anorthite content of the plagioclase is greater than 50 percent. Includes rocks defined modally in QAPF fields 9 and 10 and their subdivisions."@en ;
  rdfs:comment "dct:source--  LeMaitre et al. 2002"@en ;
  rdfs:label "gabbroid"@en ;
  rdfs:subClassOf gslth:phaneritic_igneous_rock ;
.
gslth:generic_conglomerate
  a owl:Class ;
  rdfs:comment "Sedimentary rock composed of at least 30 percent rounded to subangular fragments larger than 2 mm in diameter; typically contains finer grained material in interstices between larger fragments. If more than 15 percent of the fine grained matrix is of indeterminant clastic or diagenetic origin and the fabric is matrix supported, may also be categorized as wackestone. If rock has unsorted or poorly sorted texture with a wide range of particle sizes, may also be categorized as diamictite."@en ;
  rdfs:comment "dct:source--  Neuendorf et al. 2005; SLTTs 2004; particle sizes defined from Krumbein phi scale (W C Krumbein and L L Sloss, Stratigraphy and Sedimentation, 2nd edition, Freeman, San Francisco, 1963; Krumbein and Pettijohn, 1938, Manual of Sedimentary Petrography: New York, Appleton Century Co., Inc.)"@en ;
  rdfs:label "generic conglomerate"@en ;
  rdfs:subClassOf gslth:sedimentary_rock ;
.
gslth:generic_mudstone
  a owl:Class ;
  rdfs:comment "Distinction of intrabasinal, diagenetic, or clastic genesis for very fine-grained carbonate minerals is so interpretive that it is proposed to not define the mudstone category based on intrabasinal vs epiclastic distinction required for clastic sedimentary rock-carbonate sedimentary rock categorization in this system. Schnurrenberger, D., Russell, J. and Kelts, K., 2003, Classification of lacustrine sediments based on sedimentary components: Journal of Paleolimnology, v.29, p141-154."@en ;
  rdfs:comment "Sedimentary rock consisting of less than 30 percent gravel-size (2 mm) particles and with a mud to sand ratio greater than 1. Clasts may be of any composition or origin."@en ;
  rdfs:comment "dct:source--  Pettijohn et al. 1987 referenced in Hallsworth and Knox 1999; extrapolated from Folk, 1954, Figure 1a; particle sizes defined from Krumbein phi scale (W C Krumbein and L L Sloss, Stratigraphy and Sedimentation, 2nd edition, Freeman, San Francisco, 1963; Krumbein and Pettijohn, 1938, Manual of Sedimentary Petrography: New York, Appleton Century Co., Inc.)"@en ;
  rdfs:label "generic mudstone"@en ;
  rdfs:subClassOf gslth:sedimentary_rock ;
.
gslth:generic_sandstone
  a owl:Class ;
  rdfs:comment "Sedimentary rock in which less than 30 percent of particles are greater than 2 mm in diameter (gravel) and the sand to mud ratio is at least 1."@en ;
  rdfs:comment "dct:source--  SLTTs 2004; Neuendorf et al. 2005; particle sizes defined from Krumbein phi scale (W C Krumbein and L L Sloss, Stratigraphy and Sedimentation, 2nd edition, Freeman, San Francisco, 1963; Krumbein and Pettijohn, 1938, Manual of Sedimentary Petrography: New York, Appleton Century Co., Inc.)"@en ;
  rdfs:label "generic sandstone"@en ;
  rdfs:subClassOf gslth:sedimentary_rock ;
.
gslth:glass_rich_igneous_rock
  a owl:Class ;
  rdfs:comment "Igneous rock that contains greater than 50 percent massive glass."@en ;
  rdfs:comment "dct:source--  This vocabulary, based on Gillespie and Styles 1999"@en ;
  rdfs:label "glass rich igneous rock"@en ;
  rdfs:subClassOf gslth:igneous_rock ;
.
gslth:glassy_igneous_rock
  a owl:Class ;
  rdfs:comment "Change percent criteria from 90 to 80 percent for version 2009."@en ;
  rdfs:comment "Igneous rock that consists of greater than 80 percent massive glass."@en ;
  rdfs:comment "Note that this category is used for massive glassy rocks. Much of the pyroclastic material in a pyroclastic rock may be composed of glass, but the rock is named based on its fragmental nature."@en ;
  rdfs:comment "dct:source--  This vocabulary"@en ;
  rdfs:label "glassy igneous rock"@en ;
  rdfs:subClassOf gslth:glass_rich_igneous_rock ;
.
gslth:glaucophane_lawsonite_epidote_metamorphic_rock
  a owl:Class ;
  a owl:NamedIndividual ;
  rdfs:comment "A metamorphic rock of roughly basaltic composition, defined by the presence of glaucophane with lawsonite or epidote. Other minerals that may be present include jadeite, albite, chlorite, garnet, and muscovite (phengitic white mica). Typically fine-grained, dark colored. Category for rocks commonly referred to as blueschist."@en ;
  rdfs:comment "Fabric is weakly developed in this rock in many cases, so the fabric categories 'foliated metamorphic rock, 'schist' or 'granofels' may apply."@en ;
  rdfs:comment "dct:source--  This vocabulary"@en ;
  rdfs:comment "skos:altLabel--  blauschiefer"@de ;
  rdfs:label "glaucophane lawsonite epidote metamorphic rock"@en ;
  rdfs:label "glaukophanschiefer"@de ;
  rdfs:subClassOf gslth:metamorphic_rock ;
.
gslth:gneiss
  a owl:Class ;
  rdfs:comment "Foliated metamorphic rock with bands or lenticles rich in granular minerals alternating with bands or lenticles rich in minerals with a flaky or elongate prismatic habit. Mylonitic foliation or well developed, continuous schistosity (greater than 50 percent of the rock consists of grains participate in a planar or linear fabric) precludes classification with this concept."@en ;
  rdfs:comment "dct:source--  Neuendorf et al. 2005"@en ;
  rdfs:label "gneiss"@en ;
  rdfs:subClassOf gslth:foliated_metamorphic_rock ;
.
gslth:grainstone
  a owl:Class ;
  a owl:NamedIndividual ;
  rdfs:comment "Carbonate sedimentary rock with recognizable depositional fabric that is grain-supported, and constituent particles are of intrabasinal origin; contains little or no mud matrix. Distinction from sandstone is based on interpretation of intrabasinal origin of clasts and grain-supported fabric, but grainstone definition does not include a grain size criteria."@en ;
  rdfs:comment "dct:source--  Dunham 1962"@en ;
  rdfs:comment "skos:altLabel--  carbonate grainstone"@en ;
  rdfs:label "grainstone"@en ;
  rdfs:subClassOf gslth:carbonate_sedimentary_rock ;
.
gslth:granite
  a owl:Class ;
  rdfs:comment "Phaneritic crystalline rock consisting of quartz, alkali feldspar and plagioclase (typically sodic) in variable amounts, usually with biotite and/or hornblende. Includes rocks defined modally in QAPF Field 3."@en ;
  rdfs:comment "dct:source--  LeMaitre et al. 2002"@en ;
  rdfs:label "granite"@en ;
  rdfs:subClassOf gslth:granitoid ;
.
gslth:granitoid
  a owl:Class ;
  a owl:NamedIndividual ;
  rdfs:comment "Phaneritic crystalline igneous rock consisting of quartz, alkali feldspar and/or plagioclase. Includes rocks defined modally in QAPF fields 2, 3, 4 and 5 as alkali feldspar granite, granite, granodiorite or tonalite."@en ;
  rdfs:comment "dct:source--  LeMaitre et al. 2002"@en ;
  rdfs:comment "skos:altLabel--  granitic rock"@en ;
  rdfs:label "granitoid"@en ;
  rdfs:subClassOf gslth:acidic_igneous_rock ;
  rdfs:subClassOf gslth:phaneritic_igneous_rock ;
.
gslth:granodiorite
  a owl:Class ;
  rdfs:comment "Phaneritic crystalline rock consisting essentially of quartz, sodic plagioclase and lesser amounts of alkali feldspar with minor hornblende and biotite. Includes rocks defined modally in QAPF field 4."@en ;
  rdfs:comment "dct:source--  LeMaitre et al. 2002"@en ;
  rdfs:label "granodiorite"@en ;
  rdfs:subClassOf gslth:granitoid ;
.
gslth:granofels
  a owl:Class ;
  rdfs:comment "Metamorphic rock with granoblastic fabric and very little or no foliation (less than 10 percent of the mineral grains in the rock are elements in a planar or linear fabric). Grainsize not specified."@en ;
  rdfs:comment "dct:source--  SLTTm 2004"@en ;
  rdfs:label "granofels"@en ;
  rdfs:subClassOf gslth:metamorphic_rock ;
.
gslth:granulite
  a owl:Class ;
  rdfs:comment "Metamorphic rock of high metamorphic grade in which Fe-Mg silicate minerals are dominantly hydroxl-free; feldspar must be present, and muscovite is absent; rock contains less than 90 percent mafic minerals, less than 75 percent calcite and/or dolomite, less than 75 percent quartz, less than 50 percent iron-bearing minerals (hematite, magnetite, limonite-group, siderite, iron-sulfides), and less than 50 percent calc-silicate minerals."@en ;
  rdfs:comment "Wimmenauer (1985) requires granulite to consist of at least 20 percent feldspar. Garnet is frequently present; some hornblende or biotite may be present. The rock has a granoblastic texture and gneissose to massive structure; grain size and fabric may be variable on a decimetric scale. Foliation is less well developed than in rock that would typically be called gneiss. The minerals present in a granulite vary depending on the protolith and the temperature and pressure conditions experienced during metamorphism. According to Fettes and Desmons (2007) the main calc-silicate minerals are calcic garnet, calcic plagioclase, calcic scapolite, diopside-hedenbergite, epidote group minerals, hydrogrossular, johannsenite, prehnite, pumpellyite, titanite, vesuvianite, wollastonite. Note that the shale and siltstone categories may apply to any of the mineralogically defined mudstone categories."@en ;
  rdfs:comment "dct:source--  Fettes and Desmons (2007). See also Wimmenauer (1985), Winkler (1979) (D.R. Bowes (1989), The Encyclopedia of Igneous and Metamorphic Petrology; Van Nostrand Reinhold ISBN: 0-442-20623-2 ; wikipedia, http://en.wikipedia.org/wiki/Granulite accessed 5/30/09"@en ;
  rdfs:label "granulite"@en ;
  rdfs:subClassOf gslth:metamorphic_rock ;
.
gslth:gravel
  a owl:Class ;
  rdfs:comment "Clastic sediment containing greater than 30 percent gravel-size particles (greater than 2.0 mm diameter). Gravel in which more than half of the particles are of epiclastic origin"@en ;
  rdfs:comment "dct:source--  definition of gravel from SLTTs 2004; particle sizes defined from Krumbein phi scale (W C Krumbein and L L Sloss, Stratigraphy and Sedimentation, 2nd edition, Freeman, San Francisco, 1963; Krumbein and Pettijohn, 1938, Manual of Sedimentary Petrography: New York, Appleton Century Co., Inc.)"@en ;
  rdfs:label "gravel"@en ;
  rdfs:subClassOf gslth:clastic_sediment ;
  rdfs:subClassOf gslth:gravel_size_sediment ;
.
gslth:gravel_size_sediment
  a owl:Class ;
  rdfs:comment "Sediment containing greater than 30 percent gravel-size particles (greater than 2.0 mm diameter). Composition or gensis of clasts not specified."@en ;
  rdfs:comment "dct:source--  SLTTs 2004; particle sizes defined from Krumbein phi scale (W C Krumbein and L L Sloss, Stratigraphy and Sedimentation, 2nd edition, Freeman, San Francisco, 1963; Krumbein and Pettijohn, 1938, Manual of Sedimentary Petrography: New York, Appleton Century Co., Inc.)"@en ;
  rdfs:label "gravel size sediment"@en ;
  rdfs:subClassOf gslth:sediment ;
.
gslth:high_magnesium_fine_grained_igneous_rocks
  a owl:Class ;
  rdfs:comment "dct:source--  LeMaitre et al. 2002"@en ;
  rdfs:comment "fine-grained igneous rock that contains unusually high concentration of MgO. For rocks that contain greater than 52 percent silica, MgO must be greater than 8 percent. For rocks containing less than 52 percent silica, MgO must be greater than 12 percent."@en ;
  rdfs:label "high magnesium fine grained igneous rock"@en ;
  rdfs:subClassOf gslth:fine_grained_igneous_rock ;
.
gslth:hornblendite
  a owl:Class ;
  rdfs:comment "Ultramafic rock that consists of greater than 40 percent hornblende plus pyroxene and has a hornblende to pyroxene ratio greater than 1. Includes olivine hornblendite, olivine-pyroxene hornblendite, pyroxene hornblendite, and hornblendite."@en ;
  rdfs:comment "dct:source--  LeMaitre et al. 2002"@en ;
  rdfs:label "hornblendite"@en ;
  rdfs:subClassOf gslth:phaneritic_igneous_rock ;
  rdfs:subClassOf gslth:ultramafic_igneous_rock ;
.
gslth:hornfels
  a owl:Class ;
  rdfs:comment "Granofels formed by contact metamorphism, composed of a mosaic of equidimensional grains in a characteristically granoblastic or decussate matrix; porphyroblasts or relict phenocrysts may be present. Typically fine grained."@en ;
  rdfs:comment "dct:source--  IUGS SCMR 2007 (http://www.bgs.ac.uk/SCMR/)"@en ;
  rdfs:label "hornfels"@en ;
  rdfs:subClassOf gslth:granofels ;
.
gslth:hybrid_sediment
  a owl:Class ;
  rdfs:comment "Sediment that does not fit any of the other sediment composition/genesis categories. Sediment consisting of three or more components which form more than 5 percent but less than 50 precent of the material."@en ;
  rdfs:comment "dct:source--  Hallsworth and Knox, 1999"@en ;
  rdfs:label "hybrid sediment"@en ;
  rdfs:subClassOf gslth:sediment ;
.
gslth:hybrid_sedimentary_rock
  a owl:Class ;
  rdfs:comment "Sedimentary rock that does not fit any of the other composition/genesis categories. Sedimentary rock consisting of three or more components which form more than 5 percent but less than 50 precent of the material."@en ;
  rdfs:comment "dct:source--  Hallsworth and Knox, 1999"@en ;
  rdfs:label "hybrid sedimentary rock"@en ;
  rdfs:subClassOf gslth:sedimentary_rock ;
.
gslth:igneous_material
  a owl:Class ;
  rdfs:comment "Earth material formed as a result of igneous processes, eg. intrusion and cooling of magma in the crust, volcanic eruption."@en ;
  rdfs:comment "dct:source--  This vocabulary"@en ;
  rdfs:label "igneous material"@en ;
  rdfs:subClassOf gslth:compound_material ;
.
gslth:igneous_rock
  a owl:Class ;
  rdfs:comment "dct:source--  Neuendorf et al 2005"@en ;
  rdfs:comment "rock formed as a result of igneous processes, for example intrusion and cooling of magma in the crust, or volcanic eruption."@en ;
  rdfs:label "igneous rock"@en ;
  rdfs:subClassOf gslth:igneous_material ;
  rdfs:subClassOf gslth:rock ;
.
gslth:impact_generated_material
  a owl:Class ;
  rdfs:comment "Material that contains features indicative of shock metamorphism, such as microscopic planar deformation features within grains or shatter cones, interpreted to be the result of extraterrestrial bolide impact. Includes breccias and melt rocks."@en ;
  rdfs:comment "dct:source--  Stöffler and Grieve 2007; Jackson 1997"@en ;
  rdfs:label "impact generated material"@en ;
  rdfs:subClassOf gslth:composite_genesis_material ;
.
gslth:impure_calcareous_carbonate_sediment
  a owl:Class ;
  a owl:NamedIndividual ;
  rdfs:comment "Carbonate sediment in which between 50 and 90 percent of the constituents are composed of one (or more) of the carbonate minerals in particles of intrabasinal origin, and a calcite (plus aragonite) to dolomite ratio greater than 1 to 1."@en ;
  rdfs:comment "dct:source--  This vocabulary"@en ;
  rdfs:comment "skos:altLabel--  calcareous marl"@en ;
  rdfs:label "impure calcareous carbonate sediment"@en ;
  rdfs:subClassOf gslth:calcareous_carbonate_sediment ;
  rdfs:subClassOf gslth:impure_carbonate_sediment ;
.
gslth:impure_carbonate_sediment
  a owl:Class ;
  a owl:NamedIndividual ;
  rdfs:comment "Carbonate sediment in which between 50 and 90 percent of the constituents are composed of one (or more) of the carbonate minerals in particles of intrabasinal origin."@en ;
  rdfs:comment "dct:source--  This vocabulary"@en ;
  rdfs:comment "skos:altLabel--  marl"@en ;
  rdfs:label "impure carbonate sediment"@en ;
  rdfs:subClassOf gslth:carbonate_sediment ;
.
gslth:impure_carbonate_sedimentary_rock
  a owl:Class ;
  a owl:NamedIndividual ;
  rdfs:comment "Sedimentary rock in which between 50 and 90 percent of the primary and/or recrystallized constituents are composed of carbonate minerals."@en ;
  rdfs:comment "dct:source--  This vocabulary"@en ;
  rdfs:comment "skos:altLabel--  marlstone"@en ;
  rdfs:label "impure carbonate sedimentary rock"@en ;
  rdfs:subClassOf gslth:carbonate_sedimentary_rock ;
.
gslth:impure_dolomitic_sediment
  a owl:Class ;
  a owl:NamedIndividual ;
  rdfs:comment "Carbonate sediment in which between 50 and 90 percent of the constituents are composed of one (or more) of the carbonate minerals in particles of intrabasinal origin, and the ratio of magnesium carbonate to calcite (plus aragonite) greater than 1 to 1."@en ;
  rdfs:comment "dct:source--  This vocabulary"@en ;
  rdfs:comment "skos:altLabel--  dolomitic marl"@en ;
  rdfs:label "impure dolomitic sediment"@en ;
  rdfs:subClassOf gslth:dolomitic_sediment ;
  rdfs:subClassOf gslth:impure_carbonate_sediment ;
.
gslth:impure_dolostone
  a owl:Class ;
  a owl:NamedIndividual ;
  rdfs:comment "Impure carbonate sedimentary rock with a ratio of magnesium carbonate to calcite (plus aragonite) greater than 1 to 1."@en ;
  rdfs:comment "dct:source--  This vocabulary"@en ;
  rdfs:comment "skos:altLabel--  dolomitic marlstone"@en ;
  rdfs:comment "skos:altLabel--  impure dolomitic or magnesian carbonate sedimentary rock"@en ;
  rdfs:comment "skos:altLabel--  impure dolostone"@en ;
  rdfs:label "impure dolomite"@en ;
  rdfs:subClassOf gslth:dolomitic_or_magnesian_sedimentary_rock ;
  rdfs:subClassOf gslth:impure_carbonate_sedimentary_rock ;
.
gslth:impure_limestone
  a owl:Class ;
  a owl:NamedIndividual ;
  rdfs:comment "Impure carbonate sedimentary rock with a calcite (plus aragonite) to dolomite ratio greater than 1 to 1."@en ;
  rdfs:comment "dct:source--  This vocabulary"@en ;
  rdfs:comment "skos:altLabel--  calcareous marlstone"@en ;
  rdfs:label "impure limestone"@en ;
  rdfs:subClassOf gslth:calcareous_carbonate_sedimentary_rock ;
  rdfs:subClassOf gslth:impure_carbonate_sedimentary_rock ;
.
gslth:intermediate_composition_igneous_material
  a owl:Class ;
  rdfs:comment "Igneous material with between 52 and 63 percent SiO2."@en ;
  rdfs:comment "dct:source--  after LeMaitre et al. 2002"@en ;
  rdfs:label "intermediate composition igneous material"@en ;
  rdfs:subClassOf gslth:igneous_material ;
.
gslth:intermediate_composition_igneous_rock
  a owl:Class ;
  rdfs:comment "Igneous rock with between 52 and 63 percent SiO2."@en ;
  rdfs:comment "dct:source--  after LeMaitre et al. 2002"@en ;
  rdfs:label "intermediate composition igneous rock"@en ;
  rdfs:subClassOf gslth:igneous_rock ;
  rdfs:subClassOf gslth:intermediate_composition_igneous_material ;
.
gslth:iron_rich_sediment
  a owl:Class ;
  rdfs:comment "Sediment that consists of at least 50 percent iron-bearing minerals (hematite, magnetite, limonite-group, siderite, iron-sulfides), as determined by hand-lens or petrographic analysis. Corresponds to a rock typically containing 15 percent iron by weight."@en ;
  rdfs:comment "dct:source--  SLTTs 2004"@en ;
  rdfs:label "iron rich sediment"@en ;
  rdfs:subClassOf gslth:iron_rich_sedimentary_material ;
  rdfs:subClassOf gslth:sediment ;
.
gslth:iron_rich_sedimentary_material
  a owl:Class ;
  rdfs:comment "Sedimentary material of unspecified consolidation state that consists of at least 50 percent iron-bearing minerals (hematite, magnetite, limonite-group, siderite, iron-sulfides), as determined by hand-lens or petrographic analysis. Corresponds to a rock typically containing 15 percent iron by weight."@en ;
  rdfs:comment "dct:source--  SLTTs 2004"@en ;
  rdfs:label "iron rich sedimentary material"@en ;
  rdfs:subClassOf gslth:chemical_sedimentary_material ;
.
gslth:iron_rich_sedimentary_rock
  a owl:Class ;
  rdfs:comment "Sedimentary rock that consists of at least 50 percent iron-bearing minerals (hematite, magnetite, limonite-group, siderite, iron-sulfides), as determined by hand-lens or petrographic analysis. Corresponds to a rock typically containing 15 percent iron by weight."@en ;
  rdfs:comment "dct:source--  Hallsworth and Knox 1999; SLTTs 2004"@en ;
  rdfs:label "iron rich sedimentary rock"@en ;
  rdfs:subClassOf gslth:iron_rich_sedimentary_material ;
  rdfs:subClassOf gslth:sedimentary_rock ;
.
gslth:kalsilitic_and_melilitic_rock
  a owl:Class ;
  rdfs:comment "Igneous rock containing greater than 10 percent melilite or kalsilite. Typically undersaturated, ultrapotassic (kalsilitic rocks) or calcium-rich (melilitic rocks) mafic or ultramafic rocks."@en ;
  rdfs:comment "dct:source--  based on LeMaitre et al. 2002"@en ;
  rdfs:label "kalsilitic and melilitic rocks"@en ;
  rdfs:subClassOf gslth:exotic_composition_igneous_rock ;
.
gslth:komatiitic_rock
  a owl:Class ;
  rdfs:comment "Ultramafic, magnesium-rich volcanic rock, typically with spinifex texture of intergrown skeletal and bladed olivine and pyroxene crystals set in abundant glass. Includes komatiite and meimechite."@en ;
  rdfs:comment "dct:source--  LeMaitre et al. 2002"@en ;
  rdfs:label "komatiitic rock"@en ;
  rdfs:subClassOf gslth:high_magnesium_fine_grained_igneous_rocks ;
  rdfs:subClassOf gslth:ultramafic_igneous_rock ;
.
gslth:latite
  a owl:Class ;
  rdfs:comment "Latitic rock that contains between 0 and 5 percent quartz and no feldspathoid in the QAPF fraction. QAPF field 8."@en ;
  rdfs:comment "dct:source--  LeMaitre et al. 2002"@en ;
  rdfs:label "latite"@en ;
  rdfs:subClassOf gslth:latitic_rock ;
.
gslth:latitic_rock
  a owl:Class ;
  rdfs:comment "Trachytoid that has a plagioclase to total feldspar ratio between 0.35 and 0.65. QAPF fields 8, 8' and 8*."@en ;
  rdfs:comment "dct:source--  LeMaitre et al. 2002"@en ;
  rdfs:label "latitic rock"@en ;
  rdfs:subClassOf gslth:trachytoid ;
.
gslth:lignite
  a owl:Class ;
  a owl:NamedIndividual ;
  rdfs:comment "Coal that has a gross calorific value less than 24 MJ/kg (determined in conformance with ISO 1928), and vitrinite mean random reflectance less than 0.6% (determined in conformance with ISO 7404-5). Gross calorific value is recalculated to a moist, ash free basis using bed moisture (determined according to ISO 1015 or ISO 5068). Includes all low-rank coals, including sub-bitiminous coal. A consolidated, dull, soft brown to black coal having many readily discernible plant fragments set in a finer grained organic matrix. Tends to crack and fall apart on drying. Operationally sub-bituminous and bitiminous coal are qualitatively distinguished based on brown streak for sub-bitiminous coal and black streak for bituminous coal."@en ;
  rdfs:comment "dct:source--  Economic commission for Europe, committee on Sustainable Energy- United Nations (ECE-UN), 1998, International Classification of in-Seam Coals: Energy 19, 41 pp."@en ;
  rdfs:comment "skos:altLabel--  low rank coal"@en ;
  rdfs:label "lignite"@en ;
  rdfs:subClassOf gslth:coal ;
.
gslth:limestone
  a owl:Class ;
  rdfs:comment "Pure carbonate sedimentary rock with a calcite (plus aragonite) to dolomite ratio greater than 1 to 1. Includes limestone and dolomitic limestone."@en ;
  rdfs:comment "dct:source--  This vocabulary"@en ;
  rdfs:label "limestone"@en ;
  rdfs:subClassOf gslth:calcareous_carbonate_sedimentary_rock ;
  rdfs:subClassOf gslth:pure_carbonate_sedimentary_rock ;
.
gslth:marble
  a owl:Class ;
  rdfs:comment "Metamorphic rock consisting of greater than 75 percent fine- to coarse-grained recrystallized calcite and/or dolomite; usually with a granoblastic, saccharoidal texture."@en ;
  rdfs:comment "dct:source--  IUGS SCMR 2007 (http://www.bgs.ac.uk/SCMR/), SLTTm1.0 2004"@en ;
  rdfs:label "marble"@en ;
  rdfs:subClassOf gslth:metamorphic_rock ;
.
gslth:material_formed_in_surficial_environment
  a owl:Class ;
  rdfs:comment "Material that is the product of weathering processes operating on pre-existing rocks or deposits, analogous to hydrothermal or metasomatic rocks, but formed at ambient Earth surface temperature and pressure."@en ;
  rdfs:comment "dct:source--  This vocabulary"@en ;
  rdfs:label "material formed in surficial environment"@en ;
  rdfs:subClassOf gslth:composite_genesis_material ;
.
gslth:metamorphic_rock
  a owl:Class ;
  rdfs:comment "Robertson (1999) defines the boundary between diagenesis and metamorphism in sedimentary rocks as follows: “…the boundary between diagenesis and metamorphism is somewhat arbitrary and strongly dependent on the lithologies involved. For example changes take place in organic materials at lower temperatures than in rocks dominated by silicate minerals. In mudrocks, a white mica (illite) crystallinity value of &lt; 0.42D.2U obtained by X-ray diffraction analysis, is used to define the onset of metamorphism (Kisch, 1991). In this scheme, the first appearance of glaucophane, lawsonite, paragonite, prehnite, pumpellyite or stilpnomelane is taken to indicate the lower limit of metamorphism (Frey and Kisch, 1987; Bucher and Frey, 1994; Frey and Robinson, 1998). Most workers agree that such mineral growth starts at 150 ± 50° C in silicate rocks. Many lithologies may show no change in mineralogy under these conditions and hence the recognition of the onset of metamorphism will vary with bulk composition.”"@en ;
  rdfs:comment "Rock formed by solid-state mineralogical, chemical and/or structural changes to a pre-existing rock, in response to marked changes in temperature, pressure, shearing stress and chemical environment."@en ;
  rdfs:comment "dct:source--  Jackson 1997"@en ;
  rdfs:label "metamorphic rock"@en ;
  rdfs:subClassOf gslth:composite_genesis_rock ;
.
gslth:metasomatic_rock
  a owl:Class ;
  rdfs:comment "Rock that has fabric and composition indicating open-system mineralogical and chemical changes in response to interaction with a fluid phase, typically water rich."@en ;
  rdfs:comment "SLTTm (2004) proposed the following criteria to distinguish hydrothermally altered or metasomatic rock from igneous rock. \"The rock is classified as metamorphic if (1) the texture has been modified such that it can no longer be considered igneous, (2) the bulk composition of the rock is inconsistent with compositions that can be derived purely from a magma and associated processes such as assimilation and differentiation, or (3) minerals inconsistent with magmatic crystallization are present.\""@en ;
  rdfs:comment "dct:source--  This vocabulary"@en ;
  rdfs:label "metasomatic rock"@en ;
  rdfs:subClassOf gslth:composite_genesis_rock ;
.
gslth:mica_schist
  a owl:Class ;
  rdfs:comment "A schist that consists of more than 50 percent mica minerals, typically muscovite or biotite. Special type included to distinguish this common variety of schist."@en ;
  rdfs:comment "Include single subcategory of schist to indicate this common kind of schist. 'Mica rich metamorphic rock' for compound use with schist fabric term would be more compatible with treatment of blueschist (Glaucophane lawsonite epidote metamorphic rock) and greenschist (Chlorite actinolite epidote metamorphic rock), but based on the assumption that schist is the only rock type that will meet the mica-rich criteria, it seems reasonable to include as a subtype of schist."@en ;
  rdfs:comment "dct:source--  This vocabulary"@en ;
  rdfs:label "mica schist"@en ;
  rdfs:subClassOf gslth:schist ;
.
gslth:migmatite
  a owl:Class ;
  rdfs:comment "Silicate metamorphic rock that is pervasively heterogeneous on a decimeter to meter scale that typically consists of darker and lighter parts; the darker parts usually exhibit features of metamorphic rocks whereas the lighter parts are of igneous-looking appearance."@en ;
  rdfs:comment "dct:source--  Fette and Desmons (2007) (http://www.bgs.ac.uk/SCMR/)"@en ;
  rdfs:label "migmatite"@en ;
  rdfs:subClassOf gslth:metamorphic_rock ;
.
gslth:monzodiorite
  a owl:Class ;
  rdfs:comment "Phaneritic crystalline igneous rock consisting of sodic plagioclase (An0 to An50), alkali feldspar, hornblende and biotite, with or without pyroxene, and 0 to 5 percent quartz. Includes rocks defined modally in QAPF field 9."@en ;
  rdfs:comment "dct:source--  LeMaitre et al. 2002"@en ;
  rdfs:label "monzodiorite"@en ;
  rdfs:subClassOf gslth:monzodioritic_rock ;
.
gslth:monzodioritic_rock
  a owl:Class ;
  rdfs:comment "Phaneritic crystalline igneous rock consisting of sodic plagioclase (An0 to An50), alkali feldspar, hornblende and biotite, with or without pyroxene, and 0 to 10 percent feldspathoid or 0 to 20 percent quartz in the QAPF fraction. Plagioclase to total feldspar ratio in the QAPF fraction is between 0.65 and 0.9. Includes rocks defined modally in QAPF field 9, 9' and 9* as monzodiorite, foid-beaing monzodiorite, and quartz monzodiorite."@en ;
  rdfs:comment "dct:source--  This vocabulary; LeMaitre et al. 2002"@en ;
  rdfs:label "monzodioritic rock"@en ;
  rdfs:subClassOf gslth:dioritoid ;
.
gslth:monzogabbro
  a owl:Class ;
  rdfs:comment "Monzogabbroic rock that contains between 0 an 5 percent quartz and no feldspathoid mineral in the QAPF fraction. Includes rocks defined modally in QAPF field 9 ."@en ;
  rdfs:comment "dct:source--  LeMaitre et al. 2002, This vocabulary"@en ;
  rdfs:label "monzogabbro"@en ;
  rdfs:subClassOf gslth:monzogabbroic_rock ;
.
gslth:monzogabbroic_rock
  a owl:Class ;
  rdfs:comment "Gabbroid with a plagioclase to total feldspar ratio between 0.65 and 0.9. QAPF field 9, 9 prime and 9 asterisk"@en ;
  rdfs:comment "dct:source--  LeMaitre et al. 2002, This vocabulary"@en ;
  rdfs:label "monzogabbroic rock"@en ;
  rdfs:subClassOf gslth:gabbroid ;
.
gslth:monzogranite
  a owl:Class ;
  rdfs:comment "Granite that has a plagiolcase to total feldspar ratio between 0.35 and 0.65. QAPF field 3b."@en ;
  rdfs:comment "dct:source--  LeMaitre et al. 2002"@en ;
  rdfs:label "monzogranite"@en ;
  rdfs:subClassOf gslth:granite ;
.
gslth:monzonite
  a owl:Class ;
  rdfs:comment "Monzonitic rock that contains 0-5 percent quartz and no feldspathoid mineral in the QAPF fraction. Includes rocks defined modally in QAPF Field 8."@en ;
  rdfs:comment "dct:source--  LeMaitre et al. 2002"@en ;
  rdfs:label "monzonite"@en ;
  rdfs:subClassOf gslth:monzonitic_rock ;
.
gslth:monzonitic_rock
  a owl:Class ;
  rdfs:comment "Syenitoid with a plagioclase to total feldspar ratio between 0.35 and 0.65. Includes rocks in QAPF fields 8, 8*, and 8'."@en ;
  rdfs:comment "dct:source--  LeMaitre et al. 2002"@en ;
  rdfs:label "monzonitic rock"@en ;
  rdfs:subClassOf gslth:syenitoid ;
.
gslth:mud
  a owl:Class ;
  rdfs:comment "Clastic sediment consisting of less than 30 percent gravel-size (2 mm) particles and with a mud-size to sand-size particle ratio greater than 1. More than half of the particles are of epiclastic origin."@en ;
  rdfs:comment "dct:source--  definition of mud from SLTTs 2004 muddy sediment; particle sizes defined from Krumbein phi scale (W C Krumbein and L L Sloss, Stratigraphy and Sedimentation, 2nd edition, Freeman, San Francisco, 1963; Krumbein and Pettijohn, 1938, Manual of Sedimentary Petrography: New York, Appleton Century Co., Inc.)"@en ;
  rdfs:label "mud"@en ;
  rdfs:subClassOf gslth:clastic_sediment ;
  rdfs:subClassOf gslth:mud_size_sediment ;
.
gslth:mud_size_sediment
  a owl:Class ;
  rdfs:comment "Sediment consisting of less than 30 percent gravel-size (2 mm) particles and with a mud-size to sand-size particle ratio greater than 1. Clasts may be of any composition or origin."@en ;
  rdfs:comment "dct:source--  based on SLTTs 2004; Neuendorf et al. 2005; particle sizes defined from Krumbein phi scale (W C Krumbein and L L Sloss, Stratigraphy and Sedimentation, 2nd edition, Freeman, San Francisco, 1963; Krumbein and Pettijohn, 1938, Manual of Sedimentary Petrography: New York, Appleton Century Co., Inc.)"@en ;
  rdfs:label "mud size sediment"@en ;
  rdfs:subClassOf gslth:sediment ;
.
gslth:mylonitic_rock
  a owl:Class ;
  rdfs:comment "Metamorphic rock characterised by a foliation resulting from tectonic grain size reduction, in which more than 10 percent of the rock volume has undergone grain size reduction. Includes protomylonite, mylonite, ultramylonite, and blastomylonite."@en ;
  rdfs:comment "dct:source--  Marshak and Mitra 1988"@en ;
  rdfs:label "mylonitic rock"@en ;
  rdfs:subClassOf gslth:fault_related_material ;
  rdfs:subClassOf gslth:foliated_metamorphic_rock ;
.
gslth:natural_unconsolidated_material
  a owl:Class ;
  rdfs:comment "Unconsolidated material known to have natural, ie. not human-made, origin."@en ;
  rdfs:comment "dct:source--  This vocabulary"@en ;
  rdfs:label "natural unconsolidated material"@en ;
  rdfs:subClassOf gslth:unconsolidated_material ;
.
gslth:non_clastic_siliceous_sediment
  a owl:Class ;
  rdfs:comment "Sediment that consists of at least 50 percent silicate mineral material, deposited directly by chemical or biological processes at the depositional surface, or in particles formed by chemical or biological processes within the basin of deposition."@en ;
  rdfs:comment "dct:source--  NGMDB 2008; Hallsworth and Knox 1999"@en ;
  rdfs:label "non clastic siliceous sediment"@en ;
  rdfs:subClassOf gslth:non_clastic_siliceous_sedimentary_material ;
  rdfs:subClassOf gslth:sediment ;
.
gslth:non_clastic_siliceous_sedimentary_material
  a owl:Class ;
  rdfs:comment "Sedimentary material that consists of at least 50 percent silicate mineral material, deposited directly by chemical or biological processes at the depositional surface, or in particles formed by chemical or biological processes within the basin of deposition."@en ;
  rdfs:comment "dct:source--  SLTTs 2004"@en ;
  rdfs:label "non clastic siliceous sedimentary material"@en ;
  rdfs:subClassOf gslth:sedimentary_material ;
.
gslth:non_clastic_siliceous_sedimentary_rock
  a owl:Class ;
  rdfs:comment "Sedimentary rock that consists of at least 50 percent silicate mineral material, deposited directly by chemical or biological processes at the depositional surface, or in particles formed by chemical or biological processes within the basin of deposition."@en ;
  rdfs:comment "dct:source--  SLTTs 2004"@en ;
  rdfs:label "non clastic siliceous sedimentary rock"@en ;
  rdfs:subClassOf gslth:non_clastic_siliceous_sedimentary_material ;
  rdfs:subClassOf gslth:sedimentary_rock ;
.
gslth:ontology
  a owl:Ontology ;
  rdfs:comment "Rock type categories modified from CGI SimpleLithology; properties based on GeoSciML v3.2 conceptual model. Scope includes gso Rock_Material and gso Granular Material. GSO granular material is analogous to GeoSciMLv3.2 compound material particle geometry description.  "@en ;
  rdfs:label "GSO Rock Material ontology."@en ;
  owl:imports gsog:ontology ;
  owl:imports <http://loop3d.org/GSO/ontology/2020/1/geologicquality/ontology> ;
  owl:imports gscc:ontology ;
  owl:imports <http://loop3d.org/GSO/ontology/2020/1/lithology/consolidationdegree/ontology> ;
  owl:imports gsgc:ontology ;
  owl:imports gsar:ontology ;
  owl:imports <http://loop3d.org/GSO/ontology/2020/1/lithology/particleroundness/ontology/> ;
  owl:imports gspt:ontology ;
  owl:imports gsmf:ontology ;
  owl:imports gsmg:ontology ;
.
gslth:ooze
  a owl:Class ;
  a owl:NamedIndividual ;
  rdfs:comment "Biogenic sediment consisting of less than 1 percent gravel-size (greater than or equal to 2 mm) particles, with a sand to mud ratio less than 1 to 9, and less than 50 percent carbonate minerals."@en ;
  rdfs:comment "Neuendorf et al. 2005 put cutoff at 30 percent skeletal remains; this is raised to 50 percent in This vocabulary for consistency with definition of other Biogenic sediment category"@en ;
  rdfs:comment "dct:source--  based on Bates and Jackson 1987 and Hallsworth and Knox 1999"@en ;
  rdfs:comment "skos:altLabel--  biogenic mud"@en ;
  rdfs:label "ooze"@en ;
  rdfs:subClassOf gslth:biogenic_sediment ;
  rdfs:subClassOf gslth:mud_size_sediment ;
.
gslth:organic_bearing_mudstone
  a owl:Class ;
  a owl:NamedIndividual ;
  rdfs:comment "Mudstone that contains a significant amount of organic carbon, typically kerogen. commonly finely laminated, brown or black in color."@en ;
  rdfs:comment "dct:source--  Neuendorf et al. 2005; http://en.wikipedia.org/wiki/Oil_shale"@en ;
  rdfs:comment "skos:altLabel--  oil shale"@en ;
  rdfs:label "organic bearing mudstone"@en ;
  rdfs:subClassOf gslth:generic_mudstone ;
.
gslth:organic_rich_sediment
  a owl:Class ;
  rdfs:comment "Sediment with color, composition, texture and apparent density indicating greater than 50 percent organic content by weight on a moisture-free basis."@en ;
  rdfs:comment "The broader relation from organic rich sediment to biogenic sediment is based on the inference that organic rich material is always biogenic in origin. Biogenic is a broader category because not all biogenic materials are organic rich, for example shells or phosphatic bone."@en ;
  rdfs:comment "dct:source--  SLTTs 2004"@en ;
  rdfs:label "organic rich sediment"@en ;
  rdfs:subClassOf gslth:biogenic_sediment ;
  rdfs:subClassOf gslth:organic_rich_sedimentary_material ;
.
gslth:organic_rich_sedimentary_material
  a owl:Class ;
  rdfs:comment "Sedimentary material in which 50 percent or more of the primary sedimentary material is organic carbon."@en ;
  rdfs:comment "dct:source--  SLTTs 2004"@en ;
  rdfs:label "organic rich sedimentary material"@en ;
  rdfs:subClassOf gslth:sedimentary_material ;
.
gslth:organic_rich_sedimentary_rock
  a owl:Class ;
  rdfs:comment "Sapropelic coal, and asphaltite are not differentiated in This vocabulary"@en ;
  rdfs:comment "Sedimentary rock with color, composition, texture and apparent density indicating greater than 50 percent organic content by weight on a moisture-free basis."@en ;
  rdfs:comment "dct:source--  SLTTs 2004"@en ;
  rdfs:label "organic rich sedimentary rock"@en ;
  rdfs:subClassOf gslth:organic_rich_sedimentary_material ;
  rdfs:subClassOf gslth:sedimentary_rock ;
.
gslth:orthogneiss
  a owl:Class ;
  rdfs:comment "A gneiss with mineralogy and texture indicating derivation from a phaneritic igneous rock protolith. Typically consists of abundant feldspar, with quartz, and variable hornblende, biotite, and muscovite, with a relatively homogeneous character."@en ;
  rdfs:comment "dct:source--  This vocabulary"@en ;
  rdfs:label "orthogneiss"@en ;
  rdfs:subClassOf gslth:gneiss ;
.
gslth:packstone
  a owl:Class ;
  rdfs:comment "Carbonate sedimentary rock with discernible grain supported depositional texture, containing greater than 10 percent grains, and constituent particles are of intrabasinal origin; intergranular spaces are filled by matrix."@en ;
  rdfs:comment "Note that this category overlaps with 'carbonate mudstone'."@en ;
  rdfs:comment "dct:source--  Hallsworth and Knox 1999"@en ;
  rdfs:label "packstone"@en ;
  rdfs:subClassOf gslth:carbonate_sedimentary_rock ;
.
gslth:paragneiss
  a owl:Class ;
  rdfs:comment "A gneiss with mineralogy and texture indicating derivation from a sedimentary rock protolith. Typically consists of abundant quartz, mica, or calcsilicate minerals; aluminosilicate minerals or garnet commonly present. composition of rock tends to be more variable on a decimetric scale that in orthogneiss."@en ;
  rdfs:comment "dct:source--  This vocabulary"@en ;
  rdfs:label "paragneiss"@en ;
  rdfs:subClassOf gslth:gneiss ;
.
gslth:peat
  a owl:Class ;
  rdfs:comment "Unconsolidated organic-rich sediment composed of at least 50 percent semi-carbonised plant remains; individual remains commonly seen with unaided eye; yellowish brown to brownish black; generally fibrous texture; can be plastic or friable. In its natural state it can be readily cut and has a very high moisture content, generally greater than 90 percent. Liptinite to Inertinite ratio is less than one (Economic commission for Europe, committee on Sustainable Energy- United Nations (ECE-UN), 1998, International Classification of in-Seam Coals: Energy 19, 41 pp.)"@en ;
  rdfs:comment "dct:source--  Hallsworth and Knox 1999"@en ;
  rdfs:label "peat"@en ;
  rdfs:subClassOf gslth:organic_rich_sediment ;
.
gslth:pebble_gravel_size_sediment
  a owl:Class ;
  rdfs:comment "Sediment containing greater than 30 percent pebble-size particles (2.0 -64 mm in diameter)"@en ;
  rdfs:comment "dct:source--  Wentworth size scale"@en ;
  rdfs:label "pebble gravel size sediment"@en ;
  rdfs:subClassOf gslth:gravel_size_sediment ;
.
gslth:pegmatite
  a owl:Class ;
  rdfs:comment "Exceptionally coarse grained crystalline rock with interlocking crystals; most grains are 1cm or more diameter; composition is generally that of granite, but the term may refer to the coarse grained facies of any type of igneous rock;usually found as irregular dikes, lenses, or veins associated with plutons or batholiths."@en ;
  rdfs:comment "dct:source--  Neuendorf et al. 2005"@en ;
  rdfs:label "pegmatite"@en ;
  rdfs:subClassOf gslth:phaneritic_igneous_rock ;
.
gslth:peridotite
  a owl:Class ;
  rdfs:comment "Ultramafic rock consisting of more than 40 percent (by volume) olivine with pyroxene and/or amphibole and little or no feldspar. commonly altered to serpentinite. Includes rocks defined modally in the ultramafic rock classification as dunite, harzburgite, lherzolite, wehrlite, olivinite, pyroxene peridotite, pyroxene hornblende peridotite or hornblende peridotite."@en ;
  rdfs:comment "dct:source--  LeMaitre et al. 2002"@en ;
  rdfs:label "peridotite"@en ;
  rdfs:subClassOf gslth:phaneritic_igneous_rock ;
  rdfs:subClassOf gslth:ultramafic_igneous_rock ;
.
gslth:phaneritic_igneous_rock
  a owl:Class ;
  a owl:NamedIndividual ;
  rdfs:comment "Igneous rock in which the framework of the rock consists of individual crystals that can be discerned with the unaided eye. Bounding grain size is on the order of 32 to 100 microns. Igneous rocks with 'exotic' composition are excluded from this concept."@en ;
  rdfs:comment "dct:source--  Neuendorf et al. 2005"@en ;
  rdfs:comment "skos:altLabel--  coarse grained crystalline igneous rock"@en ;
  rdfs:comment "skos:altLabel--  plutonic rock"@en ;
  rdfs:label "phaneritic igneous rock"@en ;
  rdfs:subClassOf gslth:igneous_rock ;
.
gslth:phonolilte
  a owl:Class ;
  rdfs:comment "Phonolitoid in which the plagioclase to total feldspar ratio is less than 0.1. Rock consists of alkali feldspar, feldspathoid minerals, and mafic minerals."@en ;
  rdfs:comment "dct:source--  LeMaitre et al. 2002"@en ;
  rdfs:label "phonolite"@en ;
  rdfs:subClassOf gslth:phonolitoid ;
.
gslth:phonolitic_basanite
  a owl:Class ;
  rdfs:comment "Tephritoid that has a plagioclase to total feldspar ratio between 0.5 and 0.9, and contains more than 10 percent normative (CIPW) olivine."@en ;
  rdfs:comment "dct:source--  LeMaitre et al. 2002"@en ;
  rdfs:label "phonolitic basanite"@en ;
  rdfs:subClassOf gslth:tephritoid ;
.
gslth:phonolitic_foidite
  a owl:Class ;
  rdfs:comment "Foiditoid that contains less than 90 percent feldspathoid minerals in the QAPF fraction, and has a plagioclase to total feldspar ratio that is less than 0.5"@en ;
  rdfs:comment "dct:source--  LeMaitre et al. 2002"@en ;
  rdfs:label "phonolitic foidite"@en ;
  rdfs:subClassOf gslth:foiditoid ;
.
gslth:phonolitic_tephrite
  a owl:Class ;
  rdfs:comment "Tephritoid that has a plagioclase to total feldspar ratio between 0.5 and 0.9, and contains less than 10 percent normative (CIPW) olivine."@en ;
  rdfs:comment "dct:source--  LeMaitre et al. 2002"@en ;
  rdfs:label "phonolitic tephrite"@en ;
  rdfs:subClassOf gslth:tephritoid ;
.
gslth:phonolitoid
  a owl:Class ;
  a owl:NamedIndividual ;
  rdfs:comment "Fine grained igneous rock than contains less than 90 percent mafic minerals, between 10 and 60 percent feldspathoid mineral in the QAPF fraction and has a plagioclase to total feldspar ratio less than 0.5. Includes rocks defined modally in QAPF fields 11 and 12, and TAS field Ph."@en ;
  rdfs:comment "dct:source--  LeMaitre et al. 2002"@en ;
  rdfs:comment "skos:altLabel--  phonolitic rock"@en ;
  rdfs:label "phonolitoid"@en ;
  rdfs:subClassOf gslth:fine_grained_igneous_rock ;
.
gslth:phosphate_rich_sediment
  a owl:Class ;
  rdfs:comment "Sediment in which at least 50 percent of the primary and/or recrystallized constituents are phosphate minerals."@en ;
  rdfs:comment "dct:source--  SLTTs 2004"@en ;
  rdfs:label "phosphate rich sediment"@en ;
  rdfs:subClassOf gslth:phosphate_rich_sedimentary_material ;
  rdfs:subClassOf gslth:sediment ;
.
gslth:phosphate_rich_sedimentary_material
  a owl:Class ;
  rdfs:comment "Sedimentary material in which at least 50 percent of the primary and/or recrystallized constituents are phosphate minerals."@en ;
  rdfs:comment "dct:source--  SLTTs 2004"@en ;
  rdfs:label "phosphate rich sedimentary material"@en ;
  rdfs:subClassOf gslth:sedimentary_material ;
.
gslth:phosphorite
  a owl:Class ;
  rdfs:comment "Sedimentary rock in which at least 50 percent of the primary or recrystallized constituents are phosphate minerals. Most commonly occurs as a bedded primary or reworked secondary marine rock, composed of microcrystalline carbonate fluorapatite in the form of lamina, pellets, oolites and nodules, and skeletal, shell and bone fragments."@en ;
  rdfs:comment "dct:source--  HallsworthandKnox 1999, Jackson 1997"@en ;
  rdfs:label "phosphorite"@en ;
  rdfs:subClassOf gslth:phosphate_rich_sedimentary_material ;
  rdfs:subClassOf gslth:sedimentary_rock ;
.
gslth:phyllite
  a owl:Class ;
  rdfs:comment "Rock with a well developed, continuous schistosity, an average grain size between 0.1 and 0.5 millimeters, and a silvery sheen on cleavage surfaces. Individual phyllosilicate grains are barely visible with the unaided eye."@en ;
  rdfs:comment "dct:source--  IUGS SCMR 2007 (http://www.bgs.ac.uk/SCMR/)"@en ;
  rdfs:label "phyllite"@en ;
  rdfs:subClassOf gslth:foliated_metamorphic_rock ;
.
gslth:phyllonite
  a owl:Class ;
  rdfs:comment "Mylonitic rock composed largely of fine-grained mica that imparts a sheen to foliation surfaces; may have flaser lamination, isoclinal folding, and deformed veins, which indicate significant shearing. Macroscopically resembles phyllite, but formed by mechanical degradation of initially coarser rock."@en ;
  rdfs:comment "dct:source--  NADM metamorphic rock vocabulary SLTTm1.0; Marshak and Mitra 1988"@en ;
  rdfs:label "phyllonite"@en ;
  rdfs:subClassOf gslth:mylonitic_rock ;
.
gslth:porphyry
  a owl:Class ;
  rdfs:comment "Igneous rock that contains conspicuous phenocrysts in a finer grained groundmass; groundmass itself may be phaneritic or fine-grained."@en ;
  rdfs:comment "dct:source--  LeMaitre et al. 2002"@en ;
  rdfs:label "porphyry"@en ;
  rdfs:subClassOf gslth:igneous_rock ;
.
gslth:pure_calcareous_carbonate_sediment
  a owl:Class ;
  a owl:NamedIndividual ;
  rdfs:comment "Carbonate sediment in which greater than 90 percent of the constituents are composed of one (or more) of the carbonate minerals in particles of intrabasinal origin, and a calcite (plus aragonite) to dolomite ratio greater than 1 to 1."@en ;
  rdfs:comment "dct:source--  This vocabulary"@en ;
  rdfs:comment "skos:altLabel--  lime sediment"@en ;
  rdfs:label "pure calcareous carbonate sediment"@en ;
  rdfs:subClassOf gslth:calcareous_carbonate_sediment ;
  rdfs:subClassOf gslth:pure_carbonate_sediment ;
.
gslth:pure_carbonate_mudstone
  a owl:Class ;
  rdfs:comment "Mudstone that consists of greater than 90 percent carbonate minerals of intrabasinal orign in the mud fraction, and contains less than 10 percent allochems. The original depositional texture is preserved and fabric is matrix supported. Carbonate mudstone of Dunham (1962)"@en ;
  rdfs:comment "dct:source--  Dunham 1962"@en ;
  rdfs:label "pure carbonate mudstone"@en ;
  rdfs:subClassOf gslth:generic_mudstone ;
  rdfs:subClassOf gslth:pure_carbonate_sedimentary_rock ;
.
gslth:pure_carbonate_sediment
  a owl:Class ;
  rdfs:comment "Carbonate sediment in which greater than 90 percent of the constituents are composed of one (or more) of the carbonate minerals in particles of intrabasinal origin."@en ;
  rdfs:comment "dct:source--  This vocabulary"@en ;
  rdfs:label "pure carbonate sediment"@en ;
  rdfs:subClassOf gslth:carbonate_sediment ;
.
gslth:pure_carbonate_sedimentary_rock
  a owl:Class ;
  rdfs:comment "Sedimentary rock in which greater than 90 percent of the primary and/or recrystallized constituents are carbonate minerals."@en ;
  rdfs:comment "dct:source--  This vocabulary"@en ;
  rdfs:label "pure carbonate sedimentary rock"@en ;
  rdfs:subClassOf gslth:carbonate_sedimentary_rock ;
.
gslth:pure_dolomitic_sediment
  a owl:Class ;
  rdfs:comment "Carbonate sediment in which greater than 90 percent of the constituents are composed of one (or more) of the carbonate minerals in particles of intrabasinal origin, and a ratio of magnesium carbonate to calcite (plus aragonite) greater than 1 to 1."@en ;
  rdfs:comment "dct:source--  This vocabulary"@en ;
  rdfs:label "pure dolomitic sediment"@en ;
  rdfs:subClassOf gslth:dolomitic_sediment ;
  rdfs:subClassOf gslth:pure_carbonate_sediment ;
.
gslth:pyroclastic_material
  a owl:Class ;
  rdfs:comment "Fragmental igneous material that consists of more than 75 percent of particles formed by disruption as a direct result of volcanic action."@en ;
  rdfs:comment "dct:source--  LeMaitre et al. 2002"@en ;
  rdfs:label "pyroclastic material"@en ;
  rdfs:subClassOf gslth:fragmental_igneous_material ;
.
gslth:pyroclastic_rock
  a owl:Class ;
  rdfs:comment "Fragmental igneous rock that consists of greater than 75 percent fragments produced as a direct result of eruption or extrusion of magma from within the earth onto its surface. Includes autobreccia associated with lava flows and excludes deposits reworked by epiclastic processes."@en ;
  rdfs:comment "dct:source--  based on LeMaitre et al. 2002"@en ;
  rdfs:label "pyroclastic rock"@en ;
  rdfs:subClassOf gslth:fragmental_igneous_rock ;
  rdfs:subClassOf gslth:pyroclastic_material ;
.
gslth:pyroxenite
  a owl:Class ;
  rdfs:comment "Ultramafic phaneritic igneous rock composed almost entirely of one or more pyroxenes and occasionally biotite, hornblende and olivine. Includes rocks defined modally in the ultramafic rock classification as olivine pyroxenite, olivine-hornblende pyroxenite, pyroxenite, orthopyroxenite, clinopyroxenite and websterite."@en ;
  rdfs:comment "dct:source--  LeMaitre et al. 2002"@en ;
  rdfs:label "pyroxenite"@en ;
  rdfs:subClassOf gslth:phaneritic_igneous_rock ;
  rdfs:subClassOf gslth:ultramafic_igneous_rock ;
.
gslth:quartz_alkali_feldspar_syenite
  a owl:Class ;
  rdfs:comment "Alkali feldspar syenitic rock that contains 5 to 20 percent quartz and no feldspathoid in the QAPF fraction. QAPF field 6*."@en ;
  rdfs:comment "dct:source--  LeMaitre et al. 2002"@en ;
  rdfs:label "quartz alkali feldspar syenite"@en ;
  rdfs:subClassOf gslth:alkali_feldspar_syenitic_rock ;
.
gslth:quartz_alkali_feldspar_trachyte
  a owl:Class ;
  rdfs:comment "Alkali feldspar trachytic rock that contains and between 5 and 20 percent quartz mineral in the QAPF fraction. QAPF field 6*."@en ;
  rdfs:comment "dct:source--  LeMaitre et al. 2002"@en ;
  rdfs:label "quartz alkali feldspar trachyte"@en ;
  rdfs:subClassOf gslth:alkali_feldspar_trachytic_rock ;
.
gslth:quartz_anorthosite
  a owl:Class ;
  rdfs:comment "Anorthositic rock that contains between 5 and 20 percent quartz in the QAPF fraction. QAPF field 10*."@en ;
  rdfs:comment "dct:source--  LeMaitre et al. 2002"@en ;
  rdfs:label "quartz anorthosite"@en ;
  rdfs:subClassOf gslth:anorthositic_rock ;
.
gslth:quartz_diorite
  a owl:Class ;
  rdfs:comment "Dioritic rock that contains between 5 to 20 percent quartz in the QAPF fraction. QAPF field 10*."@en ;
  rdfs:comment "dct:source--  LeMaitre et al. 2002"@en ;
  rdfs:label "quartz diorite"@en ;
  rdfs:subClassOf gslth:dioritic_rock ;
.
gslth:quartz_gabbro
  a owl:Class ;
  rdfs:comment "Gabbroic rock that contains between 5 and 20 percent quartz in the QAPF fraction. QAPF field 10*."@en ;
  rdfs:comment "dct:source--  LeMaitre et al. 2002"@en ;
  rdfs:label "quartz gabbro"@en ;
  rdfs:subClassOf gslth:gabbroic_rock ;
.
gslth:quartz_latite
  a owl:Class ;
  rdfs:comment "Latitic rock that contains between 5 and 20 percent quartz in the QAPF fraction. QAPF field 8*."@en ;
  rdfs:comment "dct:source--  LeMaitre et al. 2002"@en ;
  rdfs:label "quartz latite"@en ;
  rdfs:subClassOf gslth:latitic_rock ;
.
gslth:quartz_monzodiorite
  a owl:Class ;
  rdfs:comment "Monzodioritic rock that contains between 5 and 20 percent quartz."@en ;
  rdfs:comment "dct:source--  LeMaitre et al. 2002"@en ;
  rdfs:label "quartz monzodiorite"@en ;
  rdfs:subClassOf gslth:monzodioritic_rock ;
.
gslth:quartz_monzogabbro
  a owl:Class ;
  rdfs:comment "Monzogabbroic rock that contains between 5 and 20 percent quartz in the QAPF fraction. QAPF field 9*."@en ;
  rdfs:comment "dct:source--  LeMaitre et al. 2002"@en ;
  rdfs:label "quartz monzogabbro"@en ;
  rdfs:subClassOf gslth:monzogabbroic_rock ;
.
gslth:quartz_monzonite
  a owl:Class ;
  rdfs:comment "Monzonitic rock that contains 5-20 percent quartz iin the QAPF fraction. Includes rocks defined modally in QAPF Field 8*."@en ;
  rdfs:comment "dct:source--  LeMaitre et al. 2002"@en ;
  rdfs:label "quartz monzonite"@en ;
  rdfs:subClassOf gslth:monzonitic_rock ;
.
gslth:quartz_rich_igneous_rock
  a owl:Class ;
  rdfs:comment "Occurrence of igneous rocks meeting this criteria seems to be vanishingly rare, thus subdividing the category does not seem warranted for the purposes of This vocabulary. Future usage of the vocabulary may motivate including quatzolite and quartz-rich granitoid in future revisions"@en ;
  rdfs:comment "Phaneritic crystalline igneous rock that contains less than 90 percent mafic minerals and contains greater than 60 percent quartz in the QAPF fraction."@en ;
  rdfs:comment "dct:source--  Gillespie and Styles 1999; LeMaitre et al. 2002"@en ;
  rdfs:label "quartz rich igneous rock"@en ;
  rdfs:subClassOf gslth:acidic_igneous_rock ;
  rdfs:subClassOf gslth:phaneritic_igneous_rock ;
.
gslth:quartz_syenite
  a owl:Class ;
  rdfs:comment "Syenitic rock that contains between 5 and 20 percent quartz in the QAPF fraction. Defined modally in QAPF Field 7*."@en ;
  rdfs:comment "dct:source--  LeMaitre et al. 2002"@en ;
  rdfs:label "quartz syenite"@en ;
  rdfs:subClassOf gslth:syenitic_rock ;
.
gslth:quartz_trachyte
  a owl:Class ;
  rdfs:comment "Trachytic rock that contains between 5 and 20 percent quartz in the QAPF fraction. QAPF field 7*."@en ;
  rdfs:comment "dct:source--  LeMaitre et al. 2002"@en ;
  rdfs:label "quartz trachyte"@en ;
  rdfs:subClassOf gslth:trachytic_rock ;
.
gslth:quartzite
  a owl:Class ;
  rdfs:comment "Metamorphic rock consisting of greater than or equal to 75 percent quartz; typically granoblastic texture."@en ;
  rdfs:comment "dct:source--  after Neuendorf et al. 2005"@en ;
  rdfs:label "quartzite"@en ;
  rdfs:subClassOf gslth:metamorphic_rock ;
.
gslth:residual_material
  a owl:Class ;
  rdfs:comment "Material of composite origin resulting from weathering processes at the Earth's surface, with genesis dominated by removal of chemical constituents by aqueous leaching. Miinor clastic, chemical, or organic input may also contribute. Consolidation state is not inherent in definition, but typically material is unconsolidated or weakly consolidated."@en ;
  rdfs:comment "dct:source--  This vocabulary"@en ;
  rdfs:label "residual material"@en ;
  rdfs:subClassOf gslth:material_formed_in_surficial_environment ;
.
gslth:rhyolite
  a owl:Class ;
  rdfs:comment "dct:source--  LeMaitre et al. 2002"@en ;
  rdfs:comment "rhyolitoid in which the ratio of plagioclase to total feldspar is between 0.1 and 0.65."@en ;
  rdfs:label "rhyolite"@en ;
  rdfs:subClassOf gslth:rhyolitoid ;
.
gslth:rhyolitoid
  a owl:Class ;
  a owl:NamedIndividual ;
  rdfs:comment "Note that technical definition, based on modal mineralogy plotted in a QAPF triangle may be applied qualitatively, based on phenocryst mineralogy when ground mass mineralogy can not be determined optically, or based on CIPW norm. Although TAS categories are defined based on chemical analyses, the correspondence with the QAPF defined categories is generally close enough that QAPF categories are commonly used interchangeably with TAS categories. It is important to note the basis for assignment of fine-grained igneous rocks to a specifice lithology category."@en ;
  rdfs:comment "dct:source--  LeMaitre et al. 2002"@en ;
  rdfs:comment "fine_grained_igneous_rock consisting of quartz and alkali feldspar, with minor plagioclase and biotite, in a microcrystalline, cryptocrystalline or glassy groundmass. Flow texture is common. Includes rocks defined modally in QAPF fields 2 and 3 or chemically in TAS Field R as rhyolite. QAPF normative definition is based on modal mineralogy thus: less than 90 percent mafic minerals, between 20 and 60 percent quartz in the QAPF fraction, and ratio of plagioclse to total feldspar is less than 0.65."@en ;
  rdfs:comment "skos:altLabel--  rhyolitic rock"@en ;
  rdfs:label "rhyolitoid"@en ;
  rdfs:subClassOf gslth:acidic_igneous_rock ;
  rdfs:subClassOf gslth:fine_grained_igneous_rock ;
.
gslth:rock
  a owl:Class ;
  rdfs:comment "Consolidated aggregate of one or more EarthMaterials, or a body of undifferentiated mineral matter, or of solid organic material. Includes mineral aggregates such as granite, shale, marble; glassy matter such as obsidian; and organic material such a coal. Excludes unconsolidated materials."@en ;
  rdfs:comment "dct:source--  Jackson, 1997; NADM C1 2004; Neuendorf et al 2005"@en ;
  rdfs:label "rock"@en ;
  rdfs:subClassOf gslth:compound_material ;
.
gslth:rock_gypsum_or_anhydrite
  a owl:Class ;
  rdfs:comment "Evaporite composed of at least 50 percent gypsum or anhydrite."@en ;
  rdfs:comment "dct:source--  This vocabulary"@en ;
  rdfs:label "gypsum or anhydrite"@en ;
  rdfs:subClassOf gslth:evaporite ;
.
gslth:rock_salt
  a owl:Class ;
  rdfs:comment "Evaporite composed of at least 50 percent halite."@en ;
  rdfs:comment "dct:source--  This vocabulary"@en ;
  rdfs:label "rock salt"@en ;
  rdfs:subClassOf gslth:evaporite ;
.
gslth:sand
  a owl:Class ;
  rdfs:comment "Clastic sediment in which less than 30 percent of particles are gravel (greater than 2 mm in diameter) and the sand to mud ratio is at least 1. More than half of the particles are of epiclastic origin."@en ;
  rdfs:comment "dct:source--  definition of sand from SLTTs 2004 sandy sediment; particle sizes defined from Krumbein phi scale (W C Krumbein and L L Sloss, Stratigraphy and Sedimentation, 2nd edition, Freeman, San Francisco, 1963; Krumbein and Pettijohn, 1938, Manual of Sedimentary Petrography: New York, Appleton Century Co., Inc.)"@en ;
  rdfs:label "sand"@en ;
  rdfs:subClassOf gslth:clastic_sediment ;
  rdfs:subClassOf gslth:sand_size_sediment ;
.
gslth:sand_size_sediment
  a owl:Class ;
  rdfs:comment "Sediment in which less than 30 percent of particles are gravel (greater than 2 mm in diameter) and the sand to mud ratio is at least 1. composition or genesis of clasts not specified."@en ;
  rdfs:comment "dct:source--  Neuendorf et al. 2005 ; particle sizes defined from Krumbein phi scale (W C Krumbein and L L Sloss, Stratigraphy and Sedimentation, 2nd edition, Freeman, San Francisco, 1963; Krumbein and Pettijohn, 1938, Manual of Sedimentary Petrography: New York, Appleton Century Co., Inc.)"@en ;
  rdfs:label "sand size sediment"@en ;
  rdfs:subClassOf gslth:sediment ;
.
gslth:sapropel
  a owl:Class ;
  rdfs:comment "Jelly like organic rich sediment composed of plant remains, usually algal. Liptinite to Inertinite ratio is greater than one (Economic commission for Europe, committee on Sustainable Energy- United Nations (ECE-UN), 1998, International Classification of in-Seam Coals: Energy 19, 41 pp.)"@en ;
  rdfs:comment "dct:source--  Neuendorf et al. 2005"@en ;
  rdfs:label "sapropel"@en ;
  rdfs:subClassOf gslth:organic_rich_sediment ;
.
gslth:schist
  a owl:Class ;
  rdfs:comment "Foliated phaneritic metamorphic rock with well developed, continuous schistosity, meaning that greater than 50 percent of the rock by volume is mineral grains with a thin tabular, lamellar, or acicular prismatic crystallographic habit that are oriented in a continuous planar or linear fabric."@en ;
  rdfs:comment "dct:source--  SLTTm 2004; Neuendorf et al. 2005"@en ;
  rdfs:label "schist"@en ;
  rdfs:subClassOf gslth:foliated_metamorphic_rock ;
.
gslth:sediment
  a owl:Class ;
  rdfs:comment "Unconsolidated material consisting of an aggregation of particles transported or deposited by air, water or ice, or that accumulated by other natural agents, such as chemical precipitation, and that forms in layers on the Earth's surface. Includes epiclastic deposits."@en ;
  rdfs:comment "dct:source--  SLTTs 2004"@en ;
  rdfs:label "sediment"@en ;
  rdfs:subClassOf gslth:natural_unconsolidated_material ;
  rdfs:subClassOf gslth:sedimentary_material ;
.
gslth:sedimentary_material
  a owl:Class ;
  rdfs:comment "Material formed by accumulation of solid fragmental material deposited by air, water or ice, or material that accumulated by other natural agents such as chemical precipitation from solution or secretion by organisms. Includes both sediment and sedimentary rock. Includes epiclastic deposits. All stated composition criteria are based on the mineral/ compound material (GeoSciML term)/particulate fraction of the material, irrespective of porosity or the pore-fluid. No distinctions are made based on porosity or pore fluid composition (except organic rich sediment in which liquid hydrocarbon content may be considered)."@en ;
  rdfs:comment "dct:source--  SLTTs 2004"@en ;
  rdfs:label "sedimentary material"@en ;
  rdfs:subClassOf gslth:compound_material ;
.
gslth:sedimentary_rock
  a owl:Class ;
  rdfs:comment "Rock formed by accumulation and cementation of solid fragmental material deposited by air, water or ice, or as a result of other natural agents, such as precipitation from solution, the accumulation of organic material, or from biogenic processes, including secretion by organisms. Includes epiclastic deposits."@en ;
  rdfs:comment "dct:source--  SLTTs 2004"@en ;
  rdfs:label "sedimentary rock"@en ;
  rdfs:subClassOf gslth:rock ;
  rdfs:subClassOf gslth:sedimentary_material ;
.
gslth:serpentinite
  a owl:Class ;
  rdfs:comment "Rock consisting of more than 75 percent serpentine-group minerals, eg. antigorite, chrysotile or lizardite; accessory chlorite, talc and magnetite may be present; derived from hydration of ferromagnesian silicate minerals such as olivine and pyroxene."@en ;
  rdfs:comment "dct:source--  Neuendorf et al. 2005"@en ;
  rdfs:label "serpentinite"@en ;
  rdfs:subClassOf gslth:metamorphic_rock ;
.
gslth:shale
  a owl:Class ;
  rdfs:comment "Laminated mudstone that will part or break along thin, closely spaced layers parallel to stratification."@en ;
  rdfs:comment "Note definition does not specify carbonate vs. siliclastic nature of mud."@en ;
  rdfs:comment "dct:source--  NADM SLTT sedimentary, 2004"@en ;
  rdfs:label "shale"@en ;
  rdfs:subClassOf gslth:clastic_mudstone ;
.
gslth:silicate_mud
  a owl:Class ;
  rdfs:comment "Mud size sediment that consists of less than 50 percent carbonate minerals."@en ;
  rdfs:comment "dct:source--  This vocabulary"@en ;
  rdfs:label "silicate mud"@en ;
  rdfs:subClassOf gslth:mud_size_sediment ;
.
gslth:silicate_mudstone
  a owl:Class ;
  rdfs:comment "Mudstone that contains less than 10 percent carbonate minerals."@en ;
  rdfs:comment "Operational distinction of this category will typically be based on whether or not the rock fizzes when hydrochloric acid is applied--the rock is silicate mudstone if it does not fizz. The quantitative '10 percent' criteria is fuzzy."@en ;
  rdfs:comment "dct:source--  This vocabulary"@en ;
  rdfs:label "silicate mudstone"@en ;
  rdfs:subClassOf gslth:generic_mudstone ;
.
gslth:siliceous_ooze
  a owl:Class ;
  rdfs:comment "dct:source--  This vocabulary"@en ;
  rdfs:comment "ooze that consists of more than 50 percent siliceous skeletal remains"@en ;
  rdfs:label "siliceous ooze"@en ;
  rdfs:subClassOf gslth:ooze ;
  rdfs:subClassOf gslth:silicate_mud ;
.
gslth:silt
  a owl:Class ;
  a owl:NamedIndividual ;
  rdfs:comment "Mud that consists of greater than 50 percent silt-size grains."@en ;
  rdfs:comment "dct:source--  based on SLTTs 2004; Neuendorf et al. 2005; particle size from Wentworth grade scale"@en ;
  rdfs:comment "skos:altLabel--  loess"@en ;
  rdfs:label "silt"@en ;
  rdfs:subClassOf gslth:mud ;
.
gslth:siltstone
  a owl:Class ;
  a owl:NamedIndividual ;
  rdfs:comment "Mudstone that contains detectable silt. (see comments)"@en ;
  rdfs:comment "Use of 'dectable silt' in the criteria for this category is based on the observation that in practice, distinction of claystone from 'siltstone' is typically based on a qualitative assessment of 'grittiness' (e.g. rubbing with fingers, or chewing); the property that these tests can determine is the presence or absence of silty particles in the material. Quantitative grain size analysis in the the clay/silt fraction of a lithified sediment is difficult at best, and of questionable significance because diagensis has altered the size and mineralogy of original sedimentary particles."@en ;
  rdfs:comment "dct:source--  This vocabulary"@en ;
  rdfs:comment "skos:altLabel--  Silt bearing mudstone"@en ;
  rdfs:label "siltstone"@en ;
  rdfs:subClassOf gslth:clastic_mudstone ;
.
gslth:skarn
  a owl:Class ;
  a owl:NamedIndividual ;
  rdfs:comment "Metasomatic rock consisting mainly of Ca-, Mg-, Fe-, or Mn-silicate minerals, which are free from or poor in water. Typically formed at the contact between a silicate rock or magma and a carbonate rock."@en ;
  rdfs:comment "dct:source--  Fettes and Desmons, 2007, p195"@en ;
  rdfs:comment "skos:altLabel--  exoskarn"@en ;
  rdfs:comment "skos:altLabel--  tactite"@en ;
  rdfs:label "skarn"@en ;
  rdfs:subClassOf gslth:metasomatic_rock ;
.
gslth:slate
  a owl:Class ;
  rdfs:comment "compact, fine grained rock with an average grain size less than 0.032 millimeter and a well developed schistosity (slaty cleavage), and hence can be split into slabs or thin plates."@en ;
  rdfs:comment "dct:source--  NADM metamorphic rock vocabulary SLTTm1.0; Neuendorf et al. 2005"@en ;
  rdfs:label "slate"@en ;
  rdfs:subClassOf gslth:foliated_metamorphic_rock ;
.
gslth:spilite
  a owl:Class ;
  rdfs:comment "Altered basic to intermediate composition fine-grained igneous rock in which the feldspar is partially or completely composed of of albite, typically accompanied by chlorite, calcite, quartz, epidote, prehnite, and low-tempaerature hydrous crystallization products. Preservation of eruptive volcanic features is typical."@en ;
  rdfs:comment "dct:source--  Fettes and Desmon, 2007; Best, M.G., 1982, Igneous and metamorphic petrology: New York, W.H. Freeman and company, p. 398; Neuendorf et al. 2005, p. 619."@en ;
  rdfs:label "spilite"@en ;
  rdfs:subClassOf gslth:metasomatic_rock ;
.
gslth:syenite
  a owl:Class ;
  rdfs:comment "Syenitic rock that contains between 0 and 5 percent quartz and no feldspathoid mineral in the QAPF fraction. Defined modally in QAPF Field 7."@en ;
  rdfs:comment "dct:source--  LeMaitre et al. 2002"@en ;
  rdfs:label "syenite"@en ;
  rdfs:subClassOf gslth:syenitic_rock ;
.
gslth:syenitic_rock
  a owl:Class ;
  rdfs:comment "Syenitoid with a plagioclase to total feldspar ratio between 0.1 and 0.35. Includes rocks in QAPF fields 7, 7*, and 7'."@en ;
  rdfs:comment "dct:source--  LeMaitre et al. 2002"@en ;
  rdfs:label "syenitic rock"@en ;
  rdfs:subClassOf gslth:syenitoid ;
.
gslth:syenitoid
  a owl:Class ;
  rdfs:comment "Phaneritic crystalline igneous rock with M less than 90, consisting mainly of alkali feldspar and plagioclase; minor quartz or nepheline may be present, along with pyroxene, amphibole or biotite. Ratio of plagioclase to total feldspar is less than 0.65, quartz forms less than 20 percent of QAPF fraction, and feldspathoid minerals form less than 10 percent of QAPF fraction. Includes rocks classified in QAPF fields 6, 7 and 8 and their subdivisions."@en ;
  rdfs:comment "dct:source--  LeMaitre et al. 2002"@en ;
  rdfs:label "syenitoid"@en ;
  rdfs:subClassOf gslth:phaneritic_igneous_rock ;
.
gslth:syenogranite
  a owl:Class ;
  rdfs:comment "Granite that has a plagiolcase to total feldspar ratio between 0.10 and 0.35. QAPF field 3a."@en ;
  rdfs:comment "dct:source--  LeMaitre et al. 2002"@en ;
  rdfs:label "syenogranite"@en ;
  rdfs:subClassOf gslth:granite ;
.
gslth:tephra
  a owl:Class ;
  rdfs:comment "Unconsolidated pyroclastic material in which greater than 75 percent of the fragments are deposited as a direct result of volcanic processes and the deposit has not been reworked by epiclastic processes. Includes ash, lapilli tephra, bomb tephra, block tephra and unconsolidated agglomerate."@en ;
  rdfs:comment "dct:source--  Hallsworth and Knox 1999; LeMaitre et al. 2002"@en ;
  rdfs:label "tephra"@en ;
  rdfs:subClassOf gslth:natural_unconsolidated_material ;
  rdfs:subClassOf gslth:pyroclastic_material ;
.
gslth:tephrite
  a owl:Class ;
  rdfs:comment "Tephritoid that has a plagioclase to total feldspar ratio greater than 0.9, and contains less than 10 percent normative (CIPW) olivine."@en ;
  rdfs:comment "dct:source--  LeMaitre et al. 2002"@en ;
  rdfs:label "tephrite"@en ;
  rdfs:subClassOf gslth:tephritoid ;
.
gslth:tephritic_foidite
  a owl:Class ;
  rdfs:comment "Foiditoid that contains less than 90 percent feldspathoid minerals in the QAPF fraction, and has a plagioclase to total feldspar ratio that is greater than 0.5, with less than 10 percent normative olivine"@en ;
  rdfs:comment "dct:source--  LeMaitre et al. 2002"@en ;
  rdfs:label "tephritic foidite"@en ;
  rdfs:subClassOf gslth:foiditoid ;
.
gslth:tephritic_phonolite
  a owl:Class ;
  rdfs:comment "Phonolitoid that has a plagioclase to total feldspar ratio between 0.1 and 0.5. Broadly corresponds to TAS tephriphonolite of TAS field U3."@en ;
  rdfs:comment "dct:source--  LeMaitre et al. 2002"@en ;
  rdfs:label "tephritic phonolite"@en ;
  rdfs:subClassOf gslth:phonolitoid ;
.
gslth:tephritoid
  a owl:Class ;
  a owl:NamedIndividual ;
  rdfs:comment "Fine grained igneous rock than contains less than 90 percent mafic minerals, between 10 and 60 percent feldspathoid mineral in the QAPF fraction and has a plagioclase to total feldspar ratio greater than 0.5. Includes rocks classified in QAPF field 13 and 14 or chemically in TAS field U1 as basanite or tephrite."@en ;
  rdfs:comment "dct:source--  LeMaitre et al. 2002"@en ;
  rdfs:comment "skos:altLabel--  tephritic rock"@en ;
  rdfs:label "tephritoid"@en ;
  rdfs:subClassOf gslth:fine_grained_igneous_rock ;
.
gslth:tholeiitic_basalt
  a owl:Class ;
  rdfs:comment "Definition of tholeiite and alkali basalt here are more proscriptive than those found in most reference authorities. This is to actually provide some descriptive criteria to allow assignment of rocks on a hand sample basis to the tholeiite or alkali basalt categories if detailed petrographic or chemical data are available."@en ;
  rdfs:comment "Tholeiitic basalt is defined here to contain 2 pyroxene phases and interstitial quartz or tridymite or cristobalite in the groundmass. Pyroxene (augite and orthopyroxene or pigeonite) and calcium-rich plagioclase are common phenocryst minerals. Olivine may also be a phenocryst, and when present, may have rims of pigeonite. Only in tholeiitic basalt is olivine in reaction relationship with melt. Interstitial siliceous residue may be present, and is often glassy. Tholeiitic basalt is relatively poor in sodium. This category includes most basalts of the ocean floor, most large oceanic islands, and continental flood basalts such as the Columbia River Plateau."@en ;
  rdfs:comment "dct:source--  http://en.wikipedia.org/wiki/Basalt; Carmichael, I.S. Turner, F.J., Verhoogen, John, 1974, Igneous petrology: New York, McGraw HIll Book Co., p.42-43."@en ;
  rdfs:label "tholeiitic basalt"@en ;
  rdfs:subClassOf gslth:basalt ;
.
gslth:tonalite
  a owl:Class ;
  rdfs:comment "Granitoid consisting of quartz and intermediate plagioclase, usually with biotite and amphibole. Includes rocks defined modally in QAPF field 5; ratio of plagioclase to total feldspar is greater than 0.9."@en ;
  rdfs:comment "dct:source--  LeMaitre et al. 2002"@en ;
  rdfs:label "tonalite"@en ;
  rdfs:subClassOf gslth:granitoid ;
.
gslth:trachyte
  a owl:Class ;
  rdfs:comment "Trachytoid that has a plagioclase to total feldspar ratio between 0.1 and 0.35, between 0 and 5 percent quartz in the QAPF fraction, and no feldspathoid minerals. QAPF field 7."@en ;
  rdfs:comment "dct:source--  LeMaitre et al. 2002"@en ;
  rdfs:label "trachyte"@en ;
  rdfs:subClassOf gslth:trachytic_rock ;
.
gslth:trachytic_rock
  a owl:Class ;
  rdfs:comment "LeMaitre et al. (2002) used 'trachyte' to refer to QAPF fields 7, 7', and 7* in the text (p. 30) as well as to the more restrictive category (QAPF field 7 only). The term Trachytic rock is introduced here to label this more general category of trachyte."@en ;
  rdfs:comment "Trachytoid that has a plagioclase to total feldspar ratio between 0.1 and 0.35. QAPF fields 7, 7', and 7*."@en ;
  rdfs:comment "dct:source--  LeMaitre et al. 2002"@en ;
  rdfs:label "trachytic rock"@en ;
  rdfs:subClassOf gslth:trachytoid ;
.
gslth:trachytoid
  a owl:Class ;
  rdfs:comment "Fine grained igneous rock than contains less than 90 percent mafic minerals, less than 10 percent feldspathoid mineral and less than 20 percent quartz in the QAPF fraction and has a plagioclase to total feldspar ratio less than 0.65. Mafic minerals typically include amphibole or mica; typically porphyritic. Includes rocks defined modally in QAPF fields 6, 7 and 8 (with subdivisions) or chemically in TAS Field T as trachyte or latite."@en ;
  rdfs:comment "dct:source--  LeMaitre et al. 2002"@en ;
  rdfs:label "trachytoid"@en ;
  rdfs:subClassOf gslth:fine_grained_igneous_rock ;
.
gslth:travertine
  a owl:Class ;
  rdfs:comment "Biotically or abiotically precipitated calcium carbonate, from spring-fed, heated, or ambient-temperature water. May be white and spongy, various shades of orange, tan or gray, and ranges to dense, banded or laminated rock. Macrophytes, bryophytes, algae, cyanobacteria and other organisms often colonize the surface of travertine and may be preserved, to produce the porous varieties."@en ;
  rdfs:comment "dct:source--  Neuendorf et al. 2005; http://en.wikipedia.org/wiki/Travertine; Chafetz, H.S., and Folk, R.L., 1984, Travertine: Depositional morphology an dthe bacterially constructed constituents: J. Sed. Petrology, v. 126, p.57-74."@en ;
  rdfs:label "travertine"@en ;
  rdfs:subClassOf gslth:chemical_sedimentary_material ;
  rdfs:subClassOf gslth:limestone ;
.
gslth:tuff_breccia_agglomerate_or_pyroclastic_breccia
  a owl:Class ;
  rdfs:comment "Pyroclastic rock in which greater than 25 percent of particles are greater than 64 mm in largest dimension. Includes agglomerate, pyroclastic breccia of Gillespie and Styles (1999)"@en ;
  rdfs:comment "dct:source--  Schmid 1981; LeMaitre et al. 2002"@en ;
  rdfs:label "tuff breccia agglomerate or pyroclastic breccia"@en ;
  rdfs:subClassOf gslth:pyroclastic_rock ;
.
gslth:tuffite
  a owl:Class ;
  rdfs:comment "In practice, it is likely that any rock for which there is suspicion that it may consist of redeposited pyroclastic material, usually based on sedimentary structures, irrespective of the presence or percentage of clearly epiclastic particles, would be called a tuffite. 50 percent cutoff with epiclastic rock is in contrast with LeMaitre et al., but is used for consistentency with other sedimentary rock categories following the pattern that the rock name reflects the predominant constituent."@en ;
  rdfs:comment "Rock consists of more than 50 percent particles of indeterminate pyroclastic or epiclastic origin and less than 75 percent particles of clearly pyroclastic origin. commonly the rock is laminated or exhibits size grading. (based on LeMaitre et al. 2002; Murawski and Meyer 1998)."@en ;
  rdfs:comment "dct:source--  LeMaitre et al. 2002; Murawski and Meyer 1998"@en ;
  rdfs:label "tuffit"@de ;
  rdfs:label "tuffite"@en ;
  rdfs:subClassOf gslth:rock ;
.
gslth:ultrabasic_igneous_rock
  a owl:Class ;
  rdfs:comment "Igneous rock with less than 45 percent SiO2."@en ;
  rdfs:comment "dct:source--  after LeMaitre et al. 2002"@en ;
  rdfs:label "ultrabasic igneous rock"@en ;
  rdfs:subClassOf gslth:igneous_rock ;
.
gslth:ultramafic_igneous_rock
  a owl:Class ;
  rdfs:comment "Igneous rock that consists of greater than 90 percent mafic minerals."@en ;
  rdfs:comment "dct:source--  LeMaitre et al. 2002; Gillespie and Styles 1999"@en ;
  rdfs:label "ultramafic igneous rock"@en ;
  rdfs:subClassOf gslth:igneous_rock ;
.
gslth:unconsolidated_material
  a owl:Class ;
  rdfs:comment "compoundMaterial composed of an aggregation of particles that do not adhere to each other strongly enough that the aggregate can be considered a solid in its own right."@en ;
  rdfs:comment "dct:source--  This vocabulary"@en ;
  rdfs:label "unconsolidated material"@en ;
  rdfs:subClassOf gslth:compound_material ;
.
gslth:wacke
  a owl:Class ;
  rdfs:comment "Clastic sandstone with more than 10 percent matrix of indeterminate detrital or diagenetic nature. Matrix is mud size silicate minerals (clay, feldspar, quartz, rock fragments, and alteration products)."@en ;
  rdfs:comment "Distinction from mudstone is based on inference that less that 50 percent of the mud size fraction (matrix) is original mud size detrital particles. May also grade into diamictite or conglomerate based on size distribution of discernible particles. If more than 50 percent of rock is detrital particles of intrabasinal orgin and carbonate composition, categorize as carbonate wackestone. Term is typically applied to diagenetically altered volcanic-lithic clastic rocks in which the definition of the original clasts has been obscured. Suggested boundaries between wacke and arenite range from 5 to 15 percent matrix. See Dickinson (1970) for discussion of interpretation of undiscernible matrix in diagenetically altered lithic clastic rocks. Dickinson, W.R., 1970, Interpreting detrital modes of graywacke and arkose: Journal of Sedimentary Petrology, v. 40, p. 695-707."@en ;
  rdfs:comment "dct:source--  Pettijohn, Potter, Siever, 1972, Sand and Sandstone: New York, Springer Verlag, 681 p."@en ;
  rdfs:label "piedra"@es ;
  rdfs:label "wacke"@en ;
  rdfs:subClassOf gslth:clastic_sandstone ;
.
gsmg:metamorphosed
  rdfs:subClassOf gsop:Metamorphic_Grade ;
.
gsmg:not_metamorphosed
  rdfs:subClassOf gsop:Metamorphic_Grade ;
.
