# baseURI: http://loop3d.org/GSO/ontology/2020/1/hydrology/ontology
# imports: http://loop3d.org/GSO/ontology/2020/1/common/ontology

@prefix : <http://loop3d.org/GSO/ontology/2020/1/hydrology/> .
@prefix gsoc: <http://loop3d.org/GSO/ontology/2020/1/common/> .
@prefix gsoh: <http://loop3d.org/GSO/ontology/2020/1/hydrology/> .
@prefix owl: <http://www.w3.org/2002/07/owl#> .
@prefix rdf: <http://www.w3.org/1999/02/22-rdf-syntax-ns#> .
@prefix rdfs: <http://www.w3.org/2000/01/rdf-schema#> .
@prefix dct: <http://purl.org/dc/terms/> .
@prefix skos: <http://www.w3.org/2004/02/skos/core#> .
@prefix xsd: <http://www.w3.org/2001/XMLSchema#> .

gsoh:Hydrologic_Event
  rdf:type owl:Class ;
  rdfs:label "Hydrologic Event"@en ;
  rdfs:subClassOf gsoc:Event ;
.
gsoh:Hydrologic_Process
  rdf:type owl:Class ;
  rdfs:label "Hydrologic Process"@en ;
  rdfs:subClassOf gsoc:Process ;
  rdfs:comment "Process that has a water entity as an output.  Water entities include things such as rivers, lakes, ocean, clouds, aquifers as well as various qualities like river stage, mean sea level."@en ;
.
gsoh:Sea_Level_Fluctuation
  rdf:type owl:Class ;
  rdfs:comment "process of alteration of global sea levels due to changes in either the volume of water in the world's oceans or net changes in the volume of the oceanic basins."@en ;
  rdfs:label "Sea Level Fluctuation"@en ;
  rdfs:subClassOf gsoh:Hydrologic_Process ;
.
gsoh:ontology
  rdf:type owl:Ontology ;
  rdfs:comment "Hydrology ontology"@en ;
  rdfs:label "Geoscience Ontology, Hydrology "@en ;
  owl:imports gsoc:ontology ;
    skos:definition "Shell for hydrogeology module in Geoscience Ontology"@en ;
  skos:prefLabel "Geoscience Ontology, Geoscience Ontology, "@en ;
  dct:created "2020-01-30"^^xsd:date ;
  dct:creator gsoc:boyan_brodaric ;
  dct:creator gsoc:stephen_richard ;
  dct:license <https://creativecommons.org/licenses/by/4.0/legalcode> ;
  dct:modified "2021-03-10"^^xsd:date ;
  dct:publisher "Loop3D project;  https://loop3d.org/" ;
  dct:publisher "Natural Resources Canada, Geological Survey of Canada" ;
.
:stephen_richard
  rdf:type owl:NamedIndividual ;
  rdfs:comment "e-mail: mailto:smrTucson@gmail.com " ;
  rdfs:comment "orchid-id: https://orcid.org/0000-0001-6041-5302" ;
  rdfs:label "Dr. Stephen M. Richard" ;
.
:boyan_brodaric
  rdf:type owl:NamedIndividual ;
  rdfs:comment "affiliation:  Natural Resources Canada, Geological Survey of Canada" ;
  rdfs:comment "e-mail: mailto:boyan.brodaric@canada.ca " ;
  rdfs:comment "orchid-id: https://orcid.org/0000-0002-7987-3810" ;
  rdfs:label "Dr. Boyan Brodaric" ;
.

