# baseURI: http://loop3d.org/GSO/ontology/2020/1/geologicstructure/contact/ontology

@prefix gscn: <http://loop3d.org/GSO/ontology/2020/1/geologicstructure/contact/> .
@prefix gsoc: <http://loop3d.org/GSO/ontology/2020/1/common/> .
@prefix gsog: <http://loop3d.org/GSO/ontology/2020/1/geologicfeature/> .
@prefix owl: <http://www.w3.org/2002/07/owl#> .
@prefix rdf: <http://www.w3.org/1999/02/22-rdf-syntax-ns#> .
@prefix rdfs: <http://www.w3.org/2000/01/rdf-schema#> .
@prefix xml: <http://www.w3.org/XML/1998/namespace> .
@prefix xsd: <http://www.w3.org/2001/XMLSchema#> .

gscn:Alteration_Facies_Contact
  a owl:Class ;
  rdfs:comment "A metasomatic facies contact separating rocks that have undergone alteration of a particular facies from those that have undergone metasomatism of another facies. Alteration is a kind of metasomatism that does not introduce economically important minerals."@en ;
  rdfs:comment "dct:source--  CGI contacttype SKOS vocabulary 2012-11-24"@en ;
  rdfs:label "alteration facies contact"@en ;
  rdfs:subClassOf gscn:Metamorphic_Contact ;
.
gscn:Angular_Unconformable_Contact
  a owl:Class ;
  rdfs:comment "An unconformable contact between two geological units in which the older, underlying rocks dip at an angle different from the younger, overlying strata, usually in which younger sediments rest upon the eroded surface of tilted or folded older rocks."@en ;
  rdfs:comment "dct:source--  Neuendorf, K.K.E, Mehl, J.P. & Jackson, J.A. (eds), 2005. Glossary of geology, 5th Edition. American Geological Institute, Alexandria, 779 p."@en ;
  rdfs:label "angular unconformable contact"@en ;
  rdfs:subClassOf gscn:Unconformable_Contact ;
.
gscn:Buttress_Unconformity
  a owl:Class ;
  rdfs:comment "An unconformity in which onlapping strata are truncated against a steep topographic scarp."@en ;
  rdfs:comment "dct:source--  Neuendorf, K.K.E, Mehl, J.P. & Jackson, J.A. (eds), 2005. Glossary of geology, 5th Edition. American Geological Institute, Alexandria, 779 p."@en ;
  rdfs:label "buttress unconformity"@en ;
  rdfs:subClassOf gscn:Unconformable_Contact ;
.
gscn:Chronostratigraphic_Zone_Contact
  a owl:Class ;
  rdfs:comment "A contact between bodies of material having different ages of origin."@en ;
  rdfs:comment "dct:source--  FGDC"@en ;
  rdfs:label "chronostratigraphic-zone contact"@en ;
  rdfs:subClassOf gsog:Contact ;
.
gscn:Conductivity_Contact
  a owl:Class ;
  rdfs:comment "A geophysical contact between bodies of material distinguished based on electrical conductivity characteristics"@en ;
  rdfs:comment "dct:source--  CGI contacttype SKOS vocabulary 2012-11-24"@en ;
  rdfs:label "conductivity contact"@en ;
  rdfs:subClassOf gscn:Geophysical_Contact ;
.
gscn:Conformable_Contact
  a owl:Class ;
  rdfs:comment "A contact separating two geological units in which the layers are formed one above the other in order by regular, uninterrupted deposition under the same general conditions."@en ;
  rdfs:comment "dct:source--  Neuendorf, K.K.E, Mehl, J.P. & Jackson, J.A. (eds), 2005. Glossary of geology, 5th Edition. American Geological Institute, Alexandria, 779 p."@en ;
  rdfs:label "conformable contact"@en ;
  rdfs:subClassOf gscn:Depositional_Contact ;
.
gscn:Deformation_Zone_Contact
  a owl:Class ;
  rdfs:comment "A lithogenetic bundary separating rock masses that have different deformation structure, e.g. sheared rock against non sheared rock, brecciated rock against non-brecciated rock."@en ;
  rdfs:comment "dct:source--  CGI contacttype SKOS vocabulary 2012-11-24"@en ;
  rdfs:label "deformation zone contact"@en ;
  rdfs:subClassOf gscn:Lithogenetic_Contact ;
.
gscn:Density_Contact
  a owl:Class ;
  rdfs:comment "A geophysical contact separating bodies of material with different density characteristics, generally determined through measurement and modelling of gravity variations."@en ;
  rdfs:comment "dct:source--  CGI contacttype SKOS vocabulary 2012-11-24"@en ;
  rdfs:label "density contact"@en ;
  rdfs:subClassOf gscn:Geophysical_Contact ;
.
gscn:Depositional_Contact
  a owl:Class ;
  rdfs:comment "Lithogenetic contact at which a sedimentary or volcanic rock has been deposited on (or against) another rock body. The relationship between the older underlying rocks and younger overlying rocks is unknown or not specfied."@en ;
  rdfs:comment "dct:source--  CGI contacttype SKOS vocabulary 2012-11-24"@en ;
  rdfs:label "depositional contact"@en ;
  rdfs:subClassOf gscn:Lithogenetic_Contact ;
.
gscn:Disconformable_Contact
  a owl:Class ;
  rdfs:comment "An unconformable contact between two geological units in which the bedding of the older, underlying unit is parallel to the bedding of the younger, overlying unit, but in which the contact between the two units is marked by an irregular or uneven surface of appreciable relief."@en ;
  rdfs:comment "dct:source--  Neuendorf, K.K.E, Mehl, J.P. & Jackson, J.A. (eds), 2005. Glossary of geology, 5th Edition. American Geological Institute, Alexandria, 779 p."@en ;
  rdfs:label "disconformable contact"@en ;
  rdfs:subClassOf gscn:Unconformable_Contact ;
.
gscn:Faulted_Contact
  a owl:Class ;
  rdfs:comment "A contact separating two bodies of material across which one body has slid past the other."@en ;
  rdfs:comment "dct:source--  Neuendorf, K.K.E, Mehl, J.P. & Jackson, J.A. (eds), 2005. Glossary of geology, 5th Edition. American Geological Institute, Alexandria, 779 p."@en ;
  rdfs:label "faulted contact"@en ;
  rdfs:subClassOf gsog:Contact ;
.
gscn:Geologic_Province_Contact
  a owl:Class ;
  rdfs:comment "A contact between regions characterised by their geological history or by similar structural, petrographic or stratigraphic features"@en ;
  rdfs:comment "dct:source--  Neuendorf, K.K.E, Mehl, J.P. & Jackson, J.A. (eds), 2005. Glossary of geology, 5th Edition. American Geological Institute, Alexandria, 779 p."@en ;
  rdfs:label "geologic province contact"@en ;
  rdfs:subClassOf gsog:Contact ;
.
gscn:Geophysical_Contact
  a owl:Class ;
  rdfs:comment "A contact separating bodies of material in the earth that have different geophysical properties. Use for boundaries that are detected by geophysical sensor techniques as opposed to direct lithologic observation."@en ;
  rdfs:comment "dct:source--  CGI contacttype SKOS vocabulary 2012-11-24"@en ;
  rdfs:label "geophysical contact"@en ;
  rdfs:subClassOf gsog:Contact ;
.
gscn:Glacial_Stationary_Line
  a owl:Class ;
  rdfs:comment "A boundary between a subglacial geomorphic unit and a periglacial geomorphic unit, marking the maximum extent of glacial cover. This can be thought of as the outcrop of the contact between a glacier and its substrate at some time at each point along the boundary. This contact type is included as an interim concept, assuming that in the future, there will be extensions to account better for geomorphic units and line types."@en ;
  rdfs:comment "dct:source--  CGI contacttype SKOS vocabulary 2012-11-24"@en ;
  rdfs:label "glacial stationary line"@en ;
  rdfs:subClassOf gsog:Contact ;
.
gscn:Igneous_Intrusive_Contact
  a owl:Class ;
  rdfs:comment "An intrusive contact between a younger igneous rock and an older, pre-existing geological unit into which it has been intruded."@en ;
  rdfs:comment "dct:source--  Neuendorf, K.K.E, Mehl, J.P. & Jackson, J.A. (eds), 2005. Glossary of geology, 5th Edition. American Geological Institute, Alexandria, 779 p."@en ;
  rdfs:label "igneous intrusive contact"@en ;
  rdfs:subClassOf gscn:Lithogenetic_Contact ;
.
gscn:Igneous_Phase_Contact
  a owl:Class ;
  rdfs:comment "A lithogenetic contact separating lithologically distinct phases of a single intrusive body. Does not denote nature of contact (intrusive or gradation)."@en ;
  rdfs:comment "dct:source--  CGI contacttype SKOS vocabulary 2012-11-24"@en ;
  rdfs:label "igneous phase contact"@en ;
  rdfs:subClassOf gscn:Lithogenetic_Contact ;
.
gscn:Impact_Structure_Boundary
  a owl:Class ;
  rdfs:comment "dct:source--  CGI contacttype SKOS vocabulary 2012-11-24"@en ;
  rdfs:comment "surface that bounds a body of rock affected by an extraterrestrial impact event"@en ;
  rdfs:label "impact structure boundary"@en ;
  rdfs:subClassOf gscn:Lithogenetic_Contact ;
.
gscn:Lithogenetic_Contact
  a owl:Class ;
  rdfs:comment "A non-faulted contact separating bodies of material in the earth that have different lithologic character or geologic history."@en ;
  rdfs:comment "dct:source--  CGI contacttype SKOS vocabulary 2012-11-24"@en ;
  rdfs:label "lithogenetic contact"@en ;
  rdfs:subClassOf gsog:Contact ;
.
gscn:Magnetic_Contact
  a owl:Class ;
  rdfs:comment "A geophysical contact separating bodies of material distinguished based on properties related to magnetic fields."@en ;
  rdfs:comment "dct:source--  CGI contacttype SKOS vocabulary 2012-11-24"@en ;
  rdfs:label "magnetic contact"@en ;
  rdfs:subClassOf gscn:Geophysical_Contact ;
.
gscn:Magnetic_Polarity_Contact
  a owl:Class ;
  rdfs:comment "A magentic contact between bodies of material with different polarity of remnant magnetization, e.g. between sections of ocean floor with different polarity."@en ;
  rdfs:comment "dct:source--  CGI contacttype SKOS vocabulary 2012-11-24"@en ;
  rdfs:label "magnetic polarity contact"@en ;
  rdfs:subClassOf gscn:Magnetic_Contact ;
.
gscn:Magnetic_Susceptiblity_Contact
  a owl:Class ;
  rdfs:comment "A magnetic contact between bodies of material distinguished based on magnetic susceptibility characteristics."@en ;
  rdfs:comment "dct:source--  CGI contacttype SKOS vocabulary 2012-11-24"@en ;
  rdfs:label "magnetic susceptiblity contact"@en ;
  rdfs:subClassOf gscn:Magnetic_Contact ;
.
gscn:Magnetization_Contact
  a owl:Class ;
  rdfs:comment "A magnetic contact between bodies of material distinguished based on any aspect of magnetization of material in the units."@en ;
  rdfs:comment "dct:source--  CGI contacttype SKOS vocabulary 2012-11-24"@en ;
  rdfs:label "magnetization contact"@en ;
  rdfs:subClassOf gscn:Magnetic_Contact ;
.
gscn:Metamorphic_Contact
  a owl:Class ;
  rdfs:comment "Lithogenetic contact separating rocks that have different lithologic properties related to metamorphism, metasomatism, alteration, or mineralization. Generally separates metamorphic rock bodies, but may separate metamorphosed (broadly speaking) and non-metamorphosed rock."@en ;
  rdfs:comment "dct:source--  CGI contacttype SKOS vocabulary 2012-11-24"@en ;
  rdfs:label "metamorphic contact"@en ;
  rdfs:subClassOf gscn:Lithogenetic_Contact ;
.
gscn:Metamorphic_Facies_Contact
  a owl:Class ;
  rdfs:comment "A metamorphic contact separating rocks that have undergone metamorphism of a particular facies from those that have undergone metamorphism of another facies."@en ;
  rdfs:comment "dct:source--  CGI contacttype SKOS vocabulary 2012-11-24"@en ;
  rdfs:label "metamorphic facies contact"@en ;
  rdfs:subClassOf gscn:Metamorphic_Contact ;
.
gscn:Metasomatic_Facies_Contact
  a owl:Class ;
  rdfs:comment "A metamorphic contact separating rocks that have undergone metasomatism of a particular facies from those that have undergone metasomatism of another facies. Metasomatism is distinguished from metamorphism by significant changes in bulk chemistry of the affected rock."@en ;
  rdfs:comment "dct:source--  CGI contacttype SKOS vocabulary 2012-11-24"@en ;
  rdfs:label "metasomatic facies contact"@en ;
  rdfs:subClassOf gscn:Metamorphic_Contact ;
.
gscn:Mineralisation_Assemblage_Contact
  a owl:Class ;
  rdfs:comment "A metasomatic facies contact separating rocks which have been mineralised and contain a particular mineral assemblage from those which contain a different assemblage. Mineralization is a kind of metasomatism that introduces ecomomically important minerals."@en ;
  rdfs:comment "dct:source--  CGI contacttype SKOS vocabulary 2012-11-24"@en ;
  rdfs:label "mineralisation assemblage contact"@en ;
  rdfs:subClassOf gscn:Metamorphic_Contact ;
.
gscn:Nonconformable_Contact
  a owl:Class ;
  rdfs:comment "An unconformable contact between an underlying, older nonstratified geological unit (usually intrusive igneous rocks or metamorphics) and an overlying, younger stratified geological unit."@en ;
  rdfs:comment "dct:source--  Neuendorf, K.K.E, Mehl, J.P. & Jackson, J.A. (eds), 2005. Glossary of geology, 5th Edition. American Geological Institute, Alexandria, 779 p."@en ;
  rdfs:label "nonconformable contact"@en ;
  rdfs:subClassOf gscn:Unconformable_Contact ;
.
gscn:Paraconformable_Contact
  a owl:Class ;
  rdfs:comment "An unconformable contact between two geological units in which the bedding of the older, underlying unit is parallel to the bedding of the younger, overlying unit, in which the contact between the two units is planar, and may be coincident with a bedding plane."@en ;
  rdfs:comment "dct:source--  Neuendorf, K.K.E, Mehl, J.P. & Jackson, J.A. (eds), 2005. Glossary of geology, 5th Edition. American Geological Institute, Alexandria, 779 p."@en ;
  rdfs:label "paraconformable contact"@en ;
  rdfs:subClassOf gscn:Unconformable_Contact ;
.
gscn:Radiometric_Contact
  a owl:Class ;
  rdfs:comment "A geophysical contact separating bodies of material distinguished based on the characteristics of emitted of radiant energy related to radioactivity (e.g. gamma rays)."@en ;
  rdfs:comment "dct:source--  CGI contacttype SKOS vocabulary 2012-11-24"@en ;
  rdfs:label "radiometric contact"@en ;
  rdfs:subClassOf gscn:Geophysical_Contact ;
.
gscn:Sedimentary_Facies_Contact
  a owl:Class ;
  rdfs:comment "A lithogenetic contact separating essentially coeval sedimentary material bodies distinguished by characteristics reflecting different physical or chemical processes active at the time of deposition of the sediment."@en ;
  rdfs:comment "dct:source--  base on Nichols, Gary, 1999, Sedimentology and stratigraphy, Blackwell, p. 62-63."@en ;
  rdfs:label "sedimentary facies contact"@en ;
  rdfs:subClassOf gscn:Lithogenetic_Contact ;
.
gscn:Sedimentary_Intrusive_Contact
  a owl:Class ;
  rdfs:comment "An intrusive contact between a sedimentary rock unit and plastic sediment (e.g., clay, chalk, salt, gypsum, etc.), forced upward into it from underlying sediment"@en ;
  rdfs:comment "dct:source--  Neuendorf, K.K.E, Mehl, J.P. & Jackson, J.A. (eds), 2005. Glossary of geology, 5th Edition. American Geological Institute, Alexandria, 779 p."@en ;
  rdfs:label "sedimentary intrusive contact"@en ;
  rdfs:subClassOf gscn:Lithogenetic_Contact ;
.
gscn:Seismic_Contact
  a owl:Class ;
  rdfs:comment "A geophysical contact separating bodies of material defined based on their seismic character. Seismic character is based on transmission of vibrations (seismic waves) through a rock body, and relates to the velocity of transmission, and the nature of reflection, refraction, or transformation of seismic waves by inhomogeneities in the rock body."@en ;
  rdfs:comment "dct:source--  CGI contacttype SKOS vocabulary 2012-11-24"@en ;
  rdfs:label "seismic contact"@en ;
  rdfs:subClassOf gscn:Geophysical_Contact ;
.
gscn:Unconformable_Contact
  a owl:Class ;
  rdfs:comment "A contact separating two geological units in which the younger unit succeeds the older after a substantial hiatus in deposition."@en ;
  rdfs:comment "dct:source--  Neuendorf, K.K.E, Mehl, J.P. & Jackson, J.A. (eds), 2005. Glossary of geology, 5th Edition. American Geological Institute, Alexandria, 779 p."@en ;
  rdfs:label "unconformable contact"@en ;
  rdfs:subClassOf gscn:Depositional_Contact ;
.
gscn:Volcanic_Subsidence_Zone_Boundary
  a owl:Class ;
  rdfs:comment "boundary around a body of rock that is within a zone of subsidence or cratering produced by volcanic activity."@en ;
  rdfs:comment "dct:source--  this vocabulary, concept to encompass boundary of caldron, caldera, or crater."@en ;
  rdfs:label "volcanic subsidence zone boundary"@en ;
  rdfs:subClassOf gscn:Lithogenetic_Contact ;
.
gscn:Weathering_Contact
  a owl:Class ;
  rdfs:comment "A lithogenetic contact separating bodies of material differentiated based on lithologic properties related to weathering."@en ;
  rdfs:comment "dct:source--  CGI contacttype SKOS vocabulary 2012-11-24"@en ;
  rdfs:label "weathering contact"@en ;
  rdfs:subClassOf gscn:Lithogenetic_Contact ;
.
gscn:ontology
  a owl:Ontology ;
  rdfs:comment "This file contains the 2016 SKOS-RDF version of the CGI Contact Type vocabulary. Compilation and review in MS Excel spreadsheet, converted to MS Excel for SKOS generation using GSML_SKOS_fromXLS_2016.01.xslt."@en ;
  rdfs:comment "This vocabulary specifies Contact Type concepts, as defined by the IUGS Commission for Geoscience Information (CGI) Geoscience Terminology Working Group. Originally designed for use in the contactType property in GeoSciML Contact elements, adopt here as subClasses of gsog:Contact."@en ;
  rdfs:comment "dct:creator--  CGI Concept Definition Task Group, Stephen Richard Owl adoption for Loop3D project"@en ;
  rdfs:comment "dct:date--  2012-11-24"@en ;
  rdfs:comment "dct:modified-- 2020-01-29"@en ;
  rdfs:label "Contact Type"@en ;
.
