# baseURI: http://geoscience.ca/3D/ontology/2019/1/geologicproperty
# imports: http://geoscience.ca/3D/ontology/2019/1/common

@prefix : <http://geoscience.ca/3D/ontology/2019/1/geologicproperty/> .
@prefix geologicfeature: <http://geoscience.ca/3D/ontology/2019/1/geologicfeature/> .
@prefix gkoc: <http://geoscience.ca/3D/ontology/2019/1/common/> .
@prefix gkop: <http://geoscience.ca/3D/ontology/2019/1/geologicproperty/> .
@prefix owl: <http://www.w3.org/2002/07/owl#> .
@prefix rdf: <http://www.w3.org/1999/02/22-rdf-syntax-ns#> .
@prefix rdfs: <http://www.w3.org/2000/01/rdf-schema#> .
@prefix xml: <http://www.w3.org/XML/1998/namespace> .
@prefix xsd: <http://www.w3.org/2001/XMLSchema#> .

<http://geoscience.ca/3D/ontology/2019/1/geologicproperty>
  a owl:Ontology ;
  rdfs:comment "Vocabulary of geologic properties"@en ;
  owl:imports <http://geoscience.ca/3D/ontology/2019/1/common> ;
.
gkop:Alteration_Degree
  a owl:Class ;
  rdfs:comment "Specification of the strength of observed alteration." ;
  rdfs:isDefinedBy "GeoSciML v4" ;
  rdfs:label "Alteration degree" ;
  rdfs:subClassOf gkoc:Discrete_Physical_Property ;
.
gkop:Alteration_Distribution
  a owl:Class ;
  rdfs:comment "AlterationDistribution describes the spatial distribution or geometry of alteration zones. eg: patchy, spotted, banded, viens, vein breccia, pervasive, disseminated, etc" ;
  rdfs:isDefinedBy "GeoSciML v4" ;
  rdfs:label "Alteration distribution" ;
  rdfs:subClassOf gkoc:Discrete_Physical_Property ;
.
gkop:Alteration_Type
  a owl:Class ;
  rdfs:comment "Specification of alteration types (eg; potassic, argillic, advanced argillic)"@en ;
  rdfs:isDefinedBy "GeoSciML v4" ;
  rdfs:label "Alteration type" ;
  rdfs:subClassOf gkoc:Discrete_Physical_Property ;
.
gkop:Amount
  a owl:Class ;
  rdfs:subClassOf gkoc:Quantified_Physical_Property ;
.
gkop:Bedding_Pattern
  a owl:Class ;
  rdfs:comment "Term(s) specifying patterns of bedding thickness or relationships between bedding packages. (eg; thinning upward, thickening upward)" ;
  rdfs:isDefinedBy "GeoSciML v4" ;
  rdfs:label "Bedding pattern" ;
  rdfs:subClassOf gkoc:Discrete_Physical_Property ;
.
gkop:Bedding_Style
  a owl:Class ;
  rdfs:comment "Term(s) specifying patterns of bedding thickness or relationships between bedding packages. (eg; thinning upward, thickening upward)" ;
  rdfs:isDefinedBy "GeoSciML v4" ;
  rdfs:label "Bedding style" ;
  rdfs:subClassOf gkoc:Discrete_Physical_Property ;
.
gkop:Bedding_Thickness_Category
  a owl:Class ;
  rdfs:comment "Terms characterizing the thickness of bedding in the unit. " ;
  rdfs:isDefinedBy "GeoSciML v4" ;
  rdfs:label "Bedding thickness" ;
  rdfs:subClassOf gkoc:Discrete_Physical_Property ;
.
gkop:Consolidation_Degree
  a owl:Class ;
  rdfs:comment "A property that specifies the degree to which an aggregation of EarthMaterial particles is a distinct solid material. Consolidation and induration are related concepts specified by this property. They define a continuum from unconsolidated material to very hard rock. Induration is the degree to which a consolidated material is made hard, operationally determined by how difficult it is to break a piece of the material. Consolidated materials may have varying degrees of induration (NADMSC, 2004)" ;
  rdfs:isDefinedBy "GeoSciML v4" ;
  rdfs:label "Consolidation degree" ;
  rdfs:subClassOf gkoc:Discrete_Physical_Property ;
.
gkop:Contact_Character
  a owl:Class ;
  rdfs:comment "The character of the boundary, as opposed to its type. e.g. abrupt, gradational " ;
  rdfs:isDefinedBy "GeoSciML v4" ;
  rdfs:label "Contact character" ;
  rdfs:subClassOf gkoc:Discrete_Physical_Property ;
.
gkop:Dip
  a owl:Class ;
  rdfs:comment "" ;
  rdfs:label "Dip" ;
  rdfs:subClassOf gkoc:Quantified_Physical_Property ;
.
gkop:Dip_Direction
  a owl:Class ;
  rdfs:comment "" ;
  rdfs:label "Dip direction" ;
  rdfs:subClassOf gkoc:Quantified_Physical_Property ;
.
gkop:Displacement
  a owl:Class ;
  rdfs:subClassOf gkoc:Complex_Physical_Property ;
.
gkop:Fabric_Continuity
  a owl:Class ;
  rdfs:comment "Terms to distinguish continuous vs. disjunct cleavages" ;
  rdfs:isDefinedBy "GeoSciML v4" ;
  rdfs:label "Fabric continuity" ;
  rdfs:subClassOf gkoc:Discrete_Physical_Property ;
.
gkop:Fabric_Defining_Element
  a owl:Class ;
  rdfs:comment "Kinds of describable inhomogeneity in a rock body that may define a GeologicStructure.   Examples include Discontinuity, Shaped Surface, Oriented Particle, Material Boundary, and Layer.  " ;
  rdfs:isDefinedBy "GeoSciML v4" ;
  rdfs:label "Fabric defining element" ;
  rdfs:subClassOf gkoc:Discrete_Physical_Property ;
.
gkop:Fabric_Element_Spacing
  a owl:Class ;
  rdfs:comment "" ;
  rdfs:isDefinedBy "GeoSciML v3" ;
  rdfs:label "Fabric element spacing" ;
  rdfs:subClassOf gkoc:Quantified_Physical_Property ;
.
gkop:Fabric_Intensity
  a owl:Class ;
  rdfs:comment "How well the fabric is developed. Terms such as weak, moderate, strong." ;
  rdfs:isDefinedBy "GeoSciML v4" ;
  rdfs:label "Fabric intensity" ;
  rdfs:subClassOf gkoc:Discrete_Physical_Property ;
.
gkop:Fold_Amplitude
  a owl:Class ;
  rdfs:comment "" ;
  rdfs:label "Dip direction" ;
  rdfs:subClassOf gkoc:Quantified_Physical_Property ;
.
gkop:Fold_Genetic_Model
  a owl:Class ;
  rdfs:comment "e.g. similar, parallel" ;
  rdfs:isDefinedBy "GeoSciML v3" ;
  rdfs:label "Fold genetic model" ;
  rdfs:subClassOf gkoc:Discrete_Physical_Property ;
.
gkop:Fold_Limb_Shape
  a owl:Class ;
  rdfs:comment "Straight vs curved limbs, eg kink, chevron, sinusoidal, box" ;
  rdfs:isDefinedBy "GeoSciML v4" ;
  rdfs:label "Fold limb shape" ;
  rdfs:subClassOf gkoc:Discrete_Physical_Property ;
.
gkop:Fold_Symmetry
  a owl:Class ;
  rdfs:comment "Concordance or discordance of bisecting surface and axial surface, or ratio of length of limbs. Folded surface may have asymmetry defined by limb length ratio if inflection points are defined. Defintion based on bisecting surface/axial surface angle depends on having multiple surfaces defined such that the axial surface may be identified. (symmetric, assymetric)" ;
  rdfs:isDefinedBy "GeoSciML v4" ;
  rdfs:label "Fold symmetry" ;
  rdfs:subClassOf gkoc:Discrete_Physical_Property ;
.
gkop:Fold_Wavelength
  a owl:Class ;
  rdfs:comment "" ;
  rdfs:label "Fold wavelength" ;
  rdfs:subClassOf gkoc:Quantified_Physical_Property ;
.
gkop:Geologic_Unit_Body_Morphology
  a owl:Class ;
  rdfs:comment "The geometry or form of a GeologicUnit.  Examples include: dike (dyke), cone, fan, sheet, etc. Morphology is independent of the substance (EarthMaterial) that composes the GeologicUnit or process that formed it." ;
  rdfs:isDefinedBy "GeoSciML v4" ;
  rdfs:label "Body morphology" ;
  rdfs:subClassOf gkoc:Discrete_Physical_Property ;
.
gkop:Geologic_Unit_Composition_Category
  a owl:Class ;
  rdfs:comment "Composition-based classification that requires integrating the character of the unit over large area, not applicable at the rock-material/specimen level. Examples: alkalic, subaluminous, peraluminous, I-Type, carbonate, phosphate." ;
  rdfs:isDefinedBy "GeoSciML v4" ;
  rdfs:label "Composition category" ;
  rdfs:subClassOf gkoc:Discrete_Physical_Property ;
.
gkop:Geologic_Unit_Outcrop_Character
  a owl:Class ;
  rdfs:comment "Describes the nature of outcrops formed by a geologic unit. Examples: bouldery, cliff-forming, ledge-forming, slope-forming, poorly exposed" ;
  rdfs:isDefinedBy "GeoSciML v4" ;
  rdfs:label "Outcrop character" ;
  rdfs:subClassOf gkoc:Discrete_Physical_Property ;
.
gkop:Grain_Shape
  a owl:Class ;
  rdfs:label "Grain Shape"@en ;
  rdfs:subClassOf gkoc:Discrete_Physical_Property ;
  rdfs:subClassOf [
      a owl:Restriction ;
      owl:onProperty gkop:hasTermValue ;
      owl:someValuesFrom gkop:ParticleShape ;
    ] ;
.
gkop:Grain_Size
  a owl:Class ;
  rdfs:subClassOf gkoc:Quantified_Physical_Property ;
.
gkop:Grain_Size_Average
  a owl:Class ;
  rdfs:comment "mean diameter for grain size distribution "@en ;
  rdfs:label "Grain Size Average "@en ;
  rdfs:subClassOf gkop:Grain_Size ;
.
gkop:Grain_Size_Category
  a owl:Class ;
  rdfs:comment "grain size range expressed using a named size category vocabulary" ;
  rdfs:isDefinedBy "GeoSciML v3" ;
  rdfs:label "Grain size term" ;
  rdfs:subClassOf gkoc:Discrete_Physical_Property ;
.
gkop:Grain_Size_Max
  a owl:Class ;
  rdfs:comment "upper bound of 95% interval for grain size distribution "@en ;
  rdfs:label "Grain Size Maximum "@en ;
  rdfs:subClassOf gkop:Grain_Size ;
.
gkop:Grain_Size_Min
  a owl:Class ;
  rdfs:comment "lower bound of 95% interval for grain size distribution "@en ;
  rdfs:label "Grain Size Minimum "@en ;
  rdfs:subClassOf gkop:Grain_Size ;
.
gkop:Hinge_Line_Curvature
  a owl:Class ;
  rdfs:comment "Variation in orientation of fold hinge along trend of fold, distinguish sheath from cylindrical folds. Specify with terminology eg sheath, dome, basin, cylindrical."@en ;
  rdfs:isDefinedBy "GeoSciML v4" ;
  rdfs:label "Fold hinge line curvature" ;
  rdfs:subClassOf gkoc:Discrete_Physical_Property ;
.
gkop:Hinge_Shape
  a owl:Class ;
  rdfs:comment "Rounded vs. angular hinge zones; has to do with the proportion of the wavelength that is considered part of hinge" ;
  rdfs:isDefinedBy "GeoSciML v4" ;
  rdfs:label "Fold hinge shape" ;
  rdfs:subClassOf gkoc:Discrete_Physical_Property ;
.
gkop:LineOrientation
  a owl:Class ;
  rdfs:comment "specification of the orientation of a line in space, using a trend (bearing of horizontal projection of line relative to geographic north) and plunge (inclination of line measured positive downward in degrees from local horizontal).  TBD:  add 'isdirected property to indicate if the line is directed (e.g. sense of shear), values should be Boolean,"@en ;
  rdfs:label "Line orientation"@en ;
  rdfs:subClassOf gkop:Orientation ;
  rdfs:subClassOf [
      a owl:Restriction ;
      owl:onProperty gkoc:hasPhysicalProperty ;
      owl:someValuesFrom gkop:Plunge ;
    ] ;
  rdfs:subClassOf [
      a owl:Restriction ;
      owl:onProperty gkoc:hasPhysicalProperty ;
      owl:someValuesFrom gkop:Trend ;
    ] ;
.
gkop:Metamorphic_Facies
  a owl:Class ;
  rdfs:comment "Categories that characterize mineral assemblages indicative of certain metamorphic P-T conditions. Examples include Barrovian metasedimentary zones (eg: biotite facies, kyanite facies) or assemblages developed in rocks of more mafic composition (eg: greenschist facies, amphibolite facies)."@en ;
  rdfs:isDefinedBy "GeoSciML v4" ;
  rdfs:label "Metamorphic facies" ;
  rdfs:subClassOf gkoc:Discrete_Physical_Property ;
.
gkop:Metamorphic_Grade
  a owl:Class ;
  rdfs:comment "A term to indicate the intensity or rank of metamorphism applied to an EarthMaterial (eg: high metamorphic grade, low metamorphic grade). Indicates in a general way the P-T environment in which the metamorphism took place. Determination of metamorphic grade is based on mineral assemblages (ie, facies) present in a rock that are interpreted to have crystallized in equilibrium during a particular metamorphic event."@en ;
  rdfs:isDefinedBy "GeoSciML v4" ;
  rdfs:label "Metamorphic grade" ;
  rdfs:subClassOf gkoc:Discrete_Physical_Property ;
.
gkop:Orientation
  a owl:Class ;
  rdfs:subClassOf gkoc:Complex_Physical_Property ;
.
gkop:Particle_Aspect_Ratio_Category
  a owl:Class ;
  rdfs:comment "AspectRatio describes the geometry of particles based on the ratios of lengths of long, intermediate and short axes of grains. Equates to sphericity in sedimentary rocks (ie: the degree to which the shape of a particle approximates a sphere).  A quantitative specification based on the ratio of lengths of long, intermediate and short axes of grain shape (Sneed and Folk, 1958; Zingg, 1935). (eg: prolate, slightly flattened, very bladed, equant, acicular, tabular) "@en ;
  rdfs:isDefinedBy "GeoSciML v4" ;
  rdfs:label "Particle aspect ratio "@en ;
  rdfs:subClassOf gkoc:Discrete_Physical_Property ;
.
gkop:Particle_Sorting_Category
  a owl:Class ;
  rdfs:comment "The Sorting attribute holds text terms to specify size distribution of particles in a CompoundMaterial. Terminology for sorting in sedimentary rocks is based on the quantitative Graphic Standard Deviation (IGSD) scheme proposed by Folk (1968, 1974).  Example terms for this attribute may include sedimentary terms such as well sorted and poorly sorted, or igneous terms such as porphyritic, equigranuilar, seriate." ;
  rdfs:isDefinedBy "GeoSciML v4" ;
  rdfs:label "Particle sorting" ;
  rdfs:subClassOf gkoc:Discrete_Physical_Property ;
.
gkop:Peak_Pressure
  a owl:Class ;
  rdfs:comment "peak metamorphic pressure" ;
  rdfs:isDefinedBy "GeoSciML v3" ;
  rdfs:label "Peak pressure" ;
  rdfs:subClassOf gkoc:Quantified_Physical_Property ;
.
gkop:Peak_Temperature
  a owl:Class ;
  rdfs:comment "peak metamorphic temperature" ;
  rdfs:isDefinedBy "GeoSciML v3" ;
  rdfs:label "Peak temperature" ;
  rdfs:subClassOf gkoc:Quantified_Physical_Property ;
.
gkop:PlaneOrientationStrikeDip
  a owl:Class ;
  rdfs:comment "specification of the orientation of a plane in space, using a strike (bearing of relative to geographic north of the intersection of plane with local horzontal) and dip (inclination of line normal to strike contained in the plane, measured positive downward in degrees from local horizontal)" ;
  rdfs:label "Plane orientation (strike and dip)" ;
  rdfs:subClassOf gkop:Orientation ;
  rdfs:subClassOf [
      a owl:Restriction ;
      owl:onProperty gkoc:hasPhysicalProperty ;
      owl:someValuesFrom gkop:Dip ;
    ] ;
  rdfs:subClassOf [
      a owl:Restriction ;
      owl:onProperty gkoc:hasPhysicalProperty ;
      owl:someValuesFrom gkop:Strike ;
    ] ;
.
gkop:Plane_OrientationDipDipDirection
  a owl:Class ;
  rdfs:comment "specification of the orientation of a plane in space, using a dip (inclination of line of maximum imnclination contained in the plane, measured positive downward in degrees from local horizontal) and dip direction (bearing relative to geographic north of the horizontal projection of the dip line)"@en ;
  rdfs:label "Plane orientation (dip and dip direction)"@en ;
  rdfs:subClassOf gkop:Orientation ;
  rdfs:subClassOf [
      a owl:Restriction ;
      owl:onProperty gkoc:hasPhysicalProperty ;
      owl:someValuesFrom gkop:Dip ;
    ] ;
  rdfs:subClassOf [
      a owl:Restriction ;
      owl:onProperty gkoc:hasPhysicalProperty ;
      owl:someValuesFrom gkop:Dip_Direction ;
    ] ;
.
gkop:Plunge
  a owl:Class ;
  rdfs:comment "Numeric value should be between +90 and -90.   Negative values only valid if the linear feature is directed." ;
  rdfs:label "Plunge" ;
  rdfs:subClassOf gkoc:Quantified_Physical_Property ;
.
gkop:Rock_Material_Color
  a owl:Class ;
  rdfs:comment "Property for specification of color of rocks, minerals, other Earth Material "@en ;
  rdfs:label "Earth Material Color"@en ;
  rdfs:subClassOf gkoc:Discrete_Physical_Property ;
  rdfs:subClassOf [
      a owl:Restriction ;
      owl:onProperty gkop:hasTermValue ;
      owl:someValuesFrom gkoc:Any_Color ;
    ] ;
.
gkop:Rock_Material_Composition_Category
  a owl:Class ;
  rdfs:comment "Term to specify the gross compositional character of a compound material. Composition as used here is loosely construed to include both chemical composition and petrograpic composition, thus multiple values may be applied to a single rock, e.g. metaluminous and alkalic, undersaturated and basic, etc. Terms would typically include broad chemical classifications such as silicate, carbonate, ferromagnesian, oxide.  However, this attribute may have different terminology for different kinds of rocks - for example sandstone petrographic classification terms (e.g. feldspathic) might be placed here."@en ;
  rdfs:isDefinedBy "GeoSciML v4" ;
  rdfs:label "Rock material composition category" ;
  rdfs:subClassOf gkoc:Discrete_Physical_Property ;
.
gkop:Separation
  a owl:Class ;
  rdfs:comment "a vector (magnitude and orientation) specifying the distance between the intersection of a surface on opposite sides of a displacment surface. In 3-D is the projection of a vector normal to the displaced surface into the displacment surface, but might also be specified as offset of the intersection of displacement surface and marker surface in some other profile view (e.g. horizontal/map view, or a cross section)"@en ;
  rdfs:label "Separation" ;
  rdfs:subClassOf gkop:Displacement ;
.
gkop:Slip
  a owl:Class ;
  rdfs:comment "a vector (magnitude and orientation) that links a peircing point on opposite sides of a displacement surface."@en ;
  rdfs:label "Slip"@en ;
  rdfs:subClassOf gkop:Displacement ;
.
gkop:Strike
  a owl:Class ;
  rdfs:comment "" ;
  rdfs:label "Strike" ;
  rdfs:subClassOf gkoc:Quantified_Physical_Property ;
.
gkop:Thickness
  a owl:Class ;
  rdfs:subClassOf gkoc:Quantified_Physical_Property ;
.
gkop:Trend
  a owl:Class ;
  rdfs:comment "" ;
  rdfs:label "Trend" ;
  rdfs:subClassOf gkoc:Quantified_Physical_Property ;
.
