# baseURI: http://loop3d.org/GSO/ontology/2020/1/alteredrockmaterial/ontology

@prefix alty: <http://loop3d.org/GSO/ontology/2020/1/alteredrockmaterial/> .
@prefix gslth: <http://loop3d.org/GSO/ontology/2020/1/lithology/> .
@prefix gsog: <http://loop3d.org/GSO/ontology/2020/1/geologicfeature/> .
@prefix gsoq: <http://loop3d.org/GSO/ontology/2020/1/geologicquality/> .
@prefix owl: <http://www.w3.org/2002/07/owl#> .
@prefix rdf: <http://www.w3.org/1999/02/22-rdf-syntax-ns#> .
@prefix rdfs: <http://www.w3.org/2000/01/rdf-schema#> .
@prefix xml: <http://www.w3.org/XML/1998/namespace> .
@prefix xsd: <http://www.w3.org/2001/XMLSchema#> .

alty:advanced_argillic_altered_rock
  a owl:Class ;
  rdfs:comment "Advanced argillic alteration occurs under lower pH and higher temperature conditions than argillic alteration. Kaolinite and dickite occur at lower temperatures whereas pyrophyllite and andalusite occur under high temperature conditions (T > 300°C). Quartz deposition is common. Alunite, topaz, zunyite, tourmaline, enargite and tennantite may also occur. In many cases, advanced argillic alteration zones, or “lithocaps”, develop at shallow levels above porphyry Cu–Au deposits (e.g., Lepanto-Far Southeast, Philippines; Maricunga, Chile). Advanced argillic alteration mineral assemblages precipitate from SO2- and HCl-rich magmatic vapor, which arises from an underlying intrusive source, and can also form in supergene environments, due to post-hydrothermal weathering and oxidation of pyrite, locally creating pH<1 liquid due to high concentrations of H2SO4 within the vadose zone, where kaolinite and alunite plus Fe hydroxides form."@en ;
  rdfs:comment "dct:source--  Antonio Arribas, Jeffrey Hedenquist, 2019, Environments of advanced argillic alteration: II) steam-heated, and exploration implications: Conference: Society of Resource Geology Annual SymposiumAt: University of Tokyo, Tokyo (Japan)Volume: 69, accessed at https://www.researchgate.net/publication/334230797_Environments_of_advanced_argillic_alteration_II_steam-heated_and_exploration_implications#fullTextFileContent; Constantinos Mavrogonatos et al., 2018, Mineralogical Study of the Advanced Argillic Alteration Zone at the Konos Hill Mo–Cu–Re–Au Porphyry Prospect, NE Greece: Minerals, 8, 479; doi:10.3390/min8110479;  https://en.wikipedia.org/wiki/Argillic_alteration"@en ;
  rdfs:label "advanced argillic altered rock"@en ;
  rdfs:subClassOf alty:altered_rock ;
.
alty:albitic_altered_rock
  a owl:Class ;
  rdfs:comment "dct:source--  CGI alterationtype SKOS vocabulary 2012-11-24"@en ;
  rdfs:comment "definition missing"@en ;
  rdfs:label "albitic altered rock"@en ;
  rdfs:subClassOf alty:altered_rock ;
.
alty:altered_rock
  a owl:Class ;
  rdfs:comment "Rock material has been changed by some subsurface alteration process, but the nature of the alteration is not specified."@en ;
  rdfs:label "Altered, type not specified "@en ;
  rdfs:subClassOf gslth:Metasomatic_rock ;
.
alty:alunitic_altered_rock
  a owl:Class ;
  rdfs:comment "dct:source--  CGI alterationtype SKOS vocabulary 2012-11-24"@en ;
  rdfs:comment "definition missing"@en ;
  rdfs:label "alunitic altered rock"@en ;
  rdfs:subClassOf alty:altered_rock ;
.
alty:argillic_altered_rock
  a owl:Class ;
  rdfs:comment "Argillic alteration is hydrothermal alteration of wall rock which introduces clay minerals including kaolinite, smectite and illite. The process generally occurs at low temperatures and may occur in atmospheric conditions. Argillic alteration is representative of supergene environments where low temperature groundwater becomes acidic. Argillic assemblages include kaolinite replacing plagioclase and montmorillonite replacing amphibole and plagioclase. Orthoclase is generally stable and unaffected. Argillic grades into phyllic alteration at higher temperatures in an ore deposit hydrothermal system."@en ;
  rdfs:comment "dct:source--  https://en.wikipedia.org/wiki/Argillic_alteration"@en ;
  rdfs:label "argillic altered rock"@en ;
  rdfs:subClassOf alty:altered_rock ;
.
alty:calcsilicate_altered_rock
  a owl:Class ;
  rdfs:comment "dct:source--  CGI alterationtype SKOS vocabulary 2012-11-24"@en ;
  rdfs:comment "definition missing"@en ;
  rdfs:label "calcsilicate altered rock"@en ;
  rdfs:subClassOf alty:altered_rock ;
.
alty:carbonate_altered_rock
  a owl:Class ;
  rdfs:comment "dct:source--  CGI alterationtype SKOS vocabulary 2012-11-24"@en ;
  rdfs:comment "definition missing"@en ;
  rdfs:label "carbonate altered rock"@en ;
  rdfs:subClassOf alty:altered_rock ;
.
alty:chloritic_altered_rock
  a owl:Class ;
  rdfs:comment "dct:source--  CGI alterationtype SKOS vocabulary 2012-11-24"@en ;
  rdfs:comment "definition missing"@en ;
  rdfs:label "chloritic altered rock"@en ;
  rdfs:subClassOf alty:altered_rock ;
.
alty:deuteric_altered_rock
  a owl:Class ;
  rdfs:comment "dct:source--  CGI alterationtype SKOS vocabulary 2012-11-24"@en ;
  rdfs:comment "definition missing"@en ;
  rdfs:label "deuteric altered rock"@en ;
  rdfs:subClassOf alty:altered_rock ;
.
alty:epidote_altered_rock
  a owl:Class ;
  rdfs:comment "dct:source--  CGI alterationtype SKOS vocabulary 2012-11-24"@en ;
  rdfs:comment "definition missing"@en ;
  rdfs:label "epidote altered rock"@en ;
  rdfs:subClassOf alty:altered_rock ;
.
alty:greisen
  a owl:Class ;
  rdfs:comment "Greisen is a class of endoskarn,  formed by self-generated alteration of a granite. Greisens appear as partly coarse, crystalline granite, partly vuggy with miarolitic cavities, disseminated halide minerals such as fluorite, and occasionally metallic oxide and sulfide ore minerals, borate minerals (tourmaline) and accessory phases such as sphene, beryl or topaz."@en ;
  rdfs:comment "dct:source--  https://en.wikipedia.org/wiki/Greisen"@en ;
  rdfs:label "greisen"@en ;
  rdfs:subClassOf alty:altered_rock ;
.
alty:hematitic_altered_rock
  a owl:Class ;
  rdfs:comment "dct:source--  CGI alterationtype SKOS vocabulary 2012-11-24"@en ;
  rdfs:comment "definition missing"@en ;
  rdfs:label "hematitic altered rock"@en ;
  rdfs:subClassOf alty:altered_rock ;
.
alty:kaolinitic_altered_rock
  a owl:Class ;
  rdfs:comment "dct:source--  CGI alterationtype SKOS vocabulary 2012-11-24"@en ;
  rdfs:comment "definition missing"@en ;
  rdfs:label "kaolinitic altered rock"@en ;
  rdfs:subClassOf alty:altered_rock ;
.
alty:not_altered_rock
  a owl:Class ;
  rdfs:comment "Material without any significant secondary alteration."@en ;
  rdfs:comment "dct:source--  CGI alterationtype SKOS vocabulary 2012-11-24"@en ;
  rdfs:label "material not altered"@en ;
  rdfs:subClassOf gslth:Metasomatic_rock ;
.
alty:ontology
  a owl:Ontology ;
  rdfs:comment "This vocabulary is for specification of Altered rock material categories, based on the IUGS Commission for Geoscience Information (CGI) Geoscience Terminology Working Group. Original development for populating the alteration type property in GeoSciML alterationDescription elements adopted for gsoq:Alteration_Type in GSO/Loop3D ontology. Definitions of alteration types have not been included."@en ;
  rdfs:comment "dct:creator--  CGI Concept Definition Task Group, Stpehen Richard convert to owl for Loop3D project, add definitions, change from alteration type to altered rock materials"@en ;
  rdfs:comment "dct:date--  2012-11-24"@en ;
  rdfs:comment "dct:modified-- 2020-07-18"@en ;
  rdfs:label "Altered Rock Materials"@en ;
  rdfs:seeAlso "http://resource.geosciml.org/classifier/cgi/alterationtype"@en ;
  rdfs:seeAlso "http://resource.geosciml.org/vocabulary/cgi/2016/alterationtype.rdf"@en ;
.
alty:phyllic_altered_rock
  a owl:Class ;
  rdfs:comment "Altered rock characterised by the assemblage of quartz + sericite + pyrite, and occurs at high temperatures and moderately acidic (low pH) conditions. Typically associated with copper porphyry ore deposits in calc-alkaline rocks."@en ;
  rdfs:comment "dct:source--  https://en.wikipedia.org/wiki/Phyllic_alteration"@en ;
  rdfs:label "phyllic altered rock"@en ;
  rdfs:subClassOf alty:altered_rock ;
.
alty:potassic_altered_rock
  a owl:Class ;
  rdfs:comment "dct:source--  CGI alterationtype SKOS vocabulary 2012-11-24"@en ;
  rdfs:comment "definition missing"@en ;
  rdfs:label "potassic altered rock"@en ;
  rdfs:subClassOf alty:altered_rock ;
.
alty:propylitic_altered_rock
  a owl:Class ;
  rdfs:comment "dct:source--  CGI alterationtype SKOS vocabulary 2012-11-24"@en ;
  rdfs:comment "definition missing"@en ;
  rdfs:label "propylitic altered rock"@en ;
  rdfs:subClassOf alty:altered_rock ;
.
alty:pyritic_altered_rock
  a owl:Class ;
  rdfs:comment "dct:source--  CGI alterationtype SKOS vocabulary 2012-11-24"@en ;
  rdfs:comment "definition missing"@en ;
  rdfs:label "pyritic altered rock"@en ;
  rdfs:subClassOf alty:altered_rock ;
.
alty:red_rock_altered_rock
  a owl:Class ;
  rdfs:comment "Alteration characterized by finely dispersed hematite"@en ;
  rdfs:comment "dct:source--  CGI alterationtype SKOS vocabulary 2012-11-24"@en ;
  rdfs:comment "dct:source-- Williams, P.J., 1994, Aust. J. Earth Science, v41, p381-382" ;
  rdfs:label "red rock altered rock"@en ;
  rdfs:subClassOf alty:altered_rock ;
.
alty:saussuritised_rock
  a owl:Class ;
  rdfs:comment "Rock in which calcium-bearing plagioclase feldspar is altered to an assemblage of minerals called saussurite, typically including zoisite, chlorite, amphibole, and carbonate minerals. Residual fluids present during the late stages of magmatic crystallization can react with previously formed plagioclase feldspar to form saussurite; the saussurite will be spread through the plagioclase or located near its outer margin. The plagioclase may be reconstituted into a more sodium-rich variety (albite), although the original form of the crystal is retained. Later hydrothermal alteration can produce the same result. Mafic rocks are especially susceptible to saussuritization owing to their high calcium content; the more calcium-rich portions of plagioclase in acidic rocks also are often saussuritized."@en ;
  rdfs:comment "dct:source--  https://www.britannica.com/science/saussuritization"@en ;
  rdfs:label "saussuritised rock"@en ;
  rdfs:subClassOf alty:altered_rock ;
.
alty:sericitic_altered_rock
  a owl:Class ;
  rdfs:comment "Rock in which plagioclase feldspar has been converted to sericite, an informal term for  fine-grained white phyllosilicate minerals. Commonly associated with phyllic altered rocks, used to describe less intense alteration."@en ;
  rdfs:comment "dct:source--  https://en.wikipedia.org/wiki/Sericitic_alteration"@en ;
  rdfs:label "sericitic altered rock"@en ;
  rdfs:subClassOf alty:altered_rock ;
.
alty:serpentinised_rock
  a owl:Class ;
  rdfs:comment "dct:source--  CGI alterationtype SKOS vocabulary 2012-11-24"@en ;
  rdfs:comment "definition missing"@en ;
  rdfs:label "serpentinised rock"@en ;
  rdfs:subClassOf alty:altered_rock ;
.
alty:silicified_rock
  a owl:Class ;
  rdfs:comment "dct:source--  CGI alterationtype SKOS vocabulary 2012-11-24"@en ;
  rdfs:comment "definition missing"@en ;
  rdfs:label "silicificed rock"@en ;
  rdfs:subClassOf alty:altered_rock ;
.
alty:uralitised_rock
  a owl:Class ;
  rdfs:comment "dct:source--  CGI alterationtype SKOS vocabulary 2012-11-24"@en ;
  rdfs:comment "definition missing"@en ;
  rdfs:label "uralitised rock"@en ;
  rdfs:subClassOf alty:altered_rock ;
.
alty:zeolitic_altered_rock
  a owl:Class ;
  rdfs:comment "dct:source--  CGI alterationtype SKOS vocabulary 2012-11-24"@en ;
  rdfs:comment "definition missing"@en ;
  rdfs:label "zeolitic altered rock"@en ;
  rdfs:subClassOf alty:altered_rock ;
.
