# baseURI: http://loop3d.org/GSO/ontology/2020/1/lithology/particleaspectratio/ontology
# imports: http://purl.org/dc/terms/


@prefix owl: <http://www.w3.org/2002/07/owl#> .
@prefix rdf: <http://www.w3.org/1999/02/22-rdf-syntax-ns#> .
@prefix xml: <http://www.w3.org/XML/1998/namespace> .
@prefix xsd: <http://www.w3.org/2001/XMLSchema#> .
@prefix rdfs: <http://www.w3.org/2000/01/rdf-schema#> .
@prefix gsog: <http://loop3d.org/GSO/ontology/2020/1/geologicfeature/> .
@prefix gslth: <http://loop3d.org/GSO/ontology/2020/1/lithology/> .
@prefix gsmg: <http://loop3d.org/GSO/ontology/2020/1/metamorphicgrade/> .
@prefix gsmf: <http://loop3d.org/GSO/ontology/2020/1/metamorphicfacies/> .
@prefix gsoc: <http://loop3d.org/GSO/ontology/2020/1/common/> .
@prefix gsop: <http://loop3d.org/GSO/ontology/2020/1/geologicproperty/> .
@prefix gsar: <http://loop3d.org/GSO/ontology/2020/1/lithology/particleaspectratio/> .
@prefix xlink: <http://www.w3.org/1999/xlink> .
@prefix dcterms: <http://purl.org/dc/terms/> .
@base <http://www.w3.org/2002/07/owl#> .


###  http://loop3d.org/GSO/ontology/2020/1/lithology/particleaspectratio/any_form
<http://loop3d.org/GSO/ontology/2020/1/lithology/particleaspectratio/any_form> rdf:type 
               owl:Class ; 
      dcterms:source "this vocabulary"@en ;
      rdfs:subClassOf <http://loop3d.org/GSO/ontology/2020/1/lithology/particleaspectratio/form_not_specified> ;
      rdfs:comment "Particle has some form, but it is not specified."@en ;

      rdfs:label "any form"@en .


###  http://loop3d.org/GSO/ontology/2020/1/lithology/particleaspectratio/bladed
<http://loop3d.org/GSO/ontology/2020/1/lithology/particleaspectratio/bladed> rdf:type 
             owl:Class ; 
    dcterms:source "Sneed and Folk, 1958, Pettijohn et al., 1972, NADM SLTTs, 2004"@en ;
    rdfs:subClassOf <http://loop3d.org/GSO/ontology/2020/1/lithology/particleaspectratio/any_form> ;
    rdfs:comment "Bladed group in Sneed&Folk, (1958), S/L is less than 0.7 and (L-I)/(L-S) is between 0.33 and 0.66."@en ;
    
    rdfs:label "bladed"@en .


###  http://loop3d.org/GSO/ontology/2020/1/lithology/particleaspectratio/bladed_medium
<http://loop3d.org/GSO/ontology/2020/1/lithology/particleaspectratio/bladed_medium> rdf:type 
                    owl:Class ; 
           dcterms:source "Sneed and Folk, 1958, Pettijohn et al., 1972, NADM SLTTs, 2004"@en ;
           rdfs:subClassOf <http://loop3d.org/GSO/ontology/2020/1/lithology/particleaspectratio/bladed> ;
           rdfs:comment "S/L is between 0.3 and 0.5 and (L-I)/(L-S) is between 0.33 and 0.66 Sneed&Folk, (1958)."@en ;
           
           rdfs:label "bladed medium"@en .


###  http://loop3d.org/GSO/ontology/2020/1/lithology/particleaspectratio/compact_bladed
<http://loop3d.org/GSO/ontology/2020/1/lithology/particleaspectratio/compact_bladed> rdf:type 
                     owl:Class ; 
            dcterms:source "Sneed and Folk, 1958, Pettijohn et al., 1972, NADM SLTTs, 2004"@en ;
            rdfs:subClassOf <http://loop3d.org/GSO/ontology/2020/1/lithology/particleaspectratio/bladed> ;
            rdfs:comment "S/L is between 0.5 and 0.7 and (L-I)/(L-S) is between 0.33 and 0.66 Sneed&Folk, (1958)."@en ;
            
            rdfs:label "compact bladed"@en .


###  http://loop3d.org/GSO/ontology/2020/1/lithology/particleaspectratio/equant
<http://loop3d.org/GSO/ontology/2020/1/lithology/particleaspectratio/equant> rdf:type 
             owl:Class ; 
    dcterms:source "Sneed and Folk, 1958, Pettijohn et al., 1972, NADM SLTTs, 2004"@en ;
    rdfs:subClassOf <http://loop3d.org/GSO/ontology/2020/1/lithology/particleaspectratio/any_form> ;
    rdfs:comment "Particles are compact in Sneed & Folk (1958), ratio of S/L is greater than 0.7."@en ;
    
    rdfs:label "equant"@en .


###  http://loop3d.org/GSO/ontology/2020/1/lithology/particleaspectratio/fibrous
<http://loop3d.org/GSO/ontology/2020/1/lithology/particleaspectratio/fibrous> rdf:type 
              owl:Class ; 
     dcterms:source "Sneed and Folk, 1958, Pettijohn et al., 1972, NADM SLTTs, 2004"@en ;
     rdfs:subClassOf <http://loop3d.org/GSO/ontology/2020/1/lithology/particleaspectratio/strongly_prolate> ;
     rdfs:comment "Particles are so elongate they are fibrous."@en ;
     
     rdfs:label "fibrous"@en .


###  http://loop3d.org/GSO/ontology/2020/1/lithology/particleaspectratio/form_not_specified
<http://loop3d.org/GSO/ontology/2020/1/lithology/particleaspectratio/form_not_specified> rdf:type 
                         owl:Class ; 
                dcterms:source "this vocabulary"@en ;
                rdfs:comment "Particle form may take any or no value. For use in normative descriptions."@en ;

                rdfs:label "form not specified"@en ;
                rdfs:subClassOf gslth:Particle_Aspect_Ratio_Space .


###  http://loop3d.org/GSO/ontology/2020/1/lithology/particleaspectratio/oblate
<http://loop3d.org/GSO/ontology/2020/1/lithology/particleaspectratio/oblate> rdf:type 
             owl:Class ; 
    dcterms:source "Sneed and Folk, 1958, Pettijohn et al., 1972, NADM SLTTs, 2004"@en ;
    rdfs:subClassOf <http://loop3d.org/GSO/ontology/2020/1/lithology/particleaspectratio/any_form> ;
    rdfs:comment "Particles are in 'platy group' in Sneed&Folk, (1958), S/L is less than 0.7 and (L-I)/(L-S) is less than 0.33."@en ;

    rdfs:label "oblate"@en .


###  http://loop3d.org/GSO/ontology/2020/1/lithology/particleaspectratio/oblate_medium
<http://loop3d.org/GSO/ontology/2020/1/lithology/particleaspectratio/oblate_medium> rdf:type 
                    owl:Class ; 
           dcterms:source "Sneed and Folk, 1958, Pettijohn et al., 1972, NADM SLTTs, 2004"@en ;
           rdfs:subClassOf <http://loop3d.org/GSO/ontology/2020/1/lithology/particleaspectratio/oblate> ;
           rdfs:comment "Particles are 'just platy' in Sneed&Folk, (1958), S/L is between 0.3 and 0.5 and (L-I)/(L-S) is less than 0.33."@en ;
           
           rdfs:label "oblate medium"@en .


###  http://loop3d.org/GSO/ontology/2020/1/lithology/particleaspectratio/particle_geometry_uncertain
<http://loop3d.org/GSO/ontology/2020/1/lithology/particleaspectratio/particle_geometry_uncertain> rdf:type 
                                  owl:Class ; 
                         dcterms:source "this vocabulary"@en ;
                         rdfs:subClassOf <http://loop3d.org/GSO/ontology/2020/1/lithology/particleaspectratio/form_not_specified> ;
                         rdfs:comment "Particle form is uncertain or not categorizable, generally obscured by overprinting deformation, metamorphism, or alteration, but reason is not specified."@en ;
                         
                         rdfs:label "particle form indeterminate"@en .


###  http://loop3d.org/GSO/ontology/2020/1/lithology/particleaspectratio/prolate
<http://loop3d.org/GSO/ontology/2020/1/lithology/particleaspectratio/prolate> rdf:type 
              owl:Class ; 
     dcterms:source "Sneed and Folk, 1958, Pettijohn et al., 1972, NADM SLTTs, 2004"@en ;
     rdfs:subClassOf <http://loop3d.org/GSO/ontology/2020/1/lithology/particleaspectratio/any_form> ;
     rdfs:comment "Particles are in 'elongated group' in Sneed & Folk, (1958), S/L is less than 0.7 and (L-I)/(L-S) is greater than 0.66."@en ;

     rdfs:label "prolate"@en .


###  http://loop3d.org/GSO/ontology/2020/1/lithology/particleaspectratio/prolate_medium
<http://loop3d.org/GSO/ontology/2020/1/lithology/particleaspectratio/prolate_medium> rdf:type 
                     owl:Class ; 
            dcterms:source "Sneed and Folk, 1958, Pettijohn et al., 1972, NADM SLTTs, 2004"@en ;
            rdfs:subClassOf <http://loop3d.org/GSO/ontology/2020/1/lithology/particleaspectratio/prolate> ;
            rdfs:comment "Particle are 'just elongated' in Sneed&Folk, (1958), S/L is between 0.3 and 0.5 and (L-I)/(L-S) is greater than 0.66."@en ;
            
            rdfs:label "prolate medium"@en .


###  http://loop3d.org/GSO/ontology/2020/1/lithology/particleaspectratio/slightly_flattened
<http://loop3d.org/GSO/ontology/2020/1/lithology/particleaspectratio/slightly_flattened> rdf:type 
                         owl:Class ; 
                dcterms:source "Sneed and Folk, 1958, Pettijohn et al., 1972, NADM SLTTs, 2004"@en ;
                rdfs:subClassOf <http://loop3d.org/GSO/ontology/2020/1/lithology/particleaspectratio/oblate> ;
                rdfs:comment "Particles are 'Compact-platy' in Sneed&Folk, (1958), S/L is between 0.5 and 0.7 and (L-I)/(L-S) is less than 0.33."@en ;
                
                rdfs:label "slightly flattened"@en .


###  http://loop3d.org/GSO/ontology/2020/1/lithology/particleaspectratio/slightly_prolate
<http://loop3d.org/GSO/ontology/2020/1/lithology/particleaspectratio/slightly_prolate> rdf:type 
                       owl:Class ; 
              dcterms:source "Sneed and Folk, 1958, Pettijohn et al., 1972, NADM SLTTs, 2004"@en ;
              rdfs:subClassOf <http://loop3d.org/GSO/ontology/2020/1/lithology/particleaspectratio/prolate> ;
              rdfs:comment "Particles are compact-elongated in Sneed&Folk, (1958), S/L is between 0.5 and 0.7 and (L-I)/(L-S) is greater than 0.66."@en ;
              
              rdfs:label "slightly prolate"@en .


###  http://loop3d.org/GSO/ontology/2020/1/lithology/particleaspectratio/strongly_flattened
<http://loop3d.org/GSO/ontology/2020/1/lithology/particleaspectratio/strongly_flattened> rdf:type 
                         owl:Class ; 
                dcterms:source "Sneed and Folk, 1958, Pettijohn et al., 1972, NADM SLTTs, 2004"@en ;
                rdfs:subClassOf <http://loop3d.org/GSO/ontology/2020/1/lithology/particleaspectratio/oblate> ;
                rdfs:comment "Particles are 'very platy' in Sneed&Folk, (1958), S/L is less than 0.3 and (L-I)/(L-S) is less than 0.33."@en ;
                
                rdfs:label "strongly flattened"@en .


###  http://loop3d.org/GSO/ontology/2020/1/lithology/particleaspectratio/strongly_prolate
<http://loop3d.org/GSO/ontology/2020/1/lithology/particleaspectratio/strongly_prolate> rdf:type 
                       owl:Class ; 
              dcterms:source "Sneed and Folk, 1958, Pettijohn et al., 1972, NADM SLTTs, 2004"@en ;
              rdfs:subClassOf <http://loop3d.org/GSO/ontology/2020/1/lithology/particleaspectratio/prolate> ;
              rdfs:comment "Particles are very elongated in Sneed&Folk, (1958), S/L is less than 0.3 and (L-I)/(L-S) is greater than 0.66."@en ;

              rdfs:label "strongly prolate"@en .


###  http://loop3d.org/GSO/ontology/2020/1/lithology/particleaspectratio/very_bladed
<http://loop3d.org/GSO/ontology/2020/1/lithology/particleaspectratio/very_bladed> rdf:type 
                  owl:Class ; 
         dcterms:source "Sneed and Folk, 1958, Pettijohn et al., 1972, NADM SLTTs, 2004"@en ;
         rdfs:subClassOf <http://loop3d.org/GSO/ontology/2020/1/lithology/particleaspectratio/bladed> ;
         rdfs:comment "S/L is less than 0.3 and (L-I)/(L-S) is between 0.33 and 0.66 Sneed&Folk, (1958)."@en ;
         
         rdfs:label "very bladed"@en .


###  http://loop3d.org/GSO/ontology/2020/1/lithology/particleaspectratio/ontology
<http://loop3d.org/GSO/ontology/2020/1/lithology/particleaspectratio/ontology> rdf:type 
                    owl:Ontology ;
           dcterms:creator "CGI Geoscience Terminology Working Group, OWL version by Stephen Richard"@en  ;
           dcterms:date "2016-11-25"@en  ;
		   dcterms:modified "2020-01-30"@en  ;
           dcterms:description "This file contains the CGI Particle Aspect Ratio vocabulary, as defined by the IUGS Commission for Geoscience Information (CGI) Geoscience Terminology Working Group. AspectRatio describes the geometry of particles based on the ratios of lengths of long, intermediate and short axes of grains. Equates to sphericity in sedimentary rocks (ie: the degree to which the shape of a particle approximates a sphere). A quantitative specification is based on the ratio of lengths of long, intermediate and short axes of grain shape (Sneed and Folk, 1958; Zingg, 1935). This vocabulary includes terms for specifying average shape of some collection of particles.(eg: prolate, slightly flattened, very bladed, equant, acicular, tabular). Numeric shape values from Sneed and Folk (1958) are best understood by looking at the pictures of particles with the different shapes there and in Pettijohn et al. (1972)."@en ;
           rdfs:label "Particle Aspect Ratio"@en ;
           rdfs:comment  "This file contains the 2016 SKOS-RDF version of the CGI Particle Aspect Ratio vocabulary. Compilation and review in MS Excel spreadsheet, converted to MS Excel for SKOS generation using SKOS_for_GA_from_XLS_2016.03.xslt"@en ;
		     owl:imports dcterms: ;
            .


###  Generated by the OWL API (version 4.5.9.2019-02-01T07:24:44Z) https://github.com/owlcs/owlapi
