# baseURI: http://geoscience.ca/3D/ontology/2019/1/ex-complexcontact
# imports: http://geoscience.ca/3D/ontology/2019/1/geologicfeature
# imports: http://purl.org/dc/elements/1.1/

@prefix : <http://geoscience.ca/3D/ontology/2019/1/ex-complexcontact#> .
@prefix common: <http://geoscience.ca/3D/ontology/2019/1/common/> .
@prefix con: <http://geoscience.ca/3D/ontology/2019/1/ex-complexcontact#> .
@prefix dc: <http://purl.org/dc/elements/1.1/> .
@prefix geo: <http://geoscience.ca/3D/ontology/2019/1/geologicfeature/> .
@prefix gkm: <http://geoscience.ca/3D/ontology/2019/1/geologicfeature> .
@prefix owl: <http://www.w3.org/2002/07/owl#> .
@prefix rdf: <http://www.w3.org/1999/02/22-rdf-syntax-ns#> .
@prefix rdfs: <http://www.w3.org/2000/01/rdf-schema#> .
@prefix xml: <http://www.w3.org/XML/1998/namespace> .
@prefix xsd: <http://www.w3.org/2001/XMLSchema#> .

common:Surface
  rdfs:comment "Surface (SF): A boundary in 3D space that is neither line nor point, but area"@en ;
.
<http://geoscience.ca/3D/ontology/2019/1/ex-complexcontact>
  a owl:Ontology ;
  rdfs:comment "Focus is Js, a Jurassic age sedimentary unit that has a lower clastic part with an internal tuff marker bed, and an upper limestone part. The unit unconformably overlies tilted Paleozoic strata that overly Early Proterozoic metamorphic rocks; it is intruded by a Cretaceous granite, and the granite and Js are intruded by a Cretaceous diorite dike. After the igneous activity a period of exumation and erosion removed the cover on the Jurassic sediment and Cretaceous igneous rocks, and Late Miocene sediment covered this unconformity."@en ;
  rdfs:comment "Xm, Cb, Os, and Ss and their boundary surfaces not elucidated here"@en ;
  rdfs:comment "this example references the GeologyScenarioForTesting diagram"@en ;
  owl:imports <http://geoscience.ca/3D/ontology/2019/1/geologicfeature> ;
  owl:imports dc: ;
.
con:CbFormation
  a geo:Formation ;
  rdfs:label "Bolsa Quartzite (Cambrian)"@en ;
.
con:JsDeposition
  a geo:Deposition ;
  rdfs:label "Deposition of Unit Js"@en ;
.
con:JsFormation
  a geo:Formation ;
  common:hasPart con:KdInJsDikeContact-3_1_4 ;
  common:hasPart con:KdInJsDikeContact-3_2_4 ;
  common:hasPart con:KgInJsIntrusiveContact-4_2 ;
  common:hasPart con:baseJs-6 ;
  common:hasPart con:topJs-2 ;
  geo:hasTemporalProperty [
      a geo:Chronostratigraphic_Age_Interval ;
      geo:hasOlderAge <http://resource.geosciml.org/classifier/ics/ischart/Jurassic> ;
      geo:hasYoungerAge <http://resource.geosciml.org/classifier/ics/ischart/Jurassic> ;
    ] ;
  rdfs:comment "details of unit description are in a separate Example: GKO-ExampleFormationJs.txt"@en ;
  rdfs:comment "the following parts are not elucidated in this example, but are referenced in the Contact instances below. These surfaces would participate in intrusion and also contact metamorphism processes"@en ;
  rdfs:label "Js Formation"@en ;
.
con:KdDike
  a geo:Formation ;
  common:hasConstituent [
      a geo:Diorite ;
      geo:hasPhysicalProperty [
          geo:hasNumericValue .05 ;
          geo:hasUOM [
              rdfs:type geo:mm ;
            ] ;
          rdfs:type geo:GrainSizeAverage ;
        ] ;
    ] ;
  common:hasPart con:KdUnderMs ;
  common:hasPart con:downSideKd-3_1 ;
  common:hasPart con:upSideKd-3_2 ;
  geo:Intrudes con:CbFormation ;
  geo:Intrudes con:JsFormation ;
  geo:Intrudes con:KgGranite ;
  geo:Intrudes con:XmRockBody ;
  rdfs:comment "dike has lots of intrusive contacts, on the hanging wall (up) and footwall (down) side of the dike, each contact is with a different unit."@en ;
  rdfs:comment "intrudes is subproperty of relatedTo"@en ;
  rdfs:label "Mafic Dike (Cretaceous)"@en ;
.
con:KdInJsDikeContact-3_1_4
  a geo:Rock_Body_Boundary ;
.
con:KdInJsDikeContact-3_2_4
  a geo:Rock_Body_Boundary ;
.
con:KdUnderMs
  a geo:Rock_Body_Boundary ;
  common:participantIn [
      a geo:Erosion ;
    ] ;
  rdfs:comment "Eroded surface under Ms"@en ;
.
con:KgErosionSurface-2_3
  a geo:Rock_Body_Boundary ;
  common:participantIn geo:Erosion ;
  rdfs:comment "Kg erosion surface overlain by Ms"@en ;
.
con:KgGranite
  a geo:Formation ;
  common:hasConstituent [
      a geo:Granitoid ;
      geo:hasPhysicalProperty [
          geo:hasNumericValue 5 ;
          geo:hasUOM [
              rdfs:type geo:mm ;
            ] ;
          rdfs:type geo:GrainSizeAverage ;
        ] ;
    ] ;
  common:hasPart con:KgErosionSurface-2_3 ;
  common:hasPart con:KgIntrusiveBoundary-3_1_3 ;
  common:hasPart con:KgIntrusiveBoundary-3_2_3 ;
  common:hasPart con:KgIntrusiveBoundary-4_1 ;
  common:hasPart con:KgIntrusiveBoundary-4_2 ;
  geo:Intrudes con:CbFormation ;
  geo:Intrudes con:JsFormation ;
  geo:Intrudes con:OsFormation ;
  geo:Intrudes con:XmRockBody ;
  rdfs:comment "contacts are complicated! Here are the parts:"@en ;
  rdfs:comment "intrudes is subproperty of relatedTo"@en ;
  rdfs:comment "intrusion has lots of intrusive contacts, each contact is with a different unit, also an erosion surface at the top, overlain by Ms."@en ;
  rdfs:label "Granite (Cretaceous)"@en ;
.
con:KgInJsIntrusiveContact-4_2
  a geo:Rock_Body_Boundary ;
.
con:KgIntrusiveBoundary-3_1_3
  a geo:Rock_Body_Boundary ;
  common:participantIn geo:Intrusion ;
  rdfs:comment "Kg in footwall wall of Kd contacts"@en ;
.
con:KgIntrusiveBoundary-3_2_3
  a geo:Rock_Body_Boundary ;
  common:participantIn geo:Intrusion ;
  rdfs:comment "Kg in Hanging wall of Kd"@en ;
.
con:KgIntrusiveBoundary-4_1
  a geo:Rock_Body_Boundary ;
  common:hasPart con:KgIntrusiveBoundary-4_1_1 ;
  common:hasPart con:KgIntrusiveBoundary-4_1_2 ;
  common:hasPart con:KgIntrusiveBoundary-4_1_3 ;
  common:participantIn geo:Intrusion ;
  rdfs:comment "Kg intruding the tilted Xm-Cb-Os-Ss sequence"@en ;
.
con:KgIntrusiveBoundary-4_1_1
  a geo:Rock_Body_Boundary ;
  common:HostedBy con:KgGranite ;
  rdfs:comment "Kg intruding the tilted Xm"@en ;
.
con:KgIntrusiveBoundary-4_1_2
  a geo:Rock_Body_Boundary ;
  rdfs:comment "Kg intruding tilted Cb"@en ;
.
con:KgIntrusiveBoundary-4_1_3
  a geo:Rock_Body_Boundary ;
  rdfs:comment "Kg intruding tilted Os"@en ;
.
con:KgIntrusiveBoundary-4_2
  a geo:Rock_Body_Boundary ;
  common:participantIn geo:Intrusion ;
  rdfs:comment "Kg intruding Js"@en ;
.
con:MsFormation
  a geo:Formation ;
  common:hasConstituent [
      a geo:Rock_Material ;
      rdfs:comment "TBD"@en ;
    ] ;
  common:hasPart con:baseMs-2 ;
  common:hasPart con:topMs-1 ;
  rdfs:comment "fine-grained sandstone, minor marl, some coquina"@en ;
  rdfs:label "Ms Formation"@en ;
.
con:OsBoundary-6_2
  a geo:Rock_Body_Boundary ;
.
con:OsFormation
  a geo:Formation ;
  rdfs:label "Sedimentary Rocks (Ordovician)"@en ;
.
con:SsBoundary-6_1
  a geo:Rock_Body_Boundary ;
.
con:XmBoundary-6_3
  a geo:Rock_Body_Boundary ;
  common:participantIn [
      a geo:Erosion ;
    ] ;
  geo:hasOlderHost con:XmFormation ;
  geo:hasYoungerHost con:JsFormation ;
.
con:XmFormation
  a geo:Complex ;
.
con:XmRockBody
  a geo:Complex ;
.
con:baseJs-6
  a geo:Rock_Body_Bottom ;
  common:hasPart con:baseJs-6_1 ;
  common:hasPart con:baseJs-6_2 ;
  common:hasPart con:baseJs-6_3 ;
.
con:baseJs-6_1
  a geo:Rock_Body_Bottom ;
  common:participantIn con:JsDeposition ;
  rdfs:comment "Js on Ss surface"@en ;
.
con:baseJs-6_2
  a geo:Rock_Body_Bottom ;
  common:participantIn con:JsDeposition ;
  rdfs:comment "Js on Os surface"@en ;
.
con:baseJs-6_3
  a geo:Rock_Body_Bottom ;
  common:participantIn con:JsDeposition ;
  rdfs:comment "Js on Xm surface"@en ;
.
con:baseMs-2
  a geo:Rock_Body_Bottom ;
  common:HostedBy con:MsFormation ;
  common:hasPart con:baseMs-2_1 ;
  common:hasPart con:baseMs-2_2 ;
  common:hasPart con:baseMs-2_3 ;
  common:participantIn [
      a geo:Deposition ;
    ] ;
  rdfs:comment "This is an unconformity; Ms overlies Jurassic sediment, Cretaceous dike and granite"@en ;
  rdfs:comment "base of Ms formation"@en ;
  rdfs:label "Base Ms"@en ;
.
con:baseMs-2_1
  a geo:Rock_Body_Bottom ;
  rdfs:comment "surface separating Ms on top of Js"@en ;
  rdfs:label "Ms overlies Js"@en ;
.
con:baseMs-2_2
  a geo:Rock_Body_Bottom ;
  rdfs:comment "surface separating Ms on top of Kd"@en ;
  rdfs:label "Ms overlies Kd dike"@en ;
.
con:baseMs-2_3
  a geo:Rock_Body_Bottom ;
  rdfs:comment "surface separating Ms on top of Kg"@en ;
  rdfs:label "Ms overlies Kg"@en ;
.
con:contact_Js_on_Os
  a geo:Contact ;
  geo:hasOlderHost con:OsBoundary-6_2 ;
  geo:hasOlderHost con:OsFormation ;
  geo:hasYoungerHost con:JsFormation ;
  geo:hasYoungerHost con:baseJs-6_2 ;
  rdfs:comment "OsBoundary-6_2 is Erosional Surface"@en ;
  rdfs:label "relational feature, Js formation overlies Os Formation"@en ;
.
con:contact_Js_on_Ss
  a geo:Contact ;
  geo:hasOlderHost con:SsBoundary-6_1 ;
  geo:hasOlderHost con:SsFormation ;
  geo:hasYoungerHost con:JsFormation ;
  geo:hasYoungerHost con:baseJs-6_1 ;
  rdfs:comment "SsBoundary-6_1 is Erosional Surface"@en ;
  rdfs:label "relational feature, Js formation overlies Ss Formation"@en ;
.
con:contact_Js_on_Xm
  a geo:Contact ;
  common:HostedBy con:XmBoundary-6_3 ;
  common:HostedBy con:baseJs-6_3 ;
  geo:hasOlderHost con:XmFormation ;
  geo:hasYoungerHost con:JsFormation ;
  rdfs:label "relational feature, Js formation overlies Xm Rock Body"@en ;
.
con:contact_Kd_in_Js
  a geo:Contact ;
  geo:hasOlderHost con:JsFormation ;
  geo:hasOlderHost con:KdInJsDikeContact-3_1_4 ;
  geo:hasOlderHost con:KdInJsDikeContact-3_2_4 ;
  geo:hasYoungerHost con:KdDike ;
  geo:hasYoungerHost con:downSide-3_1_4 ;
  geo:hasYoungerHost con:upSideKd-3_2_4 ;
  rdfs:label "relational feature, Kd dike intrudes Js formation"@en ;
.
con:contact_Kg_in_Js
  a geo:Contact ;
  geo:hasOlderHost con:JsFormation ;
  geo:hasOlderHost con:KgInJsIntrusiveContact-4_2 ;
  geo:hasYoungerHost con:KgGranite ;
  geo:hasYoungerHost con:KgIntrusiveBoundary-4_2 ;
  rdfs:label "relational feature, Kg granite intrudes Js formation"@en ;
.
con:contact_Ms_on_Js
  a geo:Contact ;
  geo:hasOlderHost con:JsFormation ;
  geo:hasOlderHost con:topJs-2_1 ;
  geo:hasYoungerHost con:MsFormation ;
  geo:hasYoungerHost con:baseMs-2_1 ;
  rdfs:label "relational feature, Ms formation overlies Js formation"@en ;
.
con:contact_Ms_on_Kg
  a geo:Contact ;
  geo:hasOlderHost con:KgErosionSurface-2_3 ;
  geo:hasOlderHost con:KgGranite ;
  geo:hasYoungerHost con:MsFormation ;
  geo:hasYoungerHost con:baseMs-2_3 ;
  rdfs:label "relational feature, Ms formation overlies Kg Granite on erosion surface"@en ;
.
con:downSide-3_1_4
  a geo:Rock_Body_Boundary ;
  rdfs:comment "surface separating dike from rocks beneath it"@en ;
  rdfs:label "dike intrudes Js, lower"@en ;
.
con:downSideKd-3_1
  a geo:Rock_Body_Boundary ;
  common:hasPart con:downSideKd-3_1_1 ;
  common:hasPart con:downSideKd-3_1_2 ;
  common:hasPart con:downSideKd-3_1_3 ;
  common:hasPart con:downSideKd-3_1_4 ;
  common:participantIn [
      a geo:Intrusion ;
    ] ;
  rdfs:comment "lower side of dike"@en ;
.
con:downSideKd-3_1_1
  a geo:Rock_Body_Boundary ;
  rdfs:comment "could have more properties describing contact effectw sith Xm here"@en ;
.
con:downSideKd-3_1_2
  a geo:Rock_Body_Boundary ;
.
con:downSideKd-3_1_3
  a geo:Rock_Body_Boundary ;
.
con:downSideKd-3_1_4
  a geo:Rock_Body_Boundary ;
  rdfs:comment "dike intrudes Js"@en ;
.
con:topJs-2_1
  a geo:Rock_Body_Top ;
  common:participantIn [
      a geo:Erosion ;
    ] ;
.
con:topMs-1
  a geo:Rock_Body_Top ;
  common:HostedBy con:MsFormation ;
  rdfs:comment "This is a simple disconformable contact"@en ;
  rdfs:comment "top of Ms formation"@en ;
  rdfs:label "Top Ms"@en ;
.
con:upSideKd-3_2
  a geo:Rock_Body_Boundary ;
  common:hasPart con:upSideKd-3_2_1 ;
  common:hasPart con:upSideKd-3_2_2 ;
  common:hasPart con:upSideKd-3_2_3 ;
  common:hasPart con:upSideKd-3_2_4 ;
  common:participantIn [
      a geo:Intrusion ;
    ] ;
  rdfs:comment "upper side of dike"@en ;
.
con:upSideKd-3_2_1
  a geo:Rock_Body_Boundary ;
  rdfs:comment "dike intrudes Xm"@en ;
.
con:upSideKd-3_2_2
  a geo:Rock_Body_Boundary ;
  rdfs:comment "dike intrudes Cb"@en ;
.
con:upSideKd-3_2_3
  a geo:Rock_Body_Boundary ;
  rdfs:comment "dike intrudes Kg"@en ;
.
con:upSideKd-3_2_4
  a geo:Rock_Body_Boundary ;
  rdfs:comment "dike intrudes Js"@en ;
.
geo:Complex
  dc:description "A lithostratigraphic unit composed of diverse types of any class or classes or rocks (sedimentary, igneous, metamorphic) and characterized by irregularly mixed lithology or by highly complicated structural relations. http://www.stratigraphy.org/upload/bak/litho.htm"@en ;
.
geo:Formation
  dc:description "The primary formal unit of lithostratigraphic classification. Formations are the only formal lithostratigraphic units into which the stratigraphic column everywhere should be divided completely on the basis of lithology. The contrast in lithology between formations required to justify their establishment varies with the complexity of the geology of a region and the detail needed for geologic mapping and to work out its geologic history. No formation is considered justifiable and useful that cannot be delineated at the scale of geologic mapping practiced in the region. The thickness of formations may range from less than a meter to several thousand meters. http://www.stratigraphy.org/upload/bak/litho.htm"@en ;
  rdfs:label "Formation"@en ;
.
geo:Lithostratigraphic_Unit
  dc:description "A body of rocks that is defined and recognized on the basis of its lithologic properties or combination of lithologic properties and stratigraphic relations. A lithostratigraphic unit may consist of sedimentary, or igneous, or metamorphic rocks. Lithostratigraphic units are defined and recognized by observable physical features and not by their inferred age, the time span they represent, inferred geologic history, or manner of formation. The geographic extent of a lithostratigraphic unit is controlled entirely by the continuity and extent of its diagnostic lithologic features.  http://www.stratigraphy.org/upload/bak/litho.htm"@en ;
.
geo:Quantified_Physical_Property
  rdfs:subClassOf [
      a owl:Restriction ;
      owl:onProperty geo:hasNumericValue ;
      owl:someValuesFrom xsd:double ;
    ] ;
  rdfs:subClassOf [
      a owl:Restriction ;
      owl:onProperty geo:hasUOM ;
      owl:someValuesFrom common:uom ;
    ] ;
.
geo:hasMethod
  rdfs:range common:Measurement_Method ;
.
geo:hasSpatialProperty
  rdfs:range common:Spatial_Extent ;
.
geo:proportionOf
  rdfs:domain geo:Proportion ;
.
