# baseURI: http://geoscience.ca/3D/ontology/2019/1/ex-timescale
# imports: http://geoscience.ca/3D/ontology/2019/1/common
# imports: http://geoscience.ca/3D/ontology/2019/1/geologicfeature
# imports: http://purl.org/dc/elements/1.1/
# prefix: tim

@prefix : <http://geoscience.ca/3D/ontology/2019/1/ex-timescale#> .
@prefix common: <http://geoscience.ca/3D/ontology/2019/1/common/> .
@prefix geo: <http://geoscience.ca/3D/ontology/2019/1/geologicfeature/> .
@prefix owl: <http://www.w3.org/2002/07/owl#> .
@prefix rdf: <http://www.w3.org/1999/02/22-rdf-syntax-ns#> .
@prefix rdfs: <http://www.w3.org/2000/01/rdf-schema#> .
@prefix skos: <http://www.w3.org/2004/02/skos/core#> .
@prefix tim: <http://geoscience.ca/3D/ontology/2019/1/ex-timescale#> .
@prefix xml: <http://www.w3.org/XML/1998/namespace> .
@prefix xsd: <http://www.w3.org/2001/XMLSchema#> .

common:Dynamic_Feature
  a owl:Class ;
  rdfs:comment "" ;
  rdfs:label "Dynamic Feature" ;
  rdfs:subClassOf <http://geoscience.ca/3D/ontology/2019/1/gkmtop#physical-feature> ;
  skos:prefLabel "Dynamic Feature" ;
.
common:Gap
  a owl:Class ;
  rdfs:comment """A physical void with a scattered (disconnected) host, consisting of the spaces between the scattered parts of the host.  G(x) <--> exists y [hosts-v(y,x) ^ not ICon (y)].   ICon (x): x is interior connected (continuous, not scattered)   {@en}
""" ;
  rdfs:label "Gap" ;
  rdfs:subClassOf common:Physical_Void ;
  skos:prefLabel "Gap" ;
.
common:Hole
  a owl:Class ;
  rdfs:comment """A physical void with a self-connected (non-scattered) host, consisting of some depression or cavity within the host. H(x) <--> exists y [hosts-v(y,x) ^ ICon (y)].  ICon (x): x is interior connected (continuous, not scattered)  {@en}
""" ;
  rdfs:label "Hole" ;
  rdfs:subClassOf common:Physical_Void ;
  skos:prefLabel "Hole" ;
.
common:Inherent_Feature
  rdfs:subClassOf <http://geoscience.ca/3D/ontology/2019/1/gkmtop#physical-feature> ;
.
common:Integral_Feature
  rdfs:subClassOf <http://geoscience.ca/3D/ontology/2019/1/gkmtop#physical-feature> ;
.
common:Part_Feature
  rdfs:subClassOf <http://geoscience.ca/3D/ontology/2019/1/gkmtop#physical-feature> ;
.
common:Process
  owl:equivalentClass <http://geoscience.ca/3D/ontology/2019/1/gkmtop#Process> ;
.
common:Spatial_Feature
  rdfs:subClassOf <http://geoscience.ca/3D/ontology/2019/1/gkmtop#physical-feature> ;
.
<http://geoscience.ca/3D/ontology/2019/1/ex-timescale>
  a owl:Ontology ;
  rdfs:comment "Example encoding of a geochronologic time interval" ;
  owl:imports <http://geoscience.ca/3D/ontology/2019/1/common> ;
  owl:imports <http://geoscience.ca/3D/ontology/2019/1/geologicfeature> ;
  owl:imports <http://purl.org/dc/elements/1.1/> ;
.
tim:Lower_Jurassic_Chronostrat_Unit
  a geo:Series ;
  geo:realizes tim:Lower_Jurassic_Epoch ;
  rdfs:comment "ISC2017 time scale does not define stratotypes for the Geochronologic Eras it defines" ;
  rdfs:comment "see Table 3 in http://www.stratigraphy.org/upload/bak/chron.htm for hierarchy of chronostrat and geochron unit names" ;
  rdfs:label "Lower Jurassic rocks" ;
.
tim:Lower_Jurassic_Epoch
  a geo:Epoch ;
  common:isPartOf <http://resource.geosciml.org/vocabulary/timescale/isc2017> ;
  geo:hasOlderDate [
      geo:hasDate 201.3 ;
      geo:hasUOM [
          rdfs:type common:ma ;
        ] ;
      geo:hasUncertainty 0.2 ;
      geo:isRealizedBy <http://resource.geosciml.org/classifier/ics/ischart/BaseJurassic> ;
      geo:stratotype <http://resource.geosciml.org/classifier/ics/ischart/BaseJurassicSP> ;
      rdfs:type geo:Geochronologic_Boundary ;
    ] ;
  geo:hasYoungerDate [
      geo:hasDate 174.1 ;
      geo:hasUOM [
          rdfs:type common:ma ;
        ] ;
      geo:hasUncertainty 1.0 ;
      geo:isRealizedBy <http://resource.geosciml.org/classifier/ics/ischart/BaseMiddleJurassic> ;
      geo:stratotype <http://resource.geosciml.org/classifier/ics/ischart/BaseMiddleJurassicSP> ;
      rdfs:comment "the Base Middle Jurassic class represents all rock body surfaces correlated with the surface at the Global Stratotype Point" ;
      rdfs:type geo:Geochronologic_Boundary ;
    ] ;
  rdfs:comment "Epoch is a subclass of Geochronologic Era" ;
  rdfs:comment "This is a temporal interval" ;
  rdfs:label "Lower Jurassic time interval" ;
.
geo:Geologic_Structure
  rdfs:comment "A pattern in a rock body (foliation, fold), or a feature occurring between rock bodies (contact, fracture). GeoSciML 3.2: A configuration of matter in the Earth based on describable inhomogeneity, pattern, or fracture in a Rock Body. The identity of a GeologicStructure is independent of the material that is the substrate for the structure.    Properties like \"clast-supported\",  \"matrix-supported\", and \"graded bed\" that do not involve orientation are considered kinds of GeologicStructure because they depend on the configuration of parts of a rock body. Includes sedimentary structures."@en ;
  rdfs:subClassOf <http://geoscience.ca/3D/ontology/2019/1/gkmtop#physical-feature> ;
.
geo:Geologic_Unit
  rdfs:subClassOf <http://geoscience.ca/3D/ontology/2019/1/gkmtop#Physical_Object> ;
.
<http://geoscience.ca/3D/ontology/2019/1/gkmtop#Event>
  rdfs:subClassOf [
      a owl:Restriction ;
      owl:allValuesFrom <http://geoscience.ca/3D/ontology/2019/1/gkmtop#Process> ;
      owl:onProperty geo:isManifestationOf ;
    ] ;
.
<http://geoscience.ca/3D/ontology/2019/1/gkmtop#Perdurant>
  rdfs:subClassOf <http://geoscience.ca/3D/ontology/2019/1/gkmtop#Particular> ;
  rdfs:subClassOf [
      a owl:Restriction ;
      owl:allValuesFrom common:Spatial_Extent ;
      owl:onProperty geo:hasSpatialProperty ;
    ] ;
  rdfs:subClassOf [
      a owl:Restriction ;
      owl:allValuesFrom geo:Physical_Setting ;
      owl:onProperty geo:hasSetting ;
    ] ;
  rdfs:subClassOf [
      a owl:Restriction ;
      owl:allValuesFrom geo:Temporal_Property ;
      owl:onProperty geo:hasTemporalProperty ;
    ] ;
  rdfs:subClassOf [
      a owl:Restriction ;
      owl:allValuesFrom <http://geoscience.ca/3D/ontology/2019/1/gkmtop#Perdurant> ;
      owl:onProperty common:isPartOf ;
    ] ;
  rdfs:subClassOf [
      a owl:Restriction ;
      owl:allValuesFrom <http://geoscience.ca/3D/ontology/2019/1/gkmtop#Perdurant> ;
      owl:onProperty geo:isTemporallyRelatedTo ;
    ] ;
.
<http://geoscience.ca/3D/ontology/2019/1/gkmtop#physical-feature>
  a owl:Class ;
  rdfs:comment "All features are specifically dependent on their hosts -  that is, the hosts relation is a subrelation of specific dependence.  F(x) <--> exists y [hosts(y,x)]"@en ;
  rdfs:label "Physical Feature"@en ;
  rdfs:subClassOf <http://geoscience.ca/3D/ontology/2019/1/gkmtop#Physical_Endurant> ;
  skos:prefLabel "Physical Feature"@en ;
.
<http://geoscience.ca/3D/ontology/2019/1/gkmtop#space-region>
  rdfs:label "Spatial Region"@en ;
.
