# baseURI: http://loop3d.org/GSO/ontology/2020/1/alterationtype-bc/ontology
# imports: http://loop3d.org/GSO/ontology/2020/1/alterationtype/ontology ;
# prefix: bcalt


@prefix alty: <http://loop3d.org/GSO/ontology/2020/1/alterationtype/> .
@prefix bcalt: <http://loop3d.org/GSO/ontology/2020/1/alterationtype-bc/> .
@prefix gsoq: <http://loop3d.org/GSO/ontology/2020/1/geologicquality/> .
@prefix owl: <http://www.w3.org/2002/07/owl#> .
@prefix rdf: <http://www.w3.org/1999/02/22-rdf-syntax-ns#> .
@prefix rdfs: <http://www.w3.org/2000/01/rdf-schema#> .
@prefix xml: <http://www.w3.org/XML/1998/namespace> .
@prefix xsd: <http://www.w3.org/2001/XMLSchema#> .


bcalt:ontology
  a owl:Ontology ;
  rdfs:comment "Extend CGI alteration type vocabulary to account for alteration reported in British Columbia Geological Survey, 2008, Rock Properties Database"@en ;
  rdfs:comment "dct:source-- SMR provisional 2020-06-15" @en ;
  rdfs:comment "dct:date-- 2020-06-15 "@en ;
  rdfs:label "British Columbia Alteration Type"@en ;
    rdfs:comment "dct:source -- British Columbia Geological Survey, 2008, Rock Properties Database:  Ministry of Energy, Mines and Petroleum Resources, BC Geological Survey, access online at https://catalogue.data.gov.bc.ca/dataset/2dc8a4f1-c8f8-4603-813e-855af99b7ba5/resource/51f0620a-42cf-458f-821c-bdd895f24fdc/download/of2008-4rpd.xls; see accompanying report http://www.geosciencebc.com/i/pdf/FinalReports/GBCReport_2008-9.pdf" @en ;
    owl:imports alty:ontology ;
.

bcalt:disseminated_sulphide_mineral
  a owl:Class ;
  rdfs:comment "dct:source--  British Columbia Geological Survey, 2008, Rock Properties Database"@en ;
  rdfs:comment "Alteration characterized by introduction of various sulphide minerals as framework constituents in altered rock."@en ;
  rdfs:comment "dct:source-- SMR provisional 2020-06-15" @en ;
  rdfs:label "disseminated sulphide minerals alteration"@en ;
  rdfs:subClassOf bcalt:introduced_sulphide_mineral ;
.

bcalt:introduced_sulphide_mineral
  a owl:Class ;
  rdfs:comment "dct:source--  British Columbia Geological Survey, 2008, Rock Properties Database"@en ;
  rdfs:comment "Alteration characterized by introduction of various sulphide minerals into a protolith rock as a product of hydrothermal alteration, includes veinlets, disseminated, replacement..."@en ;
  rdfs:comment "dct:source-- SMR provisional 2020-06-15" @en ;
  rdfs:label "sulphide minerals present"@en ;
  rdfs:subClassOf alty:altered ;
.


bcalt:sulphide_veinlet_alteration
  a owl:Class ;
  rdfs:comment "dct:source--  British Columbia Geological Survey, 2008, Rock Properties Database"@en ;
  rdfs:comment "Alteration characterized by introduction of various sulphide minerals as veinlets in rock body. Silica and other minerals may accompany sulphides in veinlets; alteration halos around veinlets are tricky to describe--TBD!."@en ;
  rdfs:comment "dct:source-- SMR provisional 2020-06-15" @en ;
  rdfs:label "sulphide minerals in veinlets"@en ;
  rdfs:subClassOf bcalt:introduced_sulphide_mineral ;
.

alty:pyritic_alteration    rdfs:subClassOf bcalt:introduced_sulphide_mineral .

bcalt:introduced_sulphide_mineral
  a owl:Class ;
  rdfs:comment "dct:source--  British Columbia Geological Survey, 2008, Rock Properties Database"@en ;
  rdfs:comment "Alteration characterized by introduction of various sulphide minerals as framework constituents in altered rock."@en ;
  rdfs:comment "dct:source-- SMR provisional 2020-06-15" @en ;
  rdfs:label "disseminated sulphide minerals alteration"@en ;
  rdfs:subClassOf alty:altered ;
.


bcalt:near_surface_oxidation
  a owl:Class ;
  rdfs:comment "dct:source--  British Columbia Geological Survey, 2008, Rock Properties Database"@en ;
  rdfs:comment "sulphides replaced by oxide minerals, acid leaching due to sulphide to acid reactions."@en ;
  rdfs:comment "dct:source-- SMR provisional 2020-06-15" @en ;
  rdfs:label "Near surface oxidation alteration"@en ;
  rdfs:subClassOf alty:altered ;
.